<?xml version="1.0"?>
<rdf:RDF xmlns="https://github.com/corrado877/CognitiveBiasOntologies/blob/main/CognitiveBiasOntologies.owl#"
     xml:base="https://github.com/corrado877/CognitiveBiasOntologies/blob/main/CognitiveBiasOntologies.owl"
     xmlns:aos="http://www.fao.org/aims/aos/aos.owl#"
     xmlns:cbo="https://github.com/corrado877/CognitiveBiasOntologies/blob/main/CognitiveBiasOntologies#"
     xmlns:owl="http://www.w3.org/2002/07/owl#"
     xmlns:rdf="http://www.w3.org/1999/02/22-rdf-syntax-ns#"
     xmlns:xml="http://www.w3.org/XML/1998/namespace"
     xmlns:xsd="http://www.w3.org/2001/XMLSchema#"
     xmlns:Bias="https://github.com/corrado877/CognitiveBiasOntologies/tree/main/Confabulation%20Bias#"
     xmlns:core="http://purl.org/ontology/cco/core#"
     xmlns:prov="http://www.w3.org/ns/prov#"
     xmlns:rdfs="http://www.w3.org/2000/01/rdf-schema#"
     xmlns:term="http://modellingdh.github.io/ont/odp/term/"
     xmlns:terms="http://purl.org/dc/terms/"
     xmlns:Action="http://www.ontology.se/odp/content/owl/Action.owl#"
     xmlns:partof="http://www.ontologydesignpatterns.org/cp/owl/partof.owl#"
     xmlns:Realism="https://github.com/corrado877/CognitiveBiasOntologies/tree/main/Naive%20Realism#"
     xmlns:Cynicism="https://github.com/corrado877/CognitiveBiasOntologies/tree/main/Naive%20Cynicism#"
     xmlns:ontology="https://dbpedia.org/ontology/"
     xmlns:sequence="http://www.ontologydesignpatterns.org/cp/owl/sequence.owl#"
     xmlns:parameter="http://www.ontologydesignpatterns.org/cp/owl/parameter.owl#"
     xmlns:affectedBy="https://w3id.org/affectedBy#"
     xmlns:RecencyBias="https://github.com/corrado877/CognitiveBiasOntologies/RecencyBias#"
     xmlns:participation="http://www.ontologydesignpatterns.org/cp/owl/participation.owl#"
     xmlns:Naive_Cynicism="https://github.com/corrado877/CognitiveBiasOntologies/tree/main/Naive_Cynicism#"
     xmlns:classification="http://www.ontologydesignpatterns.org/cp/owl/classification.owl#"
     xmlns:participation1="http://ontologydesignpatterns.org/cp/owl/participation.owl#"
     xmlns:ActivityPattern="http://descartes-core.org/ontologies/activities/1.0/ActivityPattern.owl#"
     xmlns:Anthropomorphism="https://github.com/corrado877/CognitiveBiasOntologies/blob/main/Antropomorphism/Anthropomorphism.owl#"
     xmlns:Anecdotal_fallacy="http://www.semanticweb.org/salva/ontologies/2024/1/Anecdotal_fallacy#"
     xmlns:Anecdotal_fallacy1="https://github.com/corrado877/CognitiveBiasOntologies/blob/main/Anecdotal_fallacy/"
     xmlns:Masked_Man_Fallacy="https://github.com/corrado877/CognitiveBiasOntologies/blob/main/Masked_man_fallacy/Masked_Man_Fallacy.owl#"
     xmlns:cpannotationschema="http://www.ontologydesignpatterns.org/schemas/cpannotationschema.owl#"
     xmlns:newsreportingevent="http://semantic.cs.put.poznan.pl/ontologies/newsreportingevent.owl#"
     xmlns:Clustering_illusion="https://github.com/corrado877/CognitiveBiasOntologies/blob/main/Clustering_illusion#"
     xmlns:Illusion_of_validity="https://github.com/corrado877/CognitiveBiasOntologies/blob/main/Illusion_of_validity/Illusion_of_validity.owl#"
     xmlns:untitled-ontology-17="http://www.semanticweb.org/mein/ontologies/2024/2/untitled-ontology-17#"
     xmlns:untitled-ontology-26="http://www.semanticweb.org/mein/ontologies/2024/3/untitled-ontology-26#"
     xmlns:GamblersFallacyOntology="https://github.com/corrado877/CognitiveBiasOntologies/blob/main/GamblersFallacyOntology/GamblersFallacyOntology.owl#"
     xmlns:Neglect_of_probability_bias="https://github.com/corrado877/CognitiveBiasOntologies/blob/main/Neglect_of_probability_bias#"
     xmlns:Insensitivity_to_sample_size="https://github.com/corrado877/CognitiveBiasOntologies/blob/main/Insensitivity_to_sample_size#">
    <owl:Ontology rdf:about="https://github.com/corrado877/CognitiveBiasOntologies/blob/main/CognitiveBiasOntologies_V.2.0.owl#">
        <terms:contributor>Dott. Stefano De Giorgis</terms:contributor>
        <terms:contributor>Prof. Aldo Gangemi</terms:contributor>
        <terms:created>01/03/24</terms:created>
        <terms:created>20/03/2024</terms:created>
        <terms:created>20/3/2024</terms:created>
        <terms:created>27-02-2024</terms:created>
        <terms:created>27/02/2024</terms:created>
        <terms:created>February 2024</terms:created>
        <terms:created rdf:datatype="http://www.w3.org/2001/XMLSchema#dateTime">2024-02-20T00:00:00</terms:created>
        <terms:creator>Alice Picco</terms:creator>
        <terms:creator>Corrado Consiglio</terms:creator>
        <terms:creator xml:lang="en">Corrado Consiglio</terms:creator>
        <terms:creator>Marco La Morte</terms:creator>
        <terms:creator>Marco Lamorte</terms:creator>
        <terms:creator>Salvatore Di Marzo</terms:creator>
        <terms:description>Anecdotal fallacy part of the Cognitive Bias Ontology</terms:description>
        <terms:description>Bias Blind Spot specification in the Cognitive Bias Ontology</terms:description>
        <terms:description>Clustering illusion part of the Cognitive Bias ontology</terms:description>
        <terms:description>Confabulation Bias specification of Cognitive Bias Ontology</terms:description>
        <terms:description>Insensitivity to sample size part of the Cognitive Bias Ontology</terms:description>
        <terms:description>Naive Cynicism specification of the Cognitive Bias Ontology</terms:description>
        <terms:description>Naive Realism specification of the Cognitive Bias Ontology</terms:description>
        <terms:description>Neglect of probability part of the Cognitive Bias Ontology</terms:description>
        <terms:description>The Anthropomorphism module of the cognitive bias ontology</terms:description>
        <terms:description xml:lang="en">The Cognitive Bias Ontologies constitute a framework for categorizing and defining various cognitive biases that shape human thinking and decision-making. This project is the result of the 2023 Knowledge Representation and Extraction course held by professor Aldo Gangemi at the University of Bologna.</terms:description>
        <terms:description>The Gamblers&apos;Fallacy module of the Cognitive Bias Ontology</terms:description>
        <terms:description>The Hot Hand Fallacy module of the Cognitive Bias Ontology</terms:description>
        <terms:description>The Illusion of validity module of the cognitive bias ontology</terms:description>
        <terms:description>The Illusory of Correlation module of the Cognitive Bias Ontology</terms:description>
        <terms:description>The Masked man fallacy module of the cognitive bias ontology</terms:description>
        <terms:description>The Pareidolia Bias module of the Cognitive Bias Ontology</terms:description>
        <terms:description>The Recency bias module of the cognitive bias ontology</terms:description>
        <terms:title>Anecdotal Fallacy ontology</terms:title>
        <terms:title>Anthropomorphism ontology</terms:title>
        <terms:title>Bias Blind Spot Ontology</terms:title>
        <terms:title>Clustering Illusion Ontology</terms:title>
        <terms:title>Confabulation Bias Ontology</terms:title>
        <terms:title>Hot Hand Fallacy Bias Ontology</terms:title>
        <terms:title>Illusion of validity ontology</terms:title>
        <terms:title>Illusory of Correlation Bias Ontology</terms:title>
        <terms:title>Insensitivity to sample size bias ontology</terms:title>
        <terms:title>Masked Man Fallacy ontology</terms:title>
        <terms:title>Naive Cynicism Ontology</terms:title>
        <terms:title>Naive Realism Ontology</terms:title>
        <terms:title>Neglect of Probability Ontology</terms:title>
        <terms:title>Recency bias ontology</terms:title>
        <terms:title>The Gamblers&apos;Fallacy Ontology Bias</terms:title>
        <terms:title>The Pareidolias Bias Ontology</terms:title>
        <cpannotationschema:hasComponent rdf:resource="http://ontologydesignpatterns.org/wiki/Submissions:AffectedBy"/>
        <cpannotationschema:hasComponent rdf:resource="http://ontologydesignpatterns.org/wiki/Submissions:Parameter"/>
        <cpannotationschema:hasComponent rdf:resource="http://ontologydesignpatterns.org/wiki/Submissions:PartOf"/>
        <cpannotationschema:hasComponent rdf:resource="http://ontologydesignpatterns.org/wiki/Submissions:Participation"/>
        <cpannotationschema:hasComponent rdf:resource="http://ontologydesignpatterns.org/wiki/Submissions:Provenance"/>
        <cpannotationschema:hasComponent rdf:resource="http://ontologydesignpatterns.org/wiki/Submissions:RecurrentEventSeries"/>
        <cpannotationschema:hasComponent rdf:resource="http://ontologydesignpatterns.org/wiki/Submissions:Experience_%26_Observation"/>
        <cpannotationschema:hasComponent rdf:resource="http://purl.org/ontology/cco/20100926/cognitivecharacteristics.html"/>
        <cpannotationschema:hasComponent rdf:resource="https://dbpedia.org/ontology/"/>
        <cpannotationschema:hasComponent rdf:resource="https://www.dbpedia.org/ontology/"/>
        <cpannotationschema:scenarios>In a lottery, a person thinks that a certain number is more likely to be drawn next because it hasn&apos;t been drawn in a long time.</cpannotationschema:scenarios>
        <cpannotationschema:scenarios>Seeing Faces in Inanimate Objects: Perceiving faces in items like electrical sockets, rocks, or tree bark due to the arrangement of patterns or shapes.</cpannotationschema:scenarios>
        <cpannotationschema:scenarios>Sports Betting: A sports bettor assumes that a team that has won several games in a row is more likely to win the next one, overlooking factors like team performance and matchups.</cpannotationschema:scenarios>
        <cpannotationschema:scenarios>Superstitions: A baseball player believes that wearing a specific pair of socks during a winning game brings good luck. However, the socks have no impact on the game&apos;s outcome, yet the player associates wearing them with success.</cpannotationschema:scenarios>
        <untitled-ontology-17:hascomponent>http://ontologydesignpatterns.org/wiki/Submissions:Experience_%26_Observation</untitled-ontology-17:hascomponent>
        <untitled-ontology-17:hascomponent>http://purl.org/ontology/cco/core#</untitled-ontology-17:hascomponent>
        <untitled-ontology-17:hascomponent>https://github.com/corrado877/CognitiveBiasOntologies/tree/main/Bias%20Blind%20Spot</untitled-ontology-17:hascomponent>
        <untitled-ontology-17:hascomponent>https://w3id.org/affectedBy</untitled-ontology-17:hascomponent>
        <untitled-ontology-17:hascomponent>https://w3id.org/framester/data/framestercore</untitled-ontology-17:hascomponent>
        <untitled-ontology-17:userstory>As a product manager, Emily was tasked with prioritizing features for the upcoming software update. Wanting to ensure an objective and user-centric approach, she initiated a team discussion to gather input.
Emily noticed that her colleague, Chris, passionately advocated for a feature related to data visualization, emphasizing its impact on user engagement. As the discussion progressed, Emily felt increasingly convinced that Chris&apos;s viewpoint was swayed by his personal interest in data visualization.
However, during a later discussion, when Emily found herself advocating for a feature that streamlined workflow processes—a functionality she personally valued—she realized the potential bias in her own decision-making. It struck her that, just like Chris, her preferences and experiences were influencing her choices.
Reflecting on this realization, Emily became more mindful of her own bias blind spot. She acknowledged the need to consider a broader range of user perspectives and experiences, recognizing that her personal preferences might not align with the diverse needs of the entire user base. This awareness prompted her to implement a more inclusive decision-making process for feature prioritization, ensuring a balanced consideration of different user needs and preferences.</untitled-ontology-17:userstory>
        <untitled-ontology-26:hascomponent>http://modellingdh.github.io/ont/odp/term</untitled-ontology-26:hascomponent>
        <untitled-ontology-26:hascomponent>https://github.com/corrado877/CognitiveBiasOntologies/tree/main/Naive%20Realism</untitled-ontology-26:hascomponent>
        <untitled-ontology-26:hascomponent>https://purl.org/ontology/cco/core#</untitled-ontology-26:hascomponent>
        <untitled-ontology-26:hascomponent>https://w3id.org/affectedBy</untitled-ontology-26:hascomponent>
        <untitled-ontology-26:hascomponent>https://w3id.org/framester/data/framestercore</untitled-ontology-26:hascomponent>
        <untitled-ontology-26:hascomponent>https://w3id.org/framester/data/framestersyn</untitled-ontology-26:hascomponent>
        <rdfs:comment>Anthropomorphism is a cognitive bias where people attribute human characteristics, emotions, or intentions to non-human entities, objects, or animals. It is a form of personification where human traits are projected onto things that do not possess them.</rdfs:comment>
        <rdfs:comment>Bias Blind Spot refers to the cognitive bias where individuals recognize and easily identify biases in others but fail to acknowledge or perceive their own cognitive biases. It involves the tendency to believe that one is less susceptible to biases than other people, leading individuals to overlook their own subjective judgments and assumptions. The bias blind spot can hinder self-awareness and critical reflection, potentially influencing decision-making, problem-solving, and interpersonal relationships. Recognizing and addressing the bias blind spot is essential for fostering a more accurate and unbiased understanding of one&apos;s own thought processes and behaviors.</rdfs:comment>
        <rdfs:comment>Confabulation bias refers to a cognitive bias characterized by the tendency to generate fabricated or inaccurate information to fill in memory gaps, often without the individual&apos;s awareness. In confabulation, individuals create false details or narratives to explain events, experiences, or gaps in their memory. This bias can occur as a result of memory errors, the brain&apos;s attempt to make sense of incomplete information, or a desire to maintain coherence in one&apos;s personal narrative. Confabulation bias can lead to the creation of vivid and plausible but entirely fictional memories, influencing one&apos;s perception of past events.</rdfs:comment>
        <rdfs:comment xml:lang="en">Illusory correlation bias refers to the tendency of individuals to perceive a relationship between two variables even when no such relationship exists or when the relationship is much weaker than assumed. This bias often occurs when people incorrectly associate two events or characteristics because they occur together in a particular pattern or sequence, leading to the erroneous belief that there is a causal connection between them.</rdfs:comment>
        <rdfs:comment>Insensitivity to sample size bias is a cognitive bias where people misjudge the reliability of information based on the sample size. In simpler terms, we often fail to consider how much a small group represents the larger population. This can lead to drawing false conclusions and making poor decisions.
People tend to treat small and large samples as equally representative, neglecting the increased accuracy of larger samples. We overgeneralize from small samples, applying their findings to the broader population without considering the margin of error.
It&apos;s related to other biases like the clustering illusion, where we underestimate randomness in small samples.
Our intuition struggles with the complex relationship between sample size and statistical uncertainty, we often lack the statistical training to analyse data critically and assess its generalizability, heuristics, which are mental shortcuts, can lead us to jump to conclusions without enough evidence.</rdfs:comment>
        <rdfs:comment>Naive cynicism is a cognitive bias characterized by the tendency to doubt others&apos; intentions and perceive actions as driven by selfish motives or ulterior motives, even in the absence of concrete evidence supporting such skepticism. Individuals exhibiting naive cynicism often display a general distrust of others, assuming that individuals or groups have hidden agendas, leading to a distorted and overly negative interpretation of people&apos;s behaviors or actions. This bias can hinder effective communication, collaboration, and relationship-building, as it contributes to an unwarranted suspicion of others&apos; motives.</rdfs:comment>
        <rdfs:comment>Naive realism is a cognitive bias characterized by the belief that one&apos;s perception of reality is objective, accurate, and unbiased. Individuals exhibiting naive realism assume that they see the world as it truly is, and they often expect others to share the same perception. This bias can lead to the misconception that one&apos;s perspective is the only valid viewpoint, overlooking the subjective nature of perception and the fact that others may interpret and experience reality differently. Naive realism can contribute to misunderstandings, conflicts, and a lack of empathy as individuals may struggle to appreciate alternative perspectives.</rdfs:comment>
        <rdfs:comment>Pareidolia bias is a psychological phenomenon in which individuals perceive familiar patterns, shapes, or meaningful images, such as faces or objects, where none actually exist. This tendency leads people to interpret ambiguous stimuli as something recognizable and significant, even when there is no intentional design or pattern present. Pareidolia bias can occur in various sensory modalities, including visual, auditory, and tactile, and it often influences how individuals interpret stimuli in their environment, such as seeing shapes in clouds or faces in inanimate objects. This bias reflects the brain&apos;s natural inclination to organize and make sense of sensory information, sometimes leading to the perception of patterns or meanings that are not objectively there.</rdfs:comment>
        <rdfs:comment xml:lang="en">The Gambler&apos;s Fallacy bias, also known as the Fallacy of the Maturity of Chances, is a cognitive bias that occurs when an individual believes that past events in a random or chance-based process can influence the likelihood of future events in the same process. It is a mistaken belief that, because a certain outcome has occurred frequently or infrequently in the past, the probability of that outcome occurring again in the future is somehow altered or &quot;due&quot; to happen.</rdfs:comment>
        <rdfs:comment xml:lang="en">The Hot Hand Fallacy Bias, also known as the Hot Hand Fallacy, is a cognitive bias that leads people to believe that a series of successful outcomes in a random or chance-based process is more likely to continue in the short term. In other words, individuals tend to think that if they or someone else has experienced a streak of wins or successes, they are more likely to keep winning or succeeding in the near future. This bias can be observed in various contexts, such as sports, gambling, or even everyday decision-making.</rdfs:comment>
        <rdfs:comment>The Masked Man fallacy, also known as the Illicit Substitution of Identicals, is a cognitive bias where people mistakenly reject two names as referring to the same person or thing if one of the names involves a description or characteristic. This occurs because people tend to treat names as rigid designators and fail to recognize that a masked or described name can refer to the same entity.</rdfs:comment>
        <rdfs:comment>The Recency Bias is a cognitive bias where people give greater importance to recent events and information while discounting older data. This bias can affect decision-making and judgment, as recent experiences may carry more weight in evaluations and assessments.</rdfs:comment>
        <rdfs:comment>The anecdotal fallacy, also known as the anecdotal evidence or personal anecdote fallacy, occurs when someone relies on personal experiences or isolated examples instead of considering a broader range of evidence or statistical data. This bias involves drawing conclusions based on a single or a few examples rather than looking at the larger picture.
While anecdotes can be powerful and emotionally compelling, they are not necessarily representative of the general reality or the overall trend. It&apos;s important to recognize that individual experiences can vary widely, and relying solely on anecdotes may lead to inaccurate or biased conclusions.</rdfs:comment>
        <rdfs:comment>The clustering illusion is a cognitive bias that involves perceiving patterns or clusters in random or unrelated data. People tend to see patterns where none actually exist, and this can lead to incorrect interpretations of information. This bias arises from the human brain&apos;s natural inclination to seek order and make sense of the world, individuals may perceive random events or data points as part of a meaningful pattern or trend. This can occur when there is no actual correlation or connection between the observed elements. The clustering illusion can impact decision-making and judgments, as individuals may base their conclusions on perceived patterns that are not statistically significant or meaningful.</rdfs:comment>
        <rdfs:comment>The neglect of probability bias is a type of cognitive bias that affects how we make decisions, particularly in situations with uncertainty. It boils down to this: a tendency to ignore the probabilities of different outcomes when making decisions, it happens because our brains are complex and sometimes take shortcuts. Considering probabilities takes effort, and sometimes we prioritize other factors like potential rewards or emotional impact. This bias can lead to poor decision-making, especially when dealing with risks and uncertainties. We might overlook likely negative outcomes or get overly fixated on unlikely but dramatic possibilities.</rdfs:comment>
        <rdfs:comment>The “Illusion of Validity” is a cognitive bias where individuals overestimate their ability to accurately interpret and predict outcomes when analyzing a set of data, especially when the data show a consistent pattern</rdfs:comment>
        <rdfs:comment>http://ontologydesignpatterns.org/wiki/Submissions:AOS_AGROVOC_Concept_Server_fundation_ontology_model</rdfs:comment>
        <rdfs:comment>http://ontologydesignpatterns.org/wiki/Submissions:Experience_%26_Observation</rdfs:comment>
        <rdfs:comment>http://ontologydesignpatterns.org/wiki/Submissions:NewsReportingEvent</rdfs:comment>
        <owl:versionInfo>Ver. 2.0</owl:versionInfo>
        <RecencyBias:hasComponent>http://ontologydesignpatterns.org/wiki/Submissions:AOS_AGROVOC_Concept_Server_fundation_ontology_model</RecencyBias:hasComponent>
        <RecencyBias:hasComponent>http://ontologydesignpatterns.org/wiki/Submissions:An_Ontology_Design_Pattern_for_Activity_Reasoning</RecencyBias:hasComponent>
        <RecencyBias:hasComponent>http://ontologydesignpatterns.org/wiki/Submissions:Classification</RecencyBias:hasComponent>
        <RecencyBias:hasComponent>http://ontologydesignpatterns.org/wiki/Submissions:Experience_%26_Observation</RecencyBias:hasComponent>
        <RecencyBias:hasComponent>http://ontologydesignpatterns.org/wiki/Submissions:NewsReportingEvent</RecencyBias:hasComponent>
        <RecencyBias:hasComponent>http://ontologydesignpatterns.org/wiki/Submissions:Parameter</RecencyBias:hasComponent>
        <RecencyBias:hasComponent>http://ontologydesignpatterns.org/wiki/Submissions:Sequence</RecencyBias:hasComponent>
        <RecencyBias:scenarios>In a job interview, a candidate performs exceptionally well in the final part of the interview. The interviewer, influenced by the Recency Bias, places disproportionate weight on this recent performance and is more likely to remember it and give it more significance in the evaluation, potentially overlooking earlier parts of the interview.</RecencyBias:scenarios>
        <Anecdotal_fallacy1:hascomponent>http://ontology.eil.utoronto.ca/icity/ActivitySpecification</Anecdotal_fallacy1:hascomponent>
        <Anecdotal_fallacy1:hascomponent>http://purl.org/ontology/cco/core#</Anecdotal_fallacy1:hascomponent>
        <Anecdotal_fallacy1:hascomponent>http://xmlns.com/foaf/0.1/</Anecdotal_fallacy1:hascomponent>
        <Anecdotal_fallacy1:hascomponent>https://raw.githubusercontent.com/modellingDH/odp_experience/master/owl/cp_experience.owl.rdfxml</Anecdotal_fallacy1:hascomponent>
        <Anecdotal_fallacy1:hascomponent>https://w3id.org/framester/data/framestercore/</Anecdotal_fallacy1:hascomponent>
        <Anecdotal_fallacy1:user_story>As a health-conscious individual, I want to adopt a new diet plan, so that I can achieve my weight loss goals. I will start researching different diet plans available in the market. I come across a testimonial from a friend who claims to have lost a significant amount of weight using the &quot;SuperShred&quot; diet plan. Intrigued by the success story, I decide to follow the &quot;SuperShred&quot; diet plan based on my friend&apos;s positive experience. I diligently adhere to the diet plan for a month, documenting my meals and progress.
At the end of the month, I notice a minimal change in my weight, and I share my experience with others, advocating for the effectiveness of the &quot;SuperShred&quot; diet. However, I fail to consider that individual responses to diet plans can vary, and factors such as metabolism, lifestyle, and overall health play a significant role. Without consulting broader nutritional guidelines or seeking professional advice, I continue promoting the &quot;SuperShred&quot; diet solely based on my personal experience. Over time, I encounter challenges or negative effects that were not apparent in the short term, but I attribute these solely to individual variations rather than considering a more comprehensive understanding of nutrition.</Anecdotal_fallacy1:user_story>
        <Anthropomorphism:hasComponent>http://ontologydesignpatterns.org/wiki/Submissions:Experience_%26_Observation</Anthropomorphism:hasComponent>
        <Anthropomorphism:hasComponent>http://ontologydesignpatterns.org/wiki/Submissions:Move</Anthropomorphism:hasComponent>
        <Anthropomorphism:scenarios>A young child attributes human emotions and intentions to his beloved puppet, Mr. Whiskers, engaging in conversations and interpreting its expressions.</Anthropomorphism:scenarios>
        <Clustering_illusion:hasComponent>http://ontology.eil.utoronto.ca/icity/ActivitySpecification</Clustering_illusion:hasComponent>
        <Clustering_illusion:hasComponent>http://xmlns.com/foaf/0.1/</Clustering_illusion:hasComponent>
        <Clustering_illusion:hasComponent>https://raw.githubusercontent.com/modellingDH/odp_experience/master/owl/cp_experience.owl.rdfxml</Clustering_illusion:hasComponent>
        <Clustering_illusion:hasComponent>https://w3id.org/framester/data/framestercore/</Clustering_illusion:hasComponent>
        <Clustering_illusion:user_story>Sarah, a regular lottery who enjoys testing her luck with weekly ticket purchases. Over the past month, Sarah notices a curious pattern emerging in the winning numbers of the local lottery. She observes that the winning numbers often consist of consecutive digits, such as 12, 13, 14, or alternating pairs like 5 and 7.
Excited by this apparent pattern, Sarah starts to develop a theory that the lottery draws are not entirely random. She begins meticulously analysing past winning numbers, searching for more evidence to support her hypothesis. With each new draw, Sarah eagerly checks the results, hoping to uncover additional patterns or trends.
As the weeks pass, Sarah becomes increasingly convinced that she has cracked the code to winning the lottery. She starts sharing her findings with friends and family, boasting about her newfound strategy for picking winning numbers. Some of her acquaintances start to believe in Sarah&apos;s theory, intrigued by the apparent predictability of the lottery draws.
Sarah decides to invest more money into buying lottery tickets, confident that her strategy will lead to big wins. However, despite her efforts, Sarah&apos;s luck doesn&apos;t seem to improve. She continues to match only a few numbers here and there, never coming close to hitting the jackpot.</Clustering_illusion:user_story>
        <GamblersFallacyOntology:hasComponent rdf:resource="https://dbpedia.org/ontology/"/>
        <Illusion_of_validity:hasComponent>http://ontologydesignpatterns.org/wiki/Submissions:AOS_AGROVOC_Concept_Server_fundation_ontology_model</Illusion_of_validity:hasComponent>
        <Illusion_of_validity:hasComponent>http://ontologydesignpatterns.org/wiki/Submissions:Action</Illusion_of_validity:hasComponent>
        <Illusion_of_validity:hasComponent>http://ontologydesignpatterns.org/wiki/Submissions:An_Ontology_Design_Pattern_for_Activity_Reasoning</Illusion_of_validity:hasComponent>
        <Illusion_of_validity:hasComponent>http://ontologydesignpatterns.org/wiki/Submissions:Experience_%26_Observation</Illusion_of_validity:hasComponent>
        <Illusion_of_validity:hasComponent>http://ontologydesignpatterns.org/wiki/Submissions:NewsReportingEvent</Illusion_of_validity:hasComponent>
        <Illusion_of_validity:hasComponent>http://ontologydesignpatterns.org/wiki/Submissions:Participation</Illusion_of_validity:hasComponent>
        <Illusion_of_validity:scenarios>&quot;John, a seasoned investor, relies on his perceived competence and past successes to make investment decisions, often ignoring the influence of unpredictable factors.&quot;</Illusion_of_validity:scenarios>
        <Insensitivity_to_sample_size:hascomponent>I&apos;m excited for the upcoming release of &quot;Nova Odyssey,&quot; an RPG lauded by several popular streamers I follow. Their glowing reviews have me hyped, but I&apos;m worried about potentially overhyping the game based on a limited perspective. I don&apos;t want to be disappointed if the gameplay doesn&apos;t match my expectations or there are hidden issues not mentioned in the reviews. I want to avoid falling prey to insensitivity to sample size bias and make a well-rounded decision about &quot;Nova Odyssey.&quot; I need tools and information that help me consider diverse perspectives, analyse gameplay beyond streamer opinions, and understand the potential for bias in early reviews. On the Reviewer, I find a mix of professional reviews and player feedback, offering diverse perspectives beyond the streamer hype. While some praise the game&apos;s visuals and story, others point out bugs and repetitive gameplay mechanics. This balanced view helps me manage my expectations.</Insensitivity_to_sample_size:hascomponent>
        <Insensitivity_to_sample_size:hascomponent>http://ontology.eil.utoronto.ca/icity/ActivitySpecification</Insensitivity_to_sample_size:hascomponent>
        <Insensitivity_to_sample_size:hascomponent>http://xmlns.com/foaf/0.1/</Insensitivity_to_sample_size:hascomponent>
        <Insensitivity_to_sample_size:hascomponent>https://raw.githubusercontent.com/modellingDH/odp_experience/master/owl/cp_experience.owl.rdfxml</Insensitivity_to_sample_size:hascomponent>
        <Insensitivity_to_sample_size:hascomponent>https://w3id.org/affectedBy</Insensitivity_to_sample_size:hascomponent>
        <Insensitivity_to_sample_size:hascomponent>https://w3id.org/framester/data/framestercore/</Insensitivity_to_sample_size:hascomponent>
        <Masked_Man_Fallacy:Scenarios>A man enters a local jazz club and is told that the great saxophonist John Smith will play that night. It happens to be also the name of a local talented surgeon. Immediately he refuses to believe that they are the same person, in his biased reasoning someone can&apos;t excel in two such diverse professions.</Masked_Man_Fallacy:Scenarios>
        <Neglect_of_probability_bias:hascomponent>http://ontology.eil.utoronto.ca/icity/ActivitySpecification</Neglect_of_probability_bias:hascomponent>
        <Neglect_of_probability_bias:hascomponent>http://xmlns.com/foaf/0.1/</Neglect_of_probability_bias:hascomponent>
        <Neglect_of_probability_bias:hascomponent>https://github.com/corrado877/CognitiveBiasOntologies/tree/main/Pareidolia%20Ontology</Neglect_of_probability_bias:hascomponent>
        <Neglect_of_probability_bias:hascomponent>https://raw.githubusercontent.com/modellingDH/odp_experience/master/owl/cp_experience.owl.rdfxml</Neglect_of_probability_bias:hascomponent>
        <Neglect_of_probability_bias:hascomponent>https://w3id.org/affectedBy</Neglect_of_probability_bias:hascomponent>
        <Neglect_of_probability_bias:hascomponent>https://w3id.org/framester/data/framestercore/</Neglect_of_probability_bias:hascomponent>
        <Neglect_of_probability_bias:user_story>The world whizzed by Amelia in a blur of emails, meetings, and looming deadlines. Each day felt like a sprint, with tasks piling up like dominoes ready to topple into chaos. But Amelia had a secret weapon - procrastination. While others fretted, she&apos;d glide through her mornings, savoring a leisurely coffee, lost in the latest meme video. &quot;There&apos;s plenty of time,&quot; she&apos;d reassure herself, &quot;the deadline is ages away.&quot;
But deadlines, like mythical dragons, had a way of sneaking up unexpectedly. One morning, the notification popped up - her major presentation, the one she&apos;d been casually pushing off like a dusty book, was due tomorrow. Panic clawed at her throat. The Improbable Dragon, as she&apos;d named her tendency to underestimate the urgency of tasks, had finally caught her.
Frantic typing filled the night, fuelled by cold pizza and desperation. The once manageable presentation morphed into a monster, swallowing her confidence and sleep. By morning, she was a hollow shell, her eyes bloodshot, her voice hoarse. The presentation stumbled, riddled with errors and apologies. The consequences, once improbable, materialized - a lost opportunity, a damaged reputation, and a mountain of work to fix the mess.</Neglect_of_probability_bias:user_story>
        <Bias:hascomponent>http://dbpedia.org/ontology/</Bias:hascomponent>
        <Bias:hascomponent>http://ontologydesignpatterns.org/wiki/Submissions:Experience_%26_Observation</Bias:hascomponent>
        <Bias:hascomponent>http://purl.org/ontology/cco/core#</Bias:hascomponent>
        <Bias:hascomponent>https://github.com/corrado877/CognitiveBiasOntologies/tree/main/Confabulation%20Bias</Bias:hascomponent>
        <Bias:hascomponent>https://w3id.org/affectedBy</Bias:hascomponent>
        <Bias:hascomponent>https://w3id.org/framester/data/framestercore</Bias:hascomponent>
        <Bias:hascomponent>https://www.w3.org/TR/rdf-schema/</Bias:hascomponent>
        <Bias:userstory>Sarah, eager to enjoy a spontaneous night with friends, attends a concert that extends well into the early morning hours. However, mindful of her family&apos;s expectations and knowing that she didn&apos;t inform them of her plans, she faces a dilemma.
The next morning, Sarah returns home, realizing she needs to explain her late-night absence. Feeling the pressure of potential consequences, she succumbs to confabulation bias. When her concerned family asks about her whereabouts, Sarah, without a clear memory of the night&apos;s events, fabricates a story about unexpectedly meeting an old friend who needed emotional support.
In her confabulated narrative, Sarah embellishes details about the encounter, creating a plausible and emotionally charged scenario to justify her late return. Unaware of the confabulation bias at play, she confidently shares this story with her family, believing it to be a genuine account of the night.
This user story highlights how confabulation bias can emerge in situations where individuals feel the need to explain their actions, especially when faced with potential scrutiny or consequences. Sarah&apos;s fabricated story, influenced by the desire to maintain coherence in her personal narrative, exemplifies the impact of confabulation on memory and communication.</Bias:userstory>
        <Cynicism:hascomponent>http://ontologydesignpatterns.org/wiki/Submissions:Experience_%26_Observation</Cynicism:hascomponent>
        <Cynicism:hascomponent>https://github.com/corrado877/CognitiveBiasOntologies/tree/main/Naive%20Cynicism</Cynicism:hascomponent>
        <Cynicism:hascomponent>https://w3id.org/framester/data/framestercore/</Cynicism:hascomponent>
        <Cynicism:userstory>Sarah, having experienced similar challenges in the past, approaches Alex and offers her assistance. She suggests collaborating on specific tasks, sharing resources, and even providing guidance to ease the workload. Her intention is rooted in empathy and a desire to foster teamwork within the department.
However, due to his naive cynicism, Alex, already stressed by the demanding project, interprets Sarah&apos;s generous offer with suspicion. He questions her motives, wondering if she&apos;s attempting to showcase her skills to gain favor with their manager or if there&apos;s an underlying agenda that might compromise his position on the project.
Despite Sarah&apos;s genuine intentions, Alex&apos;s naive cynicism leads him to decline her offer, assuming that there must be hidden motives behind her willingness to help. This scenario illustrates how naive cynicism can hinder collaboration and prevent the positive outcomes that could arise from genuine acts of assistance and teamwork.</Cynicism:userstory>
        <Realism:userstory>Maria, rooted in her cultural traditions, suggests a lively and dynamic event featuring music and dance styles typical of her background. She believes her proposal perfectly represents the essence of cultural celebration. However, her perspective is influenced by naive realism, as she assumes that her cultural traditions are universally appealing and should be the focal point of the event.
Akio, on the other hand, proposes a more serene and contemplative event that aligns with traditional Japanese cultural practices. He believes this approach would better capture the spirit of diversity and inclusivity. Akio, too, is influenced by naive realism, as he assumes that his cultural traditions represent an objective and superior choice for the event.
As the two colleagues engage in discussions about the cultural event, their naive realism becomes apparent. Maria and Akio struggle to appreciate the validity of each other&apos;s cultural traditions, assuming that their own perspectives represent an objective and universal truth.</Realism:userstory>
    </owl:Ontology>
    


    <!-- 
    ///////////////////////////////////////////////////////////////////////////////////////
    //
    // Annotation properties
    //
    ///////////////////////////////////////////////////////////////////////////////////////
     -->

    


    <!-- http://purl.org/dc/terms/contributor -->

    <owl:AnnotationProperty rdf:about="http://purl.org/dc/terms/contributor"/>
    


    <!-- http://purl.org/dc/terms/created -->

    <owl:AnnotationProperty rdf:about="http://purl.org/dc/terms/created"/>
    


    <!-- http://purl.org/dc/terms/creator -->

    <owl:AnnotationProperty rdf:about="http://purl.org/dc/terms/creator">
        <rdfs:subPropertyOf rdf:resource="http://purl.org/dc/terms/created"/>
    </owl:AnnotationProperty>
    


    <!-- http://purl.org/dc/terms/description -->

    <owl:AnnotationProperty rdf:about="http://purl.org/dc/terms/description"/>
    


    <!-- http://purl.org/dc/terms/title -->

    <owl:AnnotationProperty rdf:about="http://purl.org/dc/terms/title">
        <rdfs:subPropertyOf rdf:resource="http://purl.org/dc/terms/description"/>
    </owl:AnnotationProperty>
    


    <!-- http://www.ontologydesignpatterns.org/schemas/cpannotationschema.owl#hasComponent -->

    <owl:AnnotationProperty rdf:about="http://www.ontologydesignpatterns.org/schemas/cpannotationschema.owl#hasComponent"/>
    


    <!-- http://www.ontologydesignpatterns.org/schemas/cpannotationschema.owl#scenarios -->

    <owl:AnnotationProperty rdf:about="http://www.ontologydesignpatterns.org/schemas/cpannotationschema.owl#scenarios"/>
    


    <!-- http://www.semanticweb.org/mein/ontologies/2024/2/untitled-ontology-17#hascomponent -->

    <owl:AnnotationProperty rdf:about="http://www.semanticweb.org/mein/ontologies/2024/2/untitled-ontology-17#hascomponent"/>
    


    <!-- http://www.semanticweb.org/mein/ontologies/2024/2/untitled-ontology-17#userstory -->

    <owl:AnnotationProperty rdf:about="http://www.semanticweb.org/mein/ontologies/2024/2/untitled-ontology-17#userstory"/>
    


    <!-- http://www.semanticweb.org/mein/ontologies/2024/3/untitled-ontology-26#hascomponent -->

    <owl:AnnotationProperty rdf:about="http://www.semanticweb.org/mein/ontologies/2024/3/untitled-ontology-26#hascomponent"/>
    


    <!-- http://www.semanticweb.org/salva/ontologies/2024/1/Anecdotal_fallacy#hascomponent -->

    <owl:AnnotationProperty rdf:about="http://www.semanticweb.org/salva/ontologies/2024/1/Anecdotal_fallacy#hascomponent"/>
    


    <!-- http://www.semanticweb.org/salva/ontologies/2024/1/Anecdotal_fallacy#user_story -->

    <owl:AnnotationProperty rdf:about="http://www.semanticweb.org/salva/ontologies/2024/1/Anecdotal_fallacy#user_story"/>
    


    <!-- https://github.com/corrado877/CognitiveBiasOntologies/RecencyBias#hasComponent -->

    <owl:AnnotationProperty rdf:about="https://github.com/corrado877/CognitiveBiasOntologies/RecencyBias#hasComponent"/>
    


    <!-- https://github.com/corrado877/CognitiveBiasOntologies/RecencyBias#scenarios -->

    <owl:AnnotationProperty rdf:about="https://github.com/corrado877/CognitiveBiasOntologies/RecencyBias#scenarios"/>
    


    <!-- https://github.com/corrado877/CognitiveBiasOntologies/blob/main/Anecdotal_fallacy/hascomponent -->

    <owl:AnnotationProperty rdf:about="https://github.com/corrado877/CognitiveBiasOntologies/blob/main/Anecdotal_fallacy/hascomponent"/>
    


    <!-- https://github.com/corrado877/CognitiveBiasOntologies/blob/main/Anecdotal_fallacy/user_story -->

    <owl:AnnotationProperty rdf:about="https://github.com/corrado877/CognitiveBiasOntologies/blob/main/Anecdotal_fallacy/user_story"/>
    


    <!-- https://github.com/corrado877/CognitiveBiasOntologies/blob/main/Antropomorphism/Anthropomorphism.owl#hasComponent -->

    <owl:AnnotationProperty rdf:about="https://github.com/corrado877/CognitiveBiasOntologies/blob/main/Antropomorphism/Anthropomorphism.owl#hasComponent"/>
    


    <!-- https://github.com/corrado877/CognitiveBiasOntologies/blob/main/Antropomorphism/Anthropomorphism.owl#scenarios -->

    <owl:AnnotationProperty rdf:about="https://github.com/corrado877/CognitiveBiasOntologies/blob/main/Antropomorphism/Anthropomorphism.owl#scenarios"/>
    


    <!-- https://github.com/corrado877/CognitiveBiasOntologies/blob/main/Clustering_illusion#hasComponent -->

    <owl:AnnotationProperty rdf:about="https://github.com/corrado877/CognitiveBiasOntologies/blob/main/Clustering_illusion#hasComponent"/>
    


    <!-- https://github.com/corrado877/CognitiveBiasOntologies/blob/main/Clustering_illusion#user_story -->

    <owl:AnnotationProperty rdf:about="https://github.com/corrado877/CognitiveBiasOntologies/blob/main/Clustering_illusion#user_story"/>
    


    <!-- https://github.com/corrado877/CognitiveBiasOntologies/blob/main/GamblersFallacyOntology/GamblersFallacyOntology.owl#hasComponent -->

    <owl:AnnotationProperty rdf:about="https://github.com/corrado877/CognitiveBiasOntologies/blob/main/GamblersFallacyOntology/GamblersFallacyOntology.owl#hasComponent"/>
    


    <!-- https://github.com/corrado877/CognitiveBiasOntologies/blob/main/Illusion_of_validity/Illusion_of_validity.owl#hasComponent -->

    <owl:AnnotationProperty rdf:about="https://github.com/corrado877/CognitiveBiasOntologies/blob/main/Illusion_of_validity/Illusion_of_validity.owl#hasComponent"/>
    


    <!-- https://github.com/corrado877/CognitiveBiasOntologies/blob/main/Illusion_of_validity/Illusion_of_validity.owl#scenarios -->

    <owl:AnnotationProperty rdf:about="https://github.com/corrado877/CognitiveBiasOntologies/blob/main/Illusion_of_validity/Illusion_of_validity.owl#scenarios"/>
    


    <!-- https://github.com/corrado877/CognitiveBiasOntologies/blob/main/Insensitivity_to_sample_size#hascomponent -->

    <owl:AnnotationProperty rdf:about="https://github.com/corrado877/CognitiveBiasOntologies/blob/main/Insensitivity_to_sample_size#hascomponent"/>
    


    <!-- https://github.com/corrado877/CognitiveBiasOntologies/blob/main/Insensitivity_to_sample_size#user_story -->

    <owl:AnnotationProperty rdf:about="https://github.com/corrado877/CognitiveBiasOntologies/blob/main/Insensitivity_to_sample_size#user_story"/>
    


    <!-- https://github.com/corrado877/CognitiveBiasOntologies/blob/main/Masked_man_fallacy/Masked_Man_Fallacy.owl#Scenarios -->

    <owl:AnnotationProperty rdf:about="https://github.com/corrado877/CognitiveBiasOntologies/blob/main/Masked_man_fallacy/Masked_Man_Fallacy.owl#Scenarios"/>
    


    <!-- https://github.com/corrado877/CognitiveBiasOntologies/blob/main/Neglect_of_probability_bias#hascomponent -->

    <owl:AnnotationProperty rdf:about="https://github.com/corrado877/CognitiveBiasOntologies/blob/main/Neglect_of_probability_bias#hascomponent"/>
    


    <!-- https://github.com/corrado877/CognitiveBiasOntologies/blob/main/Neglect_of_probability_bias#user_story -->

    <owl:AnnotationProperty rdf:about="https://github.com/corrado877/CognitiveBiasOntologies/blob/main/Neglect_of_probability_bias#user_story"/>
    


    <!-- https://github.com/corrado877/CognitiveBiasOntologies/tree/main/Confabulation%20Bias#hascomponent -->

    <owl:AnnotationProperty rdf:about="https://github.com/corrado877/CognitiveBiasOntologies/tree/main/Confabulation%20Bias#hascomponent"/>
    


    <!-- https://github.com/corrado877/CognitiveBiasOntologies/tree/main/Confabulation%20Bias#userstory -->

    <owl:AnnotationProperty rdf:about="https://github.com/corrado877/CognitiveBiasOntologies/tree/main/Confabulation%20Bias#userstory"/>
    


    <!-- https://github.com/corrado877/CognitiveBiasOntologies/tree/main/Naive%20Cynicism#hascomponent -->

    <owl:AnnotationProperty rdf:about="https://github.com/corrado877/CognitiveBiasOntologies/tree/main/Naive%20Cynicism#hascomponent"/>
    


    <!-- https://github.com/corrado877/CognitiveBiasOntologies/tree/main/Naive%20Cynicism#userstory -->

    <owl:AnnotationProperty rdf:about="https://github.com/corrado877/CognitiveBiasOntologies/tree/main/Naive%20Cynicism#userstory"/>
    


    <!-- https://github.com/corrado877/CognitiveBiasOntologies/tree/main/Naive%20Realism#userstory -->

    <owl:AnnotationProperty rdf:about="https://github.com/corrado877/CognitiveBiasOntologies/tree/main/Naive%20Realism#userstory"/>
    


    <!-- 
    ///////////////////////////////////////////////////////////////////////////////////////
    //
    // Datatypes
    //
    ///////////////////////////////////////////////////////////////////////////////////////
     -->

    


    <!-- http://www.w3.org/2001/XMLSchema#string -->

    <rdf:Description rdf:about="http://www.w3.org/2001/XMLSchema#string">
        <terms:description>Define the participation of an entity in a process or an Activity</terms:description>
        <terms:description>Define the relation between an entity (activity or event) and its produced outcome.</terms:description>
    </rdf:Description>
    


    <!-- 
    ///////////////////////////////////////////////////////////////////////////////////////
    //
    // Object Properties
    //
    ///////////////////////////////////////////////////////////////////////////////////////
     -->

    


    <!-- http://descartes-core.org/ontologies/activities/1.0/ActivityPattern.owl#produces -->

    <owl:ObjectProperty rdf:about="http://descartes-core.org/ontologies/activities/1.0/ActivityPattern.owl#produces">
        <rdfs:domain rdf:resource="https://w3id.org/framester/data/framestercore/Predicting"/>
        <rdfs:range rdf:resource="https://w3id.org/framester/data/framestercore/Expectation"/>
        <rdfs:comment>Define the relation between an activity and its produced outcome.</rdfs:comment>
    </owl:ObjectProperty>
    


    <!-- http://modellingdh.github.io/ont/odp/term/inActivity -->

    <owl:ObjectProperty rdf:about="http://modellingdh.github.io/ont/odp/term/inActivity">
        <rdfs:domain>
            <owl:Class>
                <owl:unionOf rdf:parseType="Collection">
                    <rdf:Description rdf:about="https://w3id.org/framester/data/framestercore/Assessing"/>
                    <rdf:Description rdf:about="https://w3id.org/framester/data/framestercore/BecomingAware"/>
                    <rdf:Description rdf:about="https://w3id.org/framester/data/framestercore/Pattern"/>
                    <rdf:Description rdf:about="https://w3id.org/framester/data/framestercore/People"/>
                    <rdf:Description rdf:about="https://w3id.org/framester/data/framestercore/PerceptionExperience"/>
                </owl:unionOf>
            </owl:Class>
        </rdfs:domain>
        <rdfs:range>
            <owl:Class>
                <owl:unionOf rdf:parseType="Collection">
                    <rdf:Description rdf:about="https://github.com/corrado877/CognitiveBiasOntologies/blob/main/CognitiveBiasOntologies#Decision"/>
                    <rdf:Description rdf:about="https://w3id.org/framester/data/framestercore/Activity"/>
                </owl:unionOf>
            </owl:Class>
        </rdfs:range>
        <rdfs:comment>What activity/ies are affecting or affected by a certain engagement</rdfs:comment>
        <rdfs:comment>what activity/ies are affecting or affected by a certain engagement</rdfs:comment>
    </owl:ObjectProperty>
    


    <!-- http://modellingdh.github.io/ont/odp/term/includes -->

    <owl:ObjectProperty rdf:about="http://modellingdh.github.io/ont/odp/term/includes">
        <rdfs:domain>
            <owl:Class>
                <owl:unionOf rdf:parseType="Collection">
                    <rdf:Description rdf:about="https://github.com/corrado877/CognitiveBiasOntologies/blob/main/CognitiveBiasOntologies#Bias"/>
                    <rdf:Description rdf:about="https://github.com/corrado877/CognitiveBiasOntologies/blob/main/CognitiveBiasOntologies#Outcome"/>
                    <rdf:Description rdf:about="https://w3id.org/framester/data/framestercore/Activity"/>
                    <rdf:Description rdf:about="https://w3id.org/framester/data/framestercore/Event"/>
                </owl:unionOf>
            </owl:Class>
        </rdfs:domain>
        <rdfs:range>
            <owl:Class>
                <owl:unionOf rdf:parseType="Collection">
                    <rdf:Description rdf:about="https://github.com/corrado877/CognitiveBiasOntologies/blob/main/CognitiveBiasOntologies#MemoryGap"/>
                    <rdf:Description rdf:about="https://w3id.org/framester/data/framestercore/CognitiveConnection"/>
                    <rdf:Description rdf:about="https://w3id.org/framester/data/framestercore/Evidence"/>
                    <rdf:Description rdf:about="https://w3id.org/framester/data/framestercore/Pattern"/>
                    <rdf:Description rdf:about="https://w3id.org/framester/data/framestercore/PerceptionExperience"/>
                </owl:unionOf>
            </owl:Class>
        </rdfs:range>
        <rdfs:comment>A relation of mereological nature that connects a given observation with the activity that originates them: it strengthens the argument that observations are always active processes from a cognitive standpoint, regardless of how conscious they may be. A standard mereological property from another content pattern may be used in lieu of this one and therefore aligned with it.</rdfs:comment>
    </owl:ObjectProperty>
    


    <!-- http://modellingdh.github.io/ont/odp/term/isEngagedIn -->

    <owl:ObjectProperty rdf:about="http://modellingdh.github.io/ont/odp/term/isEngagedIn">
        <rdfs:domain rdf:resource="https://github.com/corrado877/CognitiveBiasOntologies/blob/main/CognitiveBiasOntologies#Agent"/>
        <rdfs:domain rdf:resource="https://w3id.org/framester/data/framestercore/People"/>
        <rdfs:range>
            <owl:Class>
                <owl:unionOf rdf:parseType="Collection">
                    <rdf:Description rdf:about="http://www.ontology.se/odp/content/owl/Action.owl#Action"/>
                    <rdf:Description rdf:about="http://www.semanticweb.org/mein/ontologies/2024/2/untitled-ontology-17#MentalProperty"/>
                    <rdf:Description rdf:about="https://w3id.org/framester/data/framestercore/Activity"/>
                    <rdf:Description rdf:about="https://w3id.org/framester/data/framestercore/Assessing"/>
                    <rdf:Description rdf:about="https://w3id.org/framester/data/framestercore/BecomingAware"/>
                    <rdf:Description rdf:about="https://w3id.org/framester/data/framestercore/Deciding"/>
                    <rdf:Description rdf:about="https://w3id.org/framester/data/framestercore/Event"/>
                    <rdf:Description rdf:about="https://w3id.org/framester/data/framestercore/PerceptionExperience"/>
                    <rdf:Description rdf:about="https://w3id.org/framester/data/framestercore/Predicting"/>
                </owl:unionOf>
            </owl:Class>
        </rdfs:range>
        <rdfs:comment>Because an activity may engage other participants than the one performing it, engagements are in general considered individual rather than collective, therefore each participants has their own engagement and only some of them will be conscious and/or documented.</rdfs:comment>
        <rdfs:comment>Links the individual to the activity which he’s engaged in.</rdfs:comment>
    </owl:ObjectProperty>
    


    <!-- http://modellingdh.github.io/ont/odp/term/isReflectionOn -->

    <owl:ObjectProperty rdf:about="http://modellingdh.github.io/ont/odp/term/isReflectionOn">
        <rdfs:domain>
            <owl:Class>
                <owl:unionOf rdf:parseType="Collection">
                    <rdf:Description rdf:about="https://github.com/corrado877/CognitiveBiasOntologies/blob/main/CognitiveBiasOntologies#HumanFeature"/>
                    <rdf:Description rdf:about="https://w3id.org/framester/data/framestercore/CognitiveConnection"/>
                    <rdf:Description rdf:about="https://w3id.org/framester/data/framestercore/Pattern"/>
                </owl:unionOf>
            </owl:Class>
        </rdfs:domain>
        <rdfs:range>
            <owl:Class>
                <owl:unionOf rdf:parseType="Collection">
                    <rdf:Description rdf:about="https://w3id.org/framester/data/framestercore/Activity"/>
                    <rdf:Description rdf:about="https://w3id.org/framester/data/framestercore/BecomingAware"/>
                    <rdf:Description rdf:about="https://w3id.org/framester/data/framestercore/PerceptionExperience"/>
                </owl:unionOf>
            </owl:Class>
        </rdfs:range>
        <rdfs:comment>Used to connect the subjective elements of an experience with the corresponding observation, which is extrapolated from the content being interacted with and in itself may not be including a critique.</rdfs:comment>
    </owl:ObjectProperty>
    


    <!-- http://modellingdh.github.io/ont/odp/term/producedObservation -->

    <owl:ObjectProperty rdf:about="http://modellingdh.github.io/ont/odp/term/producedObservation">
        <rdfs:domain>
            <owl:Class>
                <owl:unionOf rdf:parseType="Collection">
                    <rdf:Description rdf:about="https://github.com/corrado877/CognitiveBiasOntologies/blob/main/CognitiveBiasOntologies#AmbiguousStimulus"/>
                    <rdf:Description rdf:about="https://github.com/corrado877/CognitiveBiasOntologies/blob/main/CognitiveBiasOntologies#Non-humanEntity"/>
                    <rdf:Description rdf:about="https://github.com/corrado877/CognitiveBiasOntologies/blob/main/CognitiveBiasOntologies#Variables"/>
                    <rdf:Description rdf:about="https://w3id.org/framester/data/framestercore/ExperiencerObj"/>
                </owl:unionOf>
            </owl:Class>
        </rdfs:domain>
        <rdfs:range>
            <owl:Class>
                <owl:unionOf rdf:parseType="Collection">
                    <rdf:Description rdf:about="https://github.com/corrado877/CognitiveBiasOntologies/blob/main/CognitiveBiasOntologies#HumanFeature"/>
                    <rdf:Description rdf:about="https://w3id.org/framester/data/framestercore/CognitiveConnection"/>
                    <rdf:Description rdf:about="https://w3id.org/framester/data/framestercore/Pattern"/>
                </owl:unionOf>
            </owl:Class>
        </rdfs:range>
        <rdfs:comment>This property can be used to denote that something is (even indirectly, not necessary through direct reflection) responsible for the existence of an observation.</rdfs:comment>
    </owl:ObjectProperty>
    


    <!-- http://ontologydesignpatterns.org/cp/owl/participation.owl#isParticipantIn -->

    <owl:ObjectProperty rdf:about="http://ontologydesignpatterns.org/cp/owl/participation.owl#isParticipantIn">
        <rdfs:domain rdf:resource="https://github.com/corrado877/CognitiveBiasOntologies/blob/main/CognitiveBiasOntologies#PerceivedValidity"/>
        <rdfs:range rdf:resource="https://w3id.org/framester/data/framestercore/Predicting"/>
        <rdfs:comment>Define the participation of an entity in a process.</rdfs:comment>
    </owl:ObjectProperty>
    


    <!-- http://purl.org/ontology/cco/core#belief -->

    <owl:ObjectProperty rdf:about="http://purl.org/ontology/cco/core#belief">
        <rdfs:domain rdf:resource="https://github.com/corrado877/CognitiveBiasOntologies/blob/main/CognitiveBiasOntologies#Agent"/>
        <rdfs:domain rdf:resource="https://w3id.org/framester/data/framestercore/People"/>
        <rdfs:range>
            <owl:Class>
                <owl:unionOf rdf:parseType="Collection">
                    <rdf:Description rdf:about="https://w3id.org/framester/data/framestercore/Sequence"/>
                    <rdf:Description rdf:about="https://w3id.org/framester/data/framestersyn/Belief.n.1"/>
                </owl:unionOf>
            </owl:Class>
        </rdfs:range>
        <rdfs:comment>An uncertain relation for competence representation. That means beliefs, persuasions or opinions, which can also be misconceptions. A Person who believes that a sequence of past events with the same outcome can change the probability of the outcome of the same event in the future</rdfs:comment>
    </owl:ObjectProperty>
    


    <!-- http://semantic.cs.put.poznan.pl/ontologies/newsreportingevent.owl#owns -->

    <owl:ObjectProperty rdf:about="http://semantic.cs.put.poznan.pl/ontologies/newsreportingevent.owl#owns">
        <rdfs:domain rdf:resource="https://w3id.org/framester/data/framestercore/People"/>
        <rdfs:range>
            <owl:Class>
                <owl:unionOf rdf:parseType="Collection">
                    <rdf:Description rdf:about="https://dbpedia.org/resource/Knowledge"/>
                    <rdf:Description rdf:about="https://w3id.org/framester/data/framestercore/Memory"/>
                </owl:unionOf>
            </owl:Class>
        </rdfs:range>
        <rdfs:comment>This property can be used to link a certain NewsProvider with a Media that the NewsProvider ows, e.g. Fox News Channel is owned by Fox Entertainment Group, which also owns other Media (FXX Channel, etc.).
This is an universal property, it can be also used in different context (e.g. Ruslana owns a Persian cat).</rdfs:comment>
        <rdfs:comment>This property can be used to link a certain NewsProvider with a Media that the NewsProvider ows, e.g. Fox News Channel is owned by Fox Entertainment Group, which also owns other Media (FXX Channel, etc.). This is an universal property, it can be also used in different context (e.g. Ruslana owns a Persian cat).</rdfs:comment>
    </owl:ObjectProperty>
    


    <!-- http://semantic.cs.put.poznan.pl/ontologies/newsreportingevent.owl_#owns -->

    <owl:ObjectProperty rdf:about="http://semantic.cs.put.poznan.pl/ontologies/newsreportingevent.owl_#owns">
        <rdfs:domain rdf:resource="https://w3id.org/framester/data/framestercore/People"/>
        <rdfs:range rdf:resource="https://dbpedia.org/resource/Knowledge"/>
        <rdfs:comment>This property can be used to link a certain NewsProvider with a Media that the NewsProvider ows, e.g. Fox News Channel is owned by Fox Entertainment Group, which also owns other Media (FXX Channel, etc.).
This is an universal property, it can be also used in different context (e.g. Ruslana owns a Persian cat).</rdfs:comment>
    </owl:ObjectProperty>
    


    <!-- http://www.fao.org/aims/aos/aos.owl#affects -->

    <owl:ObjectProperty rdf:about="http://www.fao.org/aims/aos/aos.owl#affects">
        <rdfs:domain rdf:resource="https://dbpedia.org/resource/Knowledge"/>
        <rdfs:domain>
            <owl:Class>
                <owl:unionOf rdf:parseType="Collection">
                    <rdf:Description rdf:about="https://dbpedia.org/resource/Knowledge"/>
                    <rdf:Description rdf:about="https://github.com/corrado877/CognitiveBiasOntologies/blob/main/CognitiveBiasOntologies#RecentMemory"/>
                </owl:unionOf>
            </owl:Class>
        </rdfs:domain>
        <rdfs:range rdf:resource="https://github.com/corrado877/CognitiveBiasOntologies/blob/main/CognitiveBiasOntologies#PerceivedValidity"/>
        <rdfs:range>
            <owl:Class>
                <owl:unionOf rdf:parseType="Collection">
                    <rdf:Description rdf:about="https://github.com/corrado877/CognitiveBiasOntologies/blob/main/CognitiveBiasOntologies#PerceivedValidity"/>
                    <rdf:Description rdf:about="https://w3id.org/framester/data/framestercore/Deciding"/>
                    <rdf:Description rdf:about="https://w3id.org/framester/data/framestercore/PerceptionExperience"/>
                </owl:unionOf>
            </owl:Class>
        </rdfs:range>
        <rdfs:comment>X &lt;affects&gt; Y. Agent X acts on object Y in such a way that Y changes state or location.</rdfs:comment>
    </owl:ObjectProperty>
    


    <!-- http://www.ontology.se/odp/content/owl/Action.owl#hasConsequence -->

    <owl:ObjectProperty rdf:about="http://www.ontology.se/odp/content/owl/Action.owl#hasConsequence">
        <rdfs:domain rdf:resource="http://www.ontology.se/odp/content/owl/Action.owl#Action"/>
        <rdfs:range rdf:resource="https://github.com/corrado877/CognitiveBiasOntologies/blob/main/CognitiveBiasOntologies#Outcome"/>
        <rdfs:comment>A causal relation between actions, i.e. one action is the cause of another action. For example, the action of &quot;swimming&quot; is a consequence of &quot;jumping into deep water&quot;. The property is transitive.</rdfs:comment>
    </owl:ObjectProperty>
    


    <!-- http://www.ontologydesignpatterns.org/cp/owl/classification.owl#classifies -->

    <owl:ObjectProperty rdf:about="http://www.ontologydesignpatterns.org/cp/owl/classification.owl#classifies">
        <owl:inverseOf rdf:resource="http://www.ontologydesignpatterns.org/cp/owl/classification.owl#isClassifiedBy"/>
        <rdfs:domain>
            <owl:Class>
                <owl:unionOf rdf:parseType="Collection">
                    <rdf:Description rdf:about="https://github.com/corrado877/CognitiveBiasOntologies/blob/main/CognitiveBiasOntologies#HighImportance"/>
                    <rdf:Description rdf:about="https://github.com/corrado877/CognitiveBiasOntologies/blob/main/CognitiveBiasOntologies#LowImportance"/>
                </owl:unionOf>
            </owl:Class>
        </rdfs:domain>
        <rdfs:range>
            <owl:Class>
                <owl:unionOf rdf:parseType="Collection">
                    <rdf:Description rdf:about="https://github.com/corrado877/CognitiveBiasOntologies/blob/main/CognitiveBiasOntologies#PastMemory"/>
                    <rdf:Description rdf:about="https://github.com/corrado877/CognitiveBiasOntologies/blob/main/CognitiveBiasOntologies#RecentMemory"/>
                </owl:unionOf>
            </owl:Class>
        </rdfs:range>
        <rdfs:comment>A relation between a Concept and an Entity, e.g. the Role &apos;student&apos; classifies a Person &apos;John&apos;.</rdfs:comment>
    </owl:ObjectProperty>
    


    <!-- http://www.ontologydesignpatterns.org/cp/owl/classification.owl#isClassifiedBy -->

    <owl:ObjectProperty rdf:about="http://www.ontologydesignpatterns.org/cp/owl/classification.owl#isClassifiedBy">
        <rdfs:domain>
            <owl:Class>
                <owl:unionOf rdf:parseType="Collection">
                    <rdf:Description rdf:about="https://github.com/corrado877/CognitiveBiasOntologies/blob/main/CognitiveBiasOntologies#PastMemory"/>
                    <rdf:Description rdf:about="https://github.com/corrado877/CognitiveBiasOntologies/blob/main/CognitiveBiasOntologies#RecentMemory"/>
                </owl:unionOf>
            </owl:Class>
        </rdfs:domain>
        <rdfs:range>
            <owl:Class>
                <owl:unionOf rdf:parseType="Collection">
                    <rdf:Description rdf:about="https://github.com/corrado877/CognitiveBiasOntologies/blob/main/CognitiveBiasOntologies#HighImportance"/>
                    <rdf:Description rdf:about="https://github.com/corrado877/CognitiveBiasOntologies/blob/main/CognitiveBiasOntologies#LowImportance"/>
                </owl:unionOf>
            </owl:Class>
        </rdfs:range>
    </owl:ObjectProperty>
    


    <!-- http://www.ontologydesignpatterns.org/cp/owl/parameter.owl#hasParameter -->

    <owl:ObjectProperty rdf:about="http://www.ontologydesignpatterns.org/cp/owl/parameter.owl#hasParameter">
        <owl:inverseOf rdf:resource="http://www.ontologydesignpatterns.org/cp/owl/parameter.owl#isParameterFor"/>
        <rdfs:domain>
            <owl:Class>
                <owl:unionOf rdf:parseType="Collection">
                    <rdf:Description rdf:about="https://github.com/corrado877/CognitiveBiasOntologies/blob/main/CognitiveBiasOntologies#PastMemory"/>
                    <rdf:Description rdf:about="https://github.com/corrado877/CognitiveBiasOntologies/blob/main/CognitiveBiasOntologies#RecentMemory"/>
                    <rdf:Description rdf:about="https://w3id.org/framester/data/framestercore/Event"/>
                </owl:unionOf>
            </owl:Class>
        </rdfs:domain>
        <rdfs:range>
            <owl:Class>
                <owl:unionOf rdf:parseType="Collection">
                    <rdf:Description rdf:about="https://w3id.org/framester/data/framestercore/Importance"/>
                    <rdf:Description rdf:about="https://w3id.org/framester/data/framestercore/Probability"/>
                </owl:unionOf>
            </owl:Class>
        </rdfs:range>
    </owl:ObjectProperty>
    


    <!-- http://www.ontologydesignpatterns.org/cp/owl/parameter.owl#isParameterFor -->

    <owl:ObjectProperty rdf:about="http://www.ontologydesignpatterns.org/cp/owl/parameter.owl#isParameterFor">
        <rdfs:domain>
            <owl:Class>
                <owl:unionOf rdf:parseType="Collection">
                    <rdf:Description rdf:about="https://w3id.org/framester/data/framestercore/Importance"/>
                    <rdf:Description rdf:about="https://w3id.org/framester/data/framestercore/Probability"/>
                </owl:unionOf>
            </owl:Class>
        </rdfs:domain>
        <rdfs:range>
            <owl:Class>
                <owl:unionOf rdf:parseType="Collection">
                    <rdf:Description rdf:about="https://github.com/corrado877/CognitiveBiasOntologies/blob/main/CognitiveBiasOntologies#PastMemory"/>
                    <rdf:Description rdf:about="https://github.com/corrado877/CognitiveBiasOntologies/blob/main/CognitiveBiasOntologies#RecentMemory"/>
                    <rdf:Description rdf:about="https://w3id.org/framester/data/framestercore/Event"/>
                </owl:unionOf>
            </owl:Class>
        </rdfs:range>
    </owl:ObjectProperty>
    


    <!-- http://www.ontologydesignpatterns.org/cp/owl/participation.owl#hasParticipant -->

    <owl:ObjectProperty rdf:about="http://www.ontologydesignpatterns.org/cp/owl/participation.owl#hasParticipant">
        <owl:inverseOf rdf:resource="http://www.ontologydesignpatterns.org/cp/owl/participation.owl#isParticipantIn"/>
        <rdfs:domain>
            <owl:Class>
                <owl:unionOf rdf:parseType="Collection">
                    <rdf:Description rdf:about="https://w3id.org/framester/data/framestercore/Activity"/>
                    <rdf:Description rdf:about="https://w3id.org/framester/data/framestercore/Predicting"/>
                </owl:unionOf>
            </owl:Class>
        </rdfs:domain>
        <rdfs:range>
            <owl:Class>
                <owl:unionOf rdf:parseType="Collection">
                    <rdf:Description rdf:about="https://github.com/corrado877/CognitiveBiasOntologies/blob/main/CognitiveBiasOntologies#PerceivedValidity"/>
                    <rdf:Description rdf:about="https://w3id.org/framester/data/framestercore/People"/>
                </owl:unionOf>
            </owl:Class>
        </rdfs:range>
        <rdfs:comment>inverse property of isParticipantIn</rdfs:comment>
    </owl:ObjectProperty>
    


    <!-- http://www.ontologydesignpatterns.org/cp/owl/participation.owl#isParticipantIn -->

    <owl:ObjectProperty rdf:about="http://www.ontologydesignpatterns.org/cp/owl/participation.owl#isParticipantIn">
        <rdfs:domain>
            <owl:Class>
                <owl:unionOf rdf:parseType="Collection">
                    <rdf:Description rdf:about="https://github.com/corrado877/CognitiveBiasOntologies/blob/main/CognitiveBiasOntologies#PerceivedValidity"/>
                    <rdf:Description rdf:about="https://w3id.org/framester/data/framestercore/People"/>
                </owl:unionOf>
            </owl:Class>
        </rdfs:domain>
        <rdfs:range>
            <owl:Class>
                <owl:unionOf rdf:parseType="Collection">
                    <rdf:Description rdf:about="https://w3id.org/framester/data/framestercore/Activity"/>
                    <rdf:Description rdf:about="https://w3id.org/framester/data/framestercore/Predicting"/>
                </owl:unionOf>
            </owl:Class>
        </rdfs:range>
        <rdfs:comment>Define the participation of an entity in a process or an Activity</rdfs:comment>
    </owl:ObjectProperty>
    


    <!-- http://www.ontologydesignpatterns.org/cp/owl/partof.owl#hasPart -->

    <owl:ObjectProperty rdf:about="http://www.ontologydesignpatterns.org/cp/owl/partof.owl#hasPart">
        <owl:inverseOf rdf:resource="http://www.ontologydesignpatterns.org/cp/owl/partof.owl#isPartOf"/>
        <rdfs:domain>
            <owl:Class>
                <owl:unionOf rdf:parseType="Collection">
                    <rdf:Description rdf:about="https://w3id.org/framester/data/framestercore/Activity"/>
                    <rdf:Description rdf:about="https://w3id.org/framester/data/framestercore/Pattern"/>
                </owl:unionOf>
            </owl:Class>
        </rdfs:domain>
        <rdfs:range>
            <owl:Class>
                <owl:unionOf rdf:parseType="Collection">
                    <rdf:Description rdf:about="https://github.com/corrado877/CognitiveBiasOntologies/blob/main/CognitiveBiasOntologies#Variables"/>
                    <rdf:Description rdf:about="https://w3id.org/framester/data/framestercore/Event"/>
                </owl:unionOf>
            </owl:Class>
        </rdfs:range>
    </owl:ObjectProperty>
    


    <!-- http://www.ontologydesignpatterns.org/cp/owl/partof.owl#isPartOf -->

    <owl:ObjectProperty rdf:about="http://www.ontologydesignpatterns.org/cp/owl/partof.owl#isPartOf">
        <rdfs:domain>
            <owl:Class>
                <owl:unionOf rdf:parseType="Collection">
                    <rdf:Description rdf:about="https://github.com/corrado877/CognitiveBiasOntologies/blob/main/CognitiveBiasOntologies#Variables"/>
                    <rdf:Description rdf:about="https://w3id.org/framester/data/framestercore/Event"/>
                </owl:unionOf>
            </owl:Class>
        </rdfs:domain>
        <rdfs:range>
            <owl:Class>
                <owl:unionOf rdf:parseType="Collection">
                    <rdf:Description rdf:about="https://w3id.org/framester/data/framestercore/Activity"/>
                    <rdf:Description rdf:about="https://w3id.org/framester/data/framestercore/Pattern"/>
                </owl:unionOf>
            </owl:Class>
        </rdfs:range>
    </owl:ObjectProperty>
    


    <!-- http://www.ontologydesignpatterns.org/cp/owl/sequence.owl#follows -->

    <owl:ObjectProperty rdf:about="http://www.ontologydesignpatterns.org/cp/owl/sequence.owl#follows">
        <owl:inverseOf rdf:resource="http://www.ontologydesignpatterns.org/cp/owl/sequence.owl#precedes"/>
        <rdfs:domain rdf:resource="https://github.com/corrado877/CognitiveBiasOntologies/blob/main/CognitiveBiasOntologies#RecentMemory"/>
        <rdfs:range rdf:resource="https://github.com/corrado877/CognitiveBiasOntologies/blob/main/CognitiveBiasOntologies#PastMemory"/>
        <rdfs:comment>A relation between entities, expressing a &apos;sequence&apos; schema.</rdfs:comment>
    </owl:ObjectProperty>
    


    <!-- http://www.ontologydesignpatterns.org/cp/owl/sequence.owl#precedes -->

    <owl:ObjectProperty rdf:about="http://www.ontologydesignpatterns.org/cp/owl/sequence.owl#precedes">
        <rdfs:domain rdf:resource="https://github.com/corrado877/CognitiveBiasOntologies/blob/main/CognitiveBiasOntologies#PastMemory"/>
        <rdfs:range rdf:resource="https://github.com/corrado877/CognitiveBiasOntologies/blob/main/CognitiveBiasOntologies#RecentMemory"/>
        <rdfs:comment>A relation between entities, expressing a &apos;sequence&apos; schema.
E.g. &apos;year 1999 precedes 2000&apos;, &apos;deciding what coffee to use&apos; precedes &apos;preparing coffee&apos;, &apos;World War II follows World War I&apos;, &apos;in the Milan to Rome autoroute, Bologna precedes Florence&apos;, etc.

It can then be used between tasks, processes, time intervals, spatially locate objects, situations, etc.</rdfs:comment>
    </owl:ObjectProperty>
    


    <!-- http://www.w3.org/2000/01/rdf-schema#hasType -->

    <owl:ObjectProperty rdf:about="http://www.w3.org/2000/01/rdf-schema#hasType">
        <rdfs:domain rdf:resource="https://w3id.org/framester/data/framestercore/Evidence"/>
        <rdfs:range>
            <owl:Restriction>
                <owl:onProperty rdf:resource="https://github.com/corrado877/CognitiveBiasOntologies/tree/main/Confabulation%20Bias#Fictional"/>
                <owl:someValuesFrom rdf:resource="http://www.w3.org/2001/XMLSchema#string"/>
            </owl:Restriction>
        </rdfs:range>
    </owl:ObjectProperty>
    


    <!-- http://www.w3.org/ns/prov#wasGeneratedBy -->

    <owl:ObjectProperty rdf:about="http://www.w3.org/ns/prov#wasGeneratedBy">
        <rdfs:domain rdf:resource="https://w3id.org/framester/data/framestercore/Sequence"/>
        <rdfs:range rdf:resource="https://w3id.org/framester/data/framestercore/Activity"/>
    </owl:ObjectProperty>
    


    <!-- https://dbpedia.org/ontology/produces -->

    <owl:ObjectProperty rdf:about="https://dbpedia.org/ontology/produces">
        <rdfs:domain>
            <owl:Class>
                <owl:unionOf rdf:parseType="Collection">
                    <rdf:Description rdf:about="https://github.com/corrado877/CognitiveBiasOntologies/blob/main/CognitiveBiasOntologies#MemoryEncoding"/>
                    <rdf:Description rdf:about="https://w3id.org/framester/data/framestercore/Deciding"/>
                    <rdf:Description rdf:about="https://w3id.org/framester/data/framestercore/Event"/>
                    <rdf:Description rdf:about="https://w3id.org/framester/data/framestercore/People"/>
                    <rdf:Description rdf:about="https://w3id.org/framester/data/framestercore/PerceptionExperience"/>
                    <rdf:Description rdf:about="https://w3id.org/framester/data/framestercore/Predicting"/>
                </owl:unionOf>
            </owl:Class>
        </rdfs:domain>
        <rdfs:range>
            <owl:Class>
                <owl:unionOf rdf:parseType="Collection">
                    <rdf:Description rdf:about="https://github.com/corrado877/CognitiveBiasOntologies/blob/main/CognitiveBiasOntologies#Decision"/>
                    <rdf:Description rdf:about="https://github.com/corrado877/CognitiveBiasOntologies/blob/main/CognitiveBiasOntologies#Outcome"/>
                    <rdf:Description rdf:about="https://github.com/corrado877/CognitiveBiasOntologies/blob/main/CognitiveBiasOntologies#PerceivedValidity"/>
                    <rdf:Description rdf:about="https://w3id.org/framester/data/framestercore/Evidence"/>
                    <rdf:Description rdf:about="https://w3id.org/framester/data/framestercore/Expectation"/>
                    <rdf:Description rdf:about="https://w3id.org/framester/data/framestercore/Memory"/>
                </owl:unionOf>
            </owl:Class>
        </rdfs:range>
        <rdfs:comment>Define the relation between an activity and its produced outcome.</rdfs:comment>
        <rdfs:comment>Define the relation between an entity (activity or event) and its produced outcome.</rdfs:comment>
    </owl:ObjectProperty>
    


    <!-- https://github.com/corrado877/CognitiveBiasOntologies/blob/main/CognitiveBiasOntologies#creates -->

    <owl:ObjectProperty rdf:about="https://github.com/corrado877/CognitiveBiasOntologies/blob/main/CognitiveBiasOntologies#creates">
        <rdfs:domain>
            <owl:Class>
                <owl:unionOf rdf:parseType="Collection">
                    <rdf:Description rdf:about="https://w3id.org/framester/data/framestercore/Activity"/>
                    <rdf:Description rdf:about="https://w3id.org/framester/data/framestercore/Sequence"/>
                </owl:unionOf>
            </owl:Class>
        </rdfs:domain>
        <rdfs:range>
            <owl:Class>
                <owl:unionOf rdf:parseType="Collection">
                    <rdf:Description rdf:about="https://dbpedia.org/page/Illusion"/>
                    <rdf:Description rdf:about="https://w3id.org/framester/data/framestercore/PerceptionExperience"/>
                </owl:unionOf>
            </owl:Class>
        </rdfs:range>
        <rdfs:comment>a property connecting the illusory effect created by the Perception of Pattern</rdfs:comment>
    </owl:ObjectProperty>
    


    <!-- https://github.com/corrado877/CognitiveBiasOntologies/blob/main/CognitiveBiasOntologies#decide -->

    <owl:ObjectProperty rdf:about="https://github.com/corrado877/CognitiveBiasOntologies/blob/main/CognitiveBiasOntologies#decide">
        <rdfs:domain rdf:resource="https://github.com/corrado877/CognitiveBiasOntologies/blob/main/CognitiveBiasOntologies#Thing"/>
        <rdfs:range rdf:resource="https://github.com/corrado877/CognitiveBiasOntologies/blob/main/Neglect_of_probability_bias#Ignore"/>
        <rdfs:comment>a property that links the cognitive process of deciding how to act after receiving information.</rdfs:comment>
    </owl:ObjectProperty>
    


    <!-- https://github.com/corrado877/CognitiveBiasOntologies/blob/main/CognitiveBiasOntologies#fillsMemoryGap -->

    <owl:ObjectProperty rdf:about="https://github.com/corrado877/CognitiveBiasOntologies/blob/main/CognitiveBiasOntologies#fillsMemoryGap">
        <rdfs:domain rdf:resource="https://w3id.org/framester/data/framestercore/Evidence"/>
        <rdfs:range rdf:resource="https://github.com/corrado877/CognitiveBiasOntologies/blob/main/CognitiveBiasOntologies#MemoryGap"/>
        <rdfs:comment>represents the action or process of replenishing or restoring missing or incomplete memory or information within an entity or system.</rdfs:comment>
    </owl:ObjectProperty>
    


    <!-- https://github.com/corrado877/CognitiveBiasOntologies/blob/main/CognitiveBiasOntologies#focusesOn -->

    <owl:ObjectProperty rdf:about="https://github.com/corrado877/CognitiveBiasOntologies/blob/main/CognitiveBiasOntologies#focusesOn">
        <rdfs:domain rdf:resource="https://github.com/corrado877/CognitiveBiasOntologies/blob/main/CognitiveBiasOntologies#Agent"/>
        <rdfs:range rdf:resource="https://github.com/corrado877/CognitiveBiasOntologies/blob/main/CognitiveBiasOntologies#Bias"/>
        <rdfs:comment>describes the primary subject or area of attention associated with an entity or concept.</rdfs:comment>
    </owl:ObjectProperty>
    


    <!-- https://github.com/corrado877/CognitiveBiasOntologies/blob/main/CognitiveBiasOntologies#hasAttribute -->

    <owl:ObjectProperty rdf:about="https://github.com/corrado877/CognitiveBiasOntologies/blob/main/CognitiveBiasOntologies#hasAttribute">
        <rdfs:domain>
            <owl:Class>
                <owl:unionOf rdf:parseType="Collection">
                    <rdf:Description rdf:about="https://github.com/corrado877/CognitiveBiasOntologies/blob/main/CognitiveBiasOntologies#Outcome"/>
                    <rdf:Description rdf:about="https://w3id.org/framester/data/framestercore/Expectation"/>
                </owl:unionOf>
            </owl:Class>
        </rdfs:domain>
        <rdfs:range rdf:resource="https://w3id.org/framester/data/framestercore/Identicality"/>
        <rdfs:comment>Connects an object to one of its attributes.</rdfs:comment>
    </owl:ObjectProperty>
    


    <!-- https://github.com/corrado877/CognitiveBiasOntologies/blob/main/CognitiveBiasOntologies#hasBias -->

    <owl:ObjectProperty rdf:about="https://github.com/corrado877/CognitiveBiasOntologies/blob/main/CognitiveBiasOntologies#hasBias">
        <rdfs:domain rdf:resource="https://github.com/corrado877/CognitiveBiasOntologies/blob/main/CognitiveBiasOntologies#Agent"/>
        <rdfs:range rdf:resource="https://github.com/corrado877/CognitiveBiasOntologies/blob/main/CognitiveBiasOntologies#Bias"/>
        <rdfs:comment>Indicates an individual possesses Naive Realism Bias</rdfs:comment>
    </owl:ObjectProperty>
    


    <!-- https://github.com/corrado877/CognitiveBiasOntologies/blob/main/CognitiveBiasOntologies#hasBiasedOpinion -->

    <owl:ObjectProperty rdf:about="https://github.com/corrado877/CognitiveBiasOntologies/blob/main/CognitiveBiasOntologies#hasBiasedOpinion">
        <rdfs:domain rdf:resource="https://w3id.org/framester/data/framestercore/People"/>
        <rdfs:range>
            <owl:Class>
                <owl:unionOf rdf:parseType="Collection">
                    <rdf:Description rdf:about="https://github.com/corrado877/CognitiveBiasOntologies/blob/main/CognitiveBiasOntologies#Bias"/>
                    <rdf:Description rdf:about="https://w3id.org/framester/data/framestercore/Event"/>
                </owl:unionOf>
            </owl:Class>
        </rdfs:range>
        <rdfs:comment>A property connecting a Person who has a biased opinion about the possible outcome of a Future Event, such as a Random/Chance-based Occurrence, because he/she thinks that there is a correlation between this future event and a series of past events.</rdfs:comment>
        <rdfs:comment>a property connecting a Person who has a biased opinion about something eg the possible outcome of an Event such as a Random or Chance-based Occurrence  or a person who has a biased Opinion about a Bias.</rdfs:comment>
    </owl:ObjectProperty>
    


    <!-- https://github.com/corrado877/CognitiveBiasOntologies/blob/main/CognitiveBiasOntologies#hasEffect -->

    <owl:ObjectProperty rdf:about="https://github.com/corrado877/CognitiveBiasOntologies/blob/main/CognitiveBiasOntologies#hasEffect">
        <rdfs:domain>
            <owl:Class>
                <owl:unionOf rdf:parseType="Collection">
                    <rdf:Description rdf:about="https://w3id.org/framester/data/framestercore/CognitiveConnection"/>
                    <rdf:Description rdf:about="https://w3id.org/framester/data/framestercore/Pattern"/>
                </owl:unionOf>
            </owl:Class>
        </rdfs:domain>
        <rdfs:range rdf:resource="https://dbpedia.org/page/Illusion"/>
        <rdfs:comment>A property linking an Entity (a perceived correlation between two variables in a pattern or a perceived pattern due to any kind of external stimulus) and the illusory effect that this Entity produce.</rdfs:comment>
        <rdfs:comment>hasEffect: a property linking an Entity (a perceived correlation between two variables in a pattern or a perceived pattern due to any kind of external stimulus) and the illusory effect that this Entity produce.</rdfs:comment>
    </owl:ObjectProperty>
    


    <!-- https://github.com/corrado877/CognitiveBiasOntologies/blob/main/CognitiveBiasOntologies#hasFeature -->

    <owl:ObjectProperty rdf:about="https://github.com/corrado877/CognitiveBiasOntologies/blob/main/CognitiveBiasOntologies#hasFeature">
        <rdfs:domain rdf:resource="https://dbpedia.org/resource/Entity"/>
        <rdfs:range rdf:resource="https://github.com/corrado877/CognitiveBiasOntologies/blob/main/CognitiveBiasOntologies#Feature"/>
        <rdfs:comment>Connects an entity to its relative feature or intention.</rdfs:comment>
    </owl:ObjectProperty>
    


    <!-- https://github.com/corrado877/CognitiveBiasOntologies/blob/main/CognitiveBiasOntologies#hasInfluence -->

    <owl:ObjectProperty rdf:about="https://github.com/corrado877/CognitiveBiasOntologies/blob/main/CognitiveBiasOntologies#hasInfluence">
        <owl:inverseOf rdf:resource="https://w3id.org/affectedBy#influencedBy"/>
        <rdfs:domain>
            <owl:Class>
                <owl:unionOf rdf:parseType="Collection">
                    <rdf:Description rdf:about="https://github.com/corrado877/CognitiveBiasOntologies/blob/main/CognitiveBiasOntologies#Decision"/>
                    <rdf:Description rdf:about="https://github.com/corrado877/CognitiveBiasOntologies/blob/main/Neglect_of_probability_bias#Ignore"/>
                    <rdf:Description rdf:about="https://w3id.org/framester/data/framestercore/Pattern"/>
                    <rdf:Description rdf:about="https://w3id.org/framester/data/framestercore/Sequence"/>
                </owl:unionOf>
            </owl:Class>
        </rdfs:domain>
        <rdfs:range>
            <owl:Class>
                <owl:unionOf rdf:parseType="Collection">
                    <rdf:Description rdf:about="https://github.com/corrado877/CognitiveBiasOntologies/blob/main/CognitiveBiasOntologies#Decision"/>
                    <rdf:Description rdf:about="https://github.com/corrado877/CognitiveBiasOntologies/blob/main/CognitiveBiasOntologies#Thing"/>
                    <rdf:Description rdf:about="https://w3id.org/framester/data/framestercore/PerceptionExperience"/>
                    <rdf:Description rdf:about="https://w3id.org/framester/data/framestercore/Probability"/>
                </owl:unionOf>
            </owl:Class>
        </rdfs:range>
        <rdfs:comment>A property connecting an Entity (Pattern) that affects in different ways another entity (PerceptionExperience).</rdfs:comment>
        <rdfs:comment>A property connecting an Entity (Sequence) that affects in different ways another entity (Probability).</rdfs:comment>
    </owl:ObjectProperty>
    


    <!-- https://github.com/corrado877/CognitiveBiasOntologies/blob/main/CognitiveBiasOntologies#hasMemoryGap -->

    <owl:ObjectProperty rdf:about="https://github.com/corrado877/CognitiveBiasOntologies/blob/main/CognitiveBiasOntologies#hasMemoryGap">
        <rdfs:domain rdf:resource="https://w3id.org/framester/data/framestercore/People"/>
        <rdfs:range rdf:resource="https://github.com/corrado877/CognitiveBiasOntologies/blob/main/CognitiveBiasOntologies#MemoryGap"/>
        <rdfs:comment>signifies a period or instance where an entity lacks recall or memory of specific information or events.</rdfs:comment>
    </owl:ObjectProperty>
    


    <!-- https://github.com/corrado877/CognitiveBiasOntologies/blob/main/CognitiveBiasOntologies#hasOutcome -->

    <owl:ObjectProperty rdf:about="https://github.com/corrado877/CognitiveBiasOntologies/blob/main/CognitiveBiasOntologies#hasOutcome">
        <owl:inverseOf rdf:resource="https://github.com/corrado877/CognitiveBiasOntologies/blob/main/CognitiveBiasOntologies#isOutcomeOf"/>
        <rdfs:domain>
            <owl:Class>
                <owl:unionOf rdf:parseType="Collection">
                    <rdf:Description rdf:about="http://www.semanticweb.org/mein/ontologies/2024/2/untitled-ontology-17#MentalProperty"/>
                    <rdf:Description rdf:about="https://github.com/corrado877/CognitiveBiasOntologies/blob/main/CognitiveBiasOntologies#MemoryEncoding"/>
                    <rdf:Description rdf:about="https://w3id.org/framester/data/framestercore/Event"/>
                    <rdf:Description rdf:about="https://w3id.org/framester/data/framestercore/Sequence"/>
                </owl:unionOf>
            </owl:Class>
        </rdfs:domain>
        <rdfs:range>
            <owl:Class>
                <owl:unionOf rdf:parseType="Collection">
                    <rdf:Description rdf:about="https://github.com/corrado877/CognitiveBiasOntologies/blob/main/CognitiveBiasOntologies#Outcome"/>
                    <rdf:Description rdf:about="https://w3id.org/framester/data/framestercore/Importance"/>
                </owl:unionOf>
            </owl:Class>
        </rdfs:range>
        <rdfs:comment>A property linking an entity that produces an Outcome</rdfs:comment>
        <rdfs:comment>A property linking an entity that produces an Outcome.</rdfs:comment>
        <rdfs:comment>A property linking series of events to the same Outcome produced</rdfs:comment>
        <rdfs:comment>The final decision the individual reaches as ending result of the decision-making process.</rdfs:comment>
    </owl:ObjectProperty>
    


    <!-- https://github.com/corrado877/CognitiveBiasOntologies/blob/main/CognitiveBiasOntologies#hasOutcomeEffect -->

    <owl:ObjectProperty rdf:about="https://github.com/corrado877/CognitiveBiasOntologies/blob/main/CognitiveBiasOntologies#hasOutcomeEffect">
        <owl:inverseOf rdf:resource="https://github.com/corrado877/CognitiveBiasOntologies/blob/main/CognitiveBiasOntologies#isOutcomeEffectOf"/>
        <rdfs:domain rdf:resource="https://w3id.org/framester/data/framestercore/Sequence"/>
        <rdfs:range rdf:resource="https://dbpedia.org/page/Success"/>
        <rdfs:comment>A property linking a series of events which Outcome brings to the same effect</rdfs:comment>
    </owl:ObjectProperty>
    


    <!-- https://github.com/corrado877/CognitiveBiasOntologies/blob/main/CognitiveBiasOntologies#hasPerspective -->

    <owl:ObjectProperty rdf:about="https://github.com/corrado877/CognitiveBiasOntologies/blob/main/CognitiveBiasOntologies#hasPerspective">
        <rdfs:domain rdf:resource="https://w3id.org/framester/data/framestercore/People"/>
        <rdfs:range rdf:resource="https://w3id.org/framester/data/framestercore/Statement"/>
        <rdfs:comment>this property connect a perspective that a person or a group of Persons has about an aspect of the real world.</rdfs:comment>
    </owl:ObjectProperty>
    


    <!-- https://github.com/corrado877/CognitiveBiasOntologies/blob/main/CognitiveBiasOntologies#have_knowledge -->

    <owl:ObjectProperty rdf:about="https://github.com/corrado877/CognitiveBiasOntologies/blob/main/CognitiveBiasOntologies#have_knowledge">
        <rdfs:domain rdf:resource="https://w3id.org/framester/data/framestercore/People"/>
        <rdfs:range rdf:resource="https://github.com/corrado877/CognitiveBiasOntologies/blob/main/CognitiveBiasOntologies#Thing"/>
        <rdfs:comment>a property that links the cognitive process of storing some information regarding a topic.</rdfs:comment>
    </owl:ObjectProperty>
    


    <!-- https://github.com/corrado877/CognitiveBiasOntologies/blob/main/CognitiveBiasOntologies#ignores -->

    <owl:ObjectProperty rdf:about="https://github.com/corrado877/CognitiveBiasOntologies/blob/main/CognitiveBiasOntologies#ignores">
        <rdfs:domain rdf:resource="https://github.com/corrado877/CognitiveBiasOntologies/blob/main/CognitiveBiasOntologies#Agent"/>
        <rdfs:range rdf:resource="https://w3id.org/framester/data/framestercore/Statement"/>
        <rdfs:comment>denotes the deliberate disregard or lack of attention to a particular entity, concept, or information by another entity.</rdfs:comment>
    </owl:ObjectProperty>
    


    <!-- https://github.com/corrado877/CognitiveBiasOntologies/blob/main/CognitiveBiasOntologies#involves -->

    <owl:ObjectProperty rdf:about="https://github.com/corrado877/CognitiveBiasOntologies/blob/main/CognitiveBiasOntologies#involves">
        <rdfs:domain>
            <owl:Class>
                <owl:unionOf rdf:parseType="Collection">
                    <rdf:Description rdf:about="https://dbpedia.org/page/Illusion"/>
                    <rdf:Description rdf:about="https://w3id.org/framester/data/framestercore/Activity"/>
                    <rdf:Description rdf:about="https://w3id.org/framester/data/framestercore/Event"/>
                    <rdf:Description rdf:about="https://w3id.org/framester/data/framestercore/PerceptionExperience"/>
                </owl:unionOf>
            </owl:Class>
        </rdfs:domain>
        <rdfs:range>
            <owl:Class>
                <owl:unionOf rdf:parseType="Collection">
                    <rdf:Description rdf:about="https://dbpedia.org/resource/Entity"/>
                    <rdf:Description rdf:about="https://github.com/corrado877/CognitiveBiasOntologies/blob/main/CognitiveBiasOntologies#AmbiguousStimulus"/>
                    <rdf:Description rdf:about="https://github.com/corrado877/CognitiveBiasOntologies/blob/main/CognitiveBiasOntologies#MemoryEncoding"/>
                    <rdf:Description rdf:about="https://w3id.org/framester/data/framestercore/Assistance"/>
                    <rdf:Description rdf:about="https://w3id.org/framester/data/framestercore/ExperiencerObj"/>
                </owl:unionOf>
            </owl:Class>
        </rdfs:range>
        <rdfs:comment>Connects entites such as an activity to other entities involved in it</rdfs:comment>
        <rdfs:comment>a property connecting an entity such as Activity to any kind of thing that is involved during the execution of that Activity.</rdfs:comment>
        <rdfs:comment>a property connecting an entity to any kind of thing that is related to that Entity</rdfs:comment>
        <rdfs:comment>a property that links the cognitive process of creating the perception of an experience and the experience to which it is linked to.</rdfs:comment>
        <rdfs:comment>connects an activity to the entities involved in it.</rdfs:comment>
    </owl:ObjectProperty>
    


    <!-- https://github.com/corrado877/CognitiveBiasOntologies/blob/main/CognitiveBiasOntologies#isBiasedBy -->

    <owl:ObjectProperty rdf:about="https://github.com/corrado877/CognitiveBiasOntologies/blob/main/CognitiveBiasOntologies#isBiasedBy">
        <rdfs:domain rdf:resource="https://w3id.org/framester/data/framestercore/People"/>
        <rdfs:range rdf:resource="https://w3id.org/framester/data/framestercore/Pattern"/>
        <rdfs:comment>a property that connect a Person that is biased by the idea of seeing a Pattern such as meaningful shapes made by a visual stimulus</rdfs:comment>
    </owl:ObjectProperty>
    


    <!-- https://github.com/corrado877/CognitiveBiasOntologies/blob/main/CognitiveBiasOntologies#isOutcomeEffectOf -->

    <owl:ObjectProperty rdf:about="https://github.com/corrado877/CognitiveBiasOntologies/blob/main/CognitiveBiasOntologies#isOutcomeEffectOf">
        <rdfs:domain rdf:resource="https://dbpedia.org/page/Success"/>
        <rdfs:range rdf:resource="https://w3id.org/framester/data/framestercore/Sequence"/>
        <rdfs:comment>inverse property of HasOutcomeEffect</rdfs:comment>
    </owl:ObjectProperty>
    


    <!-- https://github.com/corrado877/CognitiveBiasOntologies/blob/main/CognitiveBiasOntologies#isOutcomeOf -->

    <owl:ObjectProperty rdf:about="https://github.com/corrado877/CognitiveBiasOntologies/blob/main/CognitiveBiasOntologies#isOutcomeOf">
        <rdfs:domain>
            <owl:Class>
                <owl:unionOf rdf:parseType="Collection">
                    <rdf:Description rdf:about="https://github.com/corrado877/CognitiveBiasOntologies/blob/main/CognitiveBiasOntologies#Outcome"/>
                    <rdf:Description rdf:about="https://w3id.org/framester/data/framestercore/Importance"/>
                </owl:unionOf>
            </owl:Class>
        </rdfs:domain>
        <rdfs:range>
            <owl:Class>
                <owl:unionOf rdf:parseType="Collection">
                    <rdf:Description rdf:about="https://github.com/corrado877/CognitiveBiasOntologies/blob/main/CognitiveBiasOntologies#MemoryEncoding"/>
                    <rdf:Description rdf:about="https://w3id.org/framester/data/framestercore/Event"/>
                    <rdf:Description rdf:about="https://w3id.org/framester/data/framestercore/Sequence"/>
                </owl:unionOf>
            </owl:Class>
        </rdfs:range>
        <rdfs:comment>Inverse property of HasOutcome property</rdfs:comment>
    </owl:ObjectProperty>
    


    <!-- https://github.com/corrado877/CognitiveBiasOntologies/blob/main/CognitiveBiasOntologies#isPerceivedAs -->

    <owl:ObjectProperty rdf:about="https://github.com/corrado877/CognitiveBiasOntologies/blob/main/CognitiveBiasOntologies#isPerceivedAs">
        <rdfs:domain>
            <owl:Class>
                <owl:unionOf rdf:parseType="Collection">
                    <rdf:Description rdf:about="https://w3id.org/framester/data/framestercore/Assistance"/>
                    <rdf:Description rdf:about="https://w3id.org/framester/data/framestercore/BecomingAware"/>
                    <rdf:Description rdf:about="https://w3id.org/framester/data/framestersyn/Belief.n.1"/>
                </owl:unionOf>
            </owl:Class>
        </rdfs:domain>
        <rdfs:range rdf:resource="https://w3id.org/framester/data/framestercore/Pattern"/>
        <rdfs:comment>a property that links a person &apos;s cognitive process of being aware of something like a trend while he/she is doing an activity and what is perceived as part of the trend.</rdfs:comment>
        <rdfs:comment>a property that links the cognitive process of perceiving something in a specific way.</rdfs:comment>
        <rdfs:comment>a property that links the cognitive process of perceiving something in a specific way. E.g. a person being aware of a trend in an activity that is perceived as a pattern in that activity. E.g. an assistance process being perceived as Malicious.</rdfs:comment>
    </owl:ObjectProperty>
    


    <!-- https://github.com/corrado877/CognitiveBiasOntologies/blob/main/CognitiveBiasOntologies#isProducedEffectBy -->

    <owl:ObjectProperty rdf:about="https://github.com/corrado877/CognitiveBiasOntologies/blob/main/CognitiveBiasOntologies#isProducedEffectBy">
        <owl:inverseOf rdf:resource="https://github.com/corrado877/CognitiveBiasOntologies/blob/main/CognitiveBiasOntologies#producesOutcomeEffect"/>
        <rdfs:domain rdf:resource="https://dbpedia.org/page/Success"/>
        <rdfs:range rdf:resource="https://w3id.org/framester/data/framestercore/Event"/>
        <rdfs:comment>inverse property of producesOutcomeEffect</rdfs:comment>
    </owl:ObjectProperty>
    


    <!-- https://github.com/corrado877/CognitiveBiasOntologies/blob/main/CognitiveBiasOntologies#isUnawareOf -->

    <owl:ObjectProperty rdf:about="https://github.com/corrado877/CognitiveBiasOntologies/blob/main/CognitiveBiasOntologies#isUnawareOf">
        <rdfs:domain rdf:resource="https://github.com/corrado877/CognitiveBiasOntologies/blob/main/CognitiveBiasOntologies#Agent"/>
        <rdfs:range rdf:resource="https://w3id.org/framester/data/framestersyn/Belief.n.1"/>
        <rdfs:comment>indicates the lack of knowledge or awareness of a particular entity or concept by another entity.</rdfs:comment>
    </owl:ObjectProperty>
    


    <!-- https://github.com/corrado877/CognitiveBiasOntologies/blob/main/CognitiveBiasOntologies#producesOutcomeEffect -->

    <owl:ObjectProperty rdf:about="https://github.com/corrado877/CognitiveBiasOntologies/blob/main/CognitiveBiasOntologies#producesOutcomeEffect">
        <rdfs:domain rdf:resource="https://w3id.org/framester/data/framestercore/Event"/>
        <rdfs:range rdf:resource="https://dbpedia.org/page/Success"/>
        <rdfs:comment>a property linking an event which Outcome will produce an effect</rdfs:comment>
    </owl:ObjectProperty>
    


    <!-- https://github.com/corrado877/CognitiveBiasOntologies/blob/main/CognitiveBiasOntologies#rejects -->

    <owl:ObjectProperty rdf:about="https://github.com/corrado877/CognitiveBiasOntologies/blob/main/CognitiveBiasOntologies#rejects">
        <rdfs:domain rdf:resource="https://github.com/corrado877/CognitiveBiasOntologies/blob/main/CognitiveBiasOntologies#PerceivedValidity"/>
        <rdfs:range rdf:resource="https://github.com/corrado877/CognitiveBiasOntologies/blob/main/CognitiveBiasOntologies#Un-knownFeature"/>
        <rdfs:comment>The act of denying a particular intention in favour of one or more others.</rdfs:comment>
    </owl:ObjectProperty>
    


    <!-- https://github.com/corrado877/CognitiveBiasOntologies/blob/main/CognitiveBiasOntologies#supports -->

    <owl:ObjectProperty rdf:about="https://github.com/corrado877/CognitiveBiasOntologies/blob/main/CognitiveBiasOntologies#supports">
        <rdfs:domain rdf:resource="https://github.com/corrado877/CognitiveBiasOntologies/blob/main/CognitiveBiasOntologies#PerceivedValidity"/>
        <rdfs:range rdf:resource="https://github.com/corrado877/CognitiveBiasOntologies/blob/main/CognitiveBiasOntologies#KnownFeature"/>
        <rdfs:comment>The act of confirming a particular intention at the expense of one or more others.</rdfs:comment>
    </owl:ObjectProperty>
    


    <!-- https://github.com/corrado877/CognitiveBiasOntologies/tree/main/Naive_Cynicism#misjudges -->

    <owl:ObjectProperty rdf:about="https://github.com/corrado877/CognitiveBiasOntologies/tree/main/Naive_Cynicism#misjudges">
        <rdfs:domain rdf:resource="https://github.com/corrado877/CognitiveBiasOntologies/blob/main/CognitiveBiasOntologies#Bias"/>
        <rdfs:range rdf:resource="https://w3id.org/framester/data/framestercore/Assistance"/>
        <rdfs:comment>a property that links the cognitive process of misinterpreting information</rdfs:comment>
    </owl:ObjectProperty>
    


    <!-- https://github.com/corrado877/CognitiveBiasOntologies/tree/main/Naive_Cynicism#receives -->

    <owl:ObjectProperty rdf:about="https://github.com/corrado877/CognitiveBiasOntologies/tree/main/Naive_Cynicism#receives">
        <rdfs:domain rdf:resource="https://w3id.org/framester/data/framestercore/People"/>
        <rdfs:range rdf:resource="https://w3id.org/framester/data/framestercore/Assistance"/>
        <rdfs:comment>denotes the capability of an entity to accept or obtain information, data, or objects from another source.</rdfs:comment>
    </owl:ObjectProperty>
    


    <!-- https://w3id.org/affectedBy#affectedBy -->

    <owl:ObjectProperty rdf:about="https://w3id.org/affectedBy#affectedBy">
        <rdfs:domain>
            <owl:Class>
                <owl:unionOf rdf:parseType="Collection">
                    <rdf:Description rdf:about="http://www.semanticweb.org/mein/ontologies/2024/2/untitled-ontology-17#MentalProperty"/>
                    <rdf:Description rdf:about="https://github.com/corrado877/CognitiveBiasOntologies/blob/main/CognitiveBiasOntologies#Outcome"/>
                    <rdf:Description rdf:about="https://w3id.org/framester/data/framestercore/PerceptionExperience"/>
                </owl:unionOf>
            </owl:Class>
        </rdfs:domain>
        <rdfs:range>
            <owl:Class>
                <owl:unionOf rdf:parseType="Collection">
                    <rdf:Description rdf:about="https://w3id.org/framester/data/framestercore/Evidence"/>
                    <rdf:Description rdf:about="https://w3id.org/framester/data/framestersyn/Belief.n.1"/>
                </owl:unionOf>
            </owl:Class>
        </rdfs:range>
    </owl:ObjectProperty>
    


    <!-- https://w3id.org/affectedBy#influencedBy -->

    <owl:ObjectProperty rdf:about="https://w3id.org/affectedBy#influencedBy">
        <rdfs:domain>
            <owl:Class>
                <owl:unionOf rdf:parseType="Collection">
                    <rdf:Description rdf:about="https://github.com/corrado877/CognitiveBiasOntologies/blob/main/CognitiveBiasOntologies#Decision"/>
                    <rdf:Description rdf:about="https://github.com/corrado877/CognitiveBiasOntologies/blob/main/CognitiveBiasOntologies#Thing"/>
                    <rdf:Description rdf:about="https://w3id.org/framester/data/framestercore/PerceptionExperience"/>
                    <rdf:Description rdf:about="https://w3id.org/framester/data/framestercore/Probability"/>
                </owl:unionOf>
            </owl:Class>
        </rdfs:domain>
        <rdfs:range>
            <owl:Class>
                <owl:unionOf rdf:parseType="Collection">
                    <rdf:Description rdf:about="https://github.com/corrado877/CognitiveBiasOntologies/blob/main/CognitiveBiasOntologies#Decision"/>
                    <rdf:Description rdf:about="https://github.com/corrado877/CognitiveBiasOntologies/blob/main/Neglect_of_probability_bias#Ignore"/>
                    <rdf:Description rdf:about="https://w3id.org/framester/data/framestercore/Pattern"/>
                    <rdf:Description rdf:about="https://w3id.org/framester/data/framestercore/Sequence"/>
                </owl:unionOf>
            </owl:Class>
        </rdfs:range>
        <rdfs:comment>A relation between qualities. A quality is influenced by another quality if the value of the latter affects the value of the former.</rdfs:comment>
    </owl:ObjectProperty>
    


    <!-- 
    ///////////////////////////////////////////////////////////////////////////////////////
    //
    // Data properties
    //
    ///////////////////////////////////////////////////////////////////////////////////////
     -->

    


    <!-- http://www.ontologydesignpatterns.org/cp/owl/parameter.owl#hasParameterDataValue -->

    <owl:DatatypeProperty rdf:about="http://www.ontologydesignpatterns.org/cp/owl/parameter.owl#hasParameterDataValue">
        <rdfs:domain rdf:resource="https://w3id.org/framester/data/framestercore/Identicality"/>
        <rdfs:domain>
            <owl:Class>
                <owl:unionOf rdf:parseType="Collection">
                    <rdf:Description rdf:about="https://w3id.org/framester/data/framestercore/Identicality"/>
                    <rdf:Description rdf:about="https://w3id.org/framester/data/framestercore/Importance"/>
                    <rdf:Description rdf:about="https://w3id.org/framester/data/framestercore/Probability"/>
                </owl:unionOf>
            </owl:Class>
        </rdfs:domain>
        <rdfs:range>
            <rdfs:Datatype>
                <owl:unionOf rdf:parseType="Collection">
                    <rdf:Description rdf:about="http://www.w3.org/2001/XMLSchema#boolean"/>
                    <rdf:Description rdf:about="http://www.w3.org/2001/XMLSchema#string"/>
                </owl:unionOf>
            </rdfs:Datatype>
        </rdfs:range>
        <rdfs:comment>A Concept can have a Parameter that constrains the attributes that a classified Entity can have in a certain Situation.</rdfs:comment>
    </owl:DatatypeProperty>
    


    <!-- https://github.com/corrado877/CognitiveBiasOntologies/blob/main/CognitiveBiasOntologies#Universal -->

    <owl:DatatypeProperty rdf:about="https://github.com/corrado877/CognitiveBiasOntologies/blob/main/CognitiveBiasOntologies#Universal">
        <rdfs:domain>
            <owl:Restriction>
                <owl:onProperty rdf:resource="https://github.com/corrado877/CognitiveBiasOntologies/blob/main/CognitiveBiasOntologies#isPerceivedAs"/>
                <owl:someValuesFrom rdf:resource="https://w3id.org/framester/data/framestersyn/Belief.n.1"/>
            </owl:Restriction>
        </rdfs:domain>
        <rdfs:range rdf:resource="http://www.w3.org/2001/XMLSchema#string"/>
        <rdfs:comment>denotes the deliberate disregard or lack of attention to a particular entity, concept, or information by another entity.</rdfs:comment>
    </owl:DatatypeProperty>
    


    <!-- https://github.com/corrado877/CognitiveBiasOntologies/tree/main/Confabulation%20Bias#Fictional -->

    <owl:DatatypeProperty rdf:about="https://github.com/corrado877/CognitiveBiasOntologies/tree/main/Confabulation%20Bias#Fictional">
        <rdfs:domain>
            <owl:Restriction>
                <owl:onProperty rdf:resource="http://www.w3.org/2000/01/rdf-schema#hasType"/>
                <owl:someValuesFrom rdf:resource="https://w3id.org/framester/data/framestercore/Evidence"/>
            </owl:Restriction>
        </rdfs:domain>
        <rdfs:range rdf:resource="http://www.w3.org/2001/XMLSchema#string"/>
    </owl:DatatypeProperty>
    


    <!-- https://github.com/corrado877/CognitiveBiasOntologies/tree/main/Naive%20Cynicism#Malicious -->

    <owl:DatatypeProperty rdf:about="https://github.com/corrado877/CognitiveBiasOntologies/tree/main/Naive%20Cynicism#Malicious">
        <rdfs:domain>
            <owl:Restriction>
                <owl:onProperty rdf:resource="https://github.com/corrado877/CognitiveBiasOntologies/blob/main/CognitiveBiasOntologies#isPerceivedAs"/>
                <owl:someValuesFrom rdf:resource="https://github.com/corrado877/CognitiveBiasOntologies/blob/main/CognitiveBiasOntologies#Outcome"/>
            </owl:Restriction>
        </rdfs:domain>
    </owl:DatatypeProperty>
    


    <!-- 
    ///////////////////////////////////////////////////////////////////////////////////////
    //
    // Classes
    //
    ///////////////////////////////////////////////////////////////////////////////////////
     -->

    


    <!-- http://www.ontology.se/odp/content/owl/Action.owl#Action -->

    <owl:Class rdf:about="http://www.ontology.se/odp/content/owl/Action.owl#Action">
        <rdfs:comment>The process of doing something. An action is performed by an agent. An action can be proposed (proposed actions make up a plan), implemented or abandoned, and it has a status and possibly one or more suspension periods.</rdfs:comment>
        <rdfs:label>Action</rdfs:label>
    </owl:Class>
    


    <!-- http://www.ontologydesignpatterns.org/cp/owl/move.owl#PhysicalObject -->

    <owl:Class rdf:about="http://www.ontologydesignpatterns.org/cp/owl/move.owl#PhysicalObject">
        <rdfs:subClassOf rdf:resource="https://github.com/corrado877/CognitiveBiasOntologies/blob/main/CognitiveBiasOntologies#Non-humanEntity"/>
        <rdfs:comment>This class comprises items of a material nature that are units for documentation and have physical boundaries that separate them completely in an objective way from other objects.</rdfs:comment>
        <rdfs:label>Physical object</rdfs:label>
    </owl:Class>
    


    <!-- http://www.semanticweb.org/mein/ontologies/2024/2/untitled-ontology-17#MentalProperty -->

    <owl:Class rdf:about="http://www.semanticweb.org/mein/ontologies/2024/2/untitled-ontology-17#MentalProperty">
        <rdfs:comment>MentalProperty, when used for decision-making, refers to the collection of intangible assets, including intellectual property, knowledge assets, creative outputs, innovative ideas, cognitive constructs, and personal and cultural heritage, that are considered and evaluated to inform and guide decision processes. In this context, MentalProperty serves as the foundation upon which decisions are made, providing valuable insights, perspectives, and resources that influence the course of action chosen. Decision-makers may assess and leverage MentalProperty assets to address challenges, capitalize on opportunities, mitigate risks, and achieve desired outcomes.</rdfs:comment>
    </owl:Class>
    


    <!-- https://dbpedia.org/page/Illusion -->

    <owl:Class rdf:about="https://dbpedia.org/page/Illusion">
        <owl:disjointWith rdf:resource="https://github.com/corrado877/CognitiveBiasOntologies/blob/main/CognitiveBiasOntologies#Variables"/>
        <owl:disjointWith rdf:resource="https://w3id.org/framester/data/framestercore/Activity"/>
        <owl:disjointWith rdf:resource="https://w3id.org/framester/data/framestercore/BecomingAware"/>
        <owl:disjointWith rdf:resource="https://w3id.org/framester/data/framestercore/CognitiveConnection"/>
        <owl:disjointWith rdf:resource="https://w3id.org/framester/data/framestercore/ExperiencerObj"/>
        <owl:disjointWith rdf:resource="https://w3id.org/framester/data/framestercore/Pattern"/>
        <owl:disjointWith rdf:resource="https://w3id.org/framester/data/framestercore/People"/>
        <owl:disjointWith rdf:resource="https://w3id.org/framester/data/framestersyn/Person"/>
        <terms:description>An illusion is a distortion of the senses, which can reveal how the mind normally organizes and interprets sensory stimulation. Although illusions distort the human perception of reality, they are generally shared by most people. Illusions may occur with any of the human senses, but visual illusions (optical illusions) are the best-known and understood. The emphasis on visual illusions occurs because vision often dominates the other senses. For example, individuals watching a ventriloquist will perceive the voice is coming from the dummy since they are able to see the dummy mouth the words.</terms:description>
        <rdfs:comment>An illusion is a distortion of the senses, which can reveal how the mind normally organizes and interprets sensory stimulation. Although illusions distort the human perception of reality, they are generally shared by most people. Illusions may occur with any of the human senses, but visual illusions (optical illusions) are the best-known and understood. The emphasis on visual illusions occurs because vision often dominates the other senses. For example, individuals watching a ventriloquist will perceive the voice is coming from the dummy since they are able to see the dummy mouth the words.</rdfs:comment>
        <rdfs:label>Illusion</rdfs:label>
    </owl:Class>
    


    <!-- https://dbpedia.org/page/Success -->

    <owl:Class rdf:about="https://dbpedia.org/page/Success">
        <owl:disjointWith rdf:resource="https://w3id.org/framester/data/framestercore/Activity"/>
        <owl:disjointWith rdf:resource="https://w3id.org/framester/data/framestercore/Event"/>
        <owl:disjointWith rdf:resource="https://w3id.org/framester/data/framestercore/People"/>
        <owl:disjointWith rdf:resource="https://w3id.org/framester/data/framestercore/Probability"/>
        <owl:disjointWith rdf:resource="https://w3id.org/framester/data/framestercore/Sequence"/>
        <terms:description>Success is the state or condition of meeting a defined range of expectations. It may be viewed as the opposite of failure. The criteria for success depend on context and may be relative to a particular observer or belief system. One person might consider a success what another person considers a failure, particularly in cases of direct competition or a zero-sum game. Similarly, the degree of success or failure in a situation may be differently viewed by distinct observers or participants, such that a situation that one considers to be a success, another might consider to be a failure, a qualified success or a neutral situation. For example, a film that is a commercial failure or even a box-office bomb can go on to receive a cult following, with the initial lack of commercial success even.</terms:description>
        <rdfs:label>Success</rdfs:label>
    </owl:Class>
    


    <!-- https://dbpedia.org/resource/Animal -->

    <owl:Class rdf:about="https://dbpedia.org/resource/Animal">
        <rdfs:subClassOf rdf:resource="https://github.com/corrado877/CognitiveBiasOntologies/blob/main/CognitiveBiasOntologies#Non-humanEntity"/>
        <rdfs:comment>Animals are multicellular, eukaryotic organisms in the biological kingdom Animalia. With few exceptions, animals consume organic material, breathe oxygen, are able to move, can reproduce sexually, and go through an ontogenetic stage in which their body consists of a hollow sphere of cells, the blastula, during embryonic development.</rdfs:comment>
        <rdfs:label>Animal</rdfs:label>
    </owl:Class>
    


    <!-- https://dbpedia.org/resource/Concept -->

    <owl:Class rdf:about="https://dbpedia.org/resource/Concept">
        <rdfs:subClassOf rdf:resource="https://github.com/corrado877/CognitiveBiasOntologies/blob/main/CognitiveBiasOntologies#Non-humanEntity"/>
        <rdfs:comment>Concepts are defined as abstract ideas. They are understood to be the fundamental building blocks of the concept behind principles, thoughts and beliefs.They play an important role in all aspects of cognition.</rdfs:comment>
        <rdfs:label>Concept</rdfs:label>
    </owl:Class>
    


    <!-- https://dbpedia.org/resource/Entity -->

    <owl:Class rdf:about="https://dbpedia.org/resource/Entity">
        <rdfs:comment>An entity is something that exists as itself, as a subject or as an object, actually or potentially, concretely or abstractly, physically or not. It need not be of material existence. In particular, abstractions and legal fictions are usually regarded as entities. In general, there is also no presumption that an entity is animate, or present. The adjectival form is entitative.</rdfs:comment>
        <rdfs:comment>An entity is something that exists as itself, as a subject or as an object, actually or potentially, concretely or abstractly, physically or not. It need not be of material existence. In particular, abstractions and legal fictions are usually regarded as entities. In general, there is also no presumption that an entity is animate, or present. The term is broad in scope and may refer to animals; natural features such as mountains; inanimate objects such as tables; numbers or sets as symbols written on a paper; human contrivances such as laws, corporations and academic disciplines; or supernatural beings such as gods and spirits. The adjectival form is entitative. (en)</rdfs:comment>
        <rdfs:label>Entity</rdfs:label>
    </owl:Class>
    


    <!-- https://dbpedia.org/resource/Knowledge -->

    <owl:Class rdf:about="https://dbpedia.org/resource/Knowledge">
        <rdfs:comment>Knowledge can be defined as awareness of facts or as practical skills, and may also refer to familiarity with objects or situations. Knowledge of facts, also called propositional knowledge, is often defined as true belief that is distinct from opinion or guesswork by virtue of justification.</rdfs:comment>
        <rdfs:label>Knowledge</rdfs:label>
    </owl:Class>
    


    <!-- https://dbpedia.org/resource/Plant -->

    <owl:Class rdf:about="https://dbpedia.org/resource/Plant">
        <rdfs:subClassOf rdf:resource="https://github.com/corrado877/CognitiveBiasOntologies/blob/main/CognitiveBiasOntologies#Non-humanEntity"/>
        <rdfs:comment>Plants are predominantly photosynthetic eukaryotes of the kingdom Plantae. Historically, the plant kingdom encompassed all living things that were not animals, and included algae and fungi; however, all current definitions of Plantae exclude the fungi and some algae, as well as the prokaryotes (the archaea and bacteria).</rdfs:comment>
        <rdfs:label>Plant</rdfs:label>
    </owl:Class>
    


    <!-- https://github.com/corrado877/CognitiveBiasOntologies/blob/main/CognitiveBiasOntologies#Agent -->

    <owl:Class rdf:about="https://github.com/corrado877/CognitiveBiasOntologies/blob/main/CognitiveBiasOntologies#Agent">
        <rdfs:subClassOf rdf:resource="https://w3id.org/framester/data/framestercore/People"/>
        <rdfs:comment>Individual who performs the Bias Blind Spot</rdfs:comment>
    </owl:Class>
    


    <!-- https://github.com/corrado877/CognitiveBiasOntologies/blob/main/CognitiveBiasOntologies#AmbiguousStimulus -->

    <owl:Class rdf:about="https://github.com/corrado877/CognitiveBiasOntologies/blob/main/CognitiveBiasOntologies#AmbiguousStimulus">
        <terms:description>A class for colleting different kinds of random stimuli that can involve a sensorial perception.</terms:description>
        <rdfs:label>Ambiguos Stimuli</rdfs:label>
    </owl:Class>
    


    <!-- https://github.com/corrado877/CognitiveBiasOntologies/blob/main/CognitiveBiasOntologies#Bias -->

    <owl:Class rdf:about="https://github.com/corrado877/CognitiveBiasOntologies/blob/main/CognitiveBiasOntologies#Bias">
        <rdfs:comment>Indicates an individual possesses Naive Realism Bias</rdfs:comment>
        <rdfs:comment>a class for defining any kind of bias</rdfs:comment>
    </owl:Class>
    


    <!-- https://github.com/corrado877/CognitiveBiasOntologies/blob/main/CognitiveBiasOntologies#Decision -->

    <owl:Class rdf:about="https://github.com/corrado877/CognitiveBiasOntologies/blob/main/CognitiveBiasOntologies#Decision">
        <owl:disjointWith rdf:resource="https://github.com/corrado877/CognitiveBiasOntologies/blob/main/CognitiveBiasOntologies#Thing"/>
        <owl:disjointWith rdf:resource="https://github.com/corrado877/CognitiveBiasOntologies/blob/main/Neglect_of_probability_bias#Ignore"/>
        <owl:disjointWith rdf:resource="https://w3id.org/framester/data/framestercore/Assessing"/>
        <owl:disjointWith rdf:resource="https://w3id.org/framester/data/framestersyn/Person"/>
        <rdfs:comment>Represents a decision subject to the bias.</rdfs:comment>
        <rdfs:comment>The final decision the individual reaches as ending result of the decision-making process.</rdfs:comment>
        <rdfs:comment>a class representing a decision made in a certain situation</rdfs:comment>
        <rdfs:label>Decision</rdfs:label>
    </owl:Class>
    


    <!-- https://github.com/corrado877/CognitiveBiasOntologies/blob/main/CognitiveBiasOntologies#Feature -->

    <owl:Class rdf:about="https://github.com/corrado877/CognitiveBiasOntologies/blob/main/CognitiveBiasOntologies#Feature">
        <rdfs:comment>The feature, description or title used to refer to an entity</rdfs:comment>
        <rdfs:comment>The feature, description or title used to refer to an entity.</rdfs:comment>
        <rdfs:label>Feature</rdfs:label>
    </owl:Class>
    


    <!-- https://github.com/corrado877/CognitiveBiasOntologies/blob/main/CognitiveBiasOntologies#FutureEvent -->

    <owl:Class rdf:about="https://github.com/corrado877/CognitiveBiasOntologies/blob/main/CognitiveBiasOntologies#FutureEvent">
        <rdfs:subClassOf rdf:resource="https://w3id.org/framester/data/framestercore/Event"/>
        <terms:description>This class represent an event that will happen in the next future.</terms:description>
        <rdfs:label>FutureEvent</rdfs:label>
    </owl:Class>
    


    <!-- https://github.com/corrado877/CognitiveBiasOntologies/blob/main/CognitiveBiasOntologies#HighImportance -->

    <owl:Class rdf:about="https://github.com/corrado877/CognitiveBiasOntologies/blob/main/CognitiveBiasOntologies#HighImportance">
        <owl:equivalentClass>
            <owl:Class>
                <owl:intersectionOf rdf:parseType="Collection">
                    <rdf:Description rdf:about="https://w3id.org/framester/data/framestercore/Importance"/>
                    <owl:Restriction>
                        <owl:onProperty rdf:resource="http://www.ontologydesignpatterns.org/cp/owl/parameter.owl#hasParameterDataValue"/>
                        <owl:hasValue>High</owl:hasValue>
                    </owl:Restriction>
                </owl:intersectionOf>
            </owl:Class>
        </owl:equivalentClass>
        <rdfs:subClassOf rdf:resource="https://w3id.org/framester/data/framestercore/Importance"/>
    </owl:Class>
    


    <!-- https://github.com/corrado877/CognitiveBiasOntologies/blob/main/CognitiveBiasOntologies#HumanFeature -->

    <owl:Class rdf:about="https://github.com/corrado877/CognitiveBiasOntologies/blob/main/CognitiveBiasOntologies#HumanFeature">
        <rdfs:subClassOf rdf:resource="https://github.com/corrado877/CognitiveBiasOntologies/blob/main/CognitiveBiasOntologies#Feature"/>
        <rdfs:comment>Defines a feature of a human being</rdfs:comment>
        <rdfs:label>Human feature</rdfs:label>
    </owl:Class>
    


    <!-- https://github.com/corrado877/CognitiveBiasOntologies/blob/main/CognitiveBiasOntologies#KnownFeature -->

    <owl:Class rdf:about="https://github.com/corrado877/CognitiveBiasOntologies/blob/main/CognitiveBiasOntologies#KnownFeature">
        <rdfs:subClassOf rdf:resource="https://dbpedia.org/resource/Knowledge"/>
        <rdfs:subClassOf rdf:resource="https://github.com/corrado877/CognitiveBiasOntologies/blob/main/CognitiveBiasOntologies#Feature"/>
        <rdfs:comment>The feature, description or title used to refer to an entity and aknowledged by the individual.</rdfs:comment>
        <rdfs:label>Known feature</rdfs:label>
    </owl:Class>
    


    <!-- https://github.com/corrado877/CognitiveBiasOntologies/blob/main/CognitiveBiasOntologies#LowImportance -->

    <owl:Class rdf:about="https://github.com/corrado877/CognitiveBiasOntologies/blob/main/CognitiveBiasOntologies#LowImportance">
        <owl:equivalentClass>
            <owl:Class>
                <owl:intersectionOf rdf:parseType="Collection">
                    <rdf:Description rdf:about="https://w3id.org/framester/data/framestercore/Importance"/>
                    <owl:Restriction>
                        <owl:onProperty rdf:resource="http://www.ontologydesignpatterns.org/cp/owl/parameter.owl#hasParameterDataValue"/>
                        <owl:hasValue>Low</owl:hasValue>
                    </owl:Restriction>
                </owl:intersectionOf>
            </owl:Class>
        </owl:equivalentClass>
        <rdfs:subClassOf rdf:resource="https://w3id.org/framester/data/framestercore/Importance"/>
    </owl:Class>
    


    <!-- https://github.com/corrado877/CognitiveBiasOntologies/blob/main/CognitiveBiasOntologies#MemoryEncoding -->

    <owl:Class rdf:about="https://github.com/corrado877/CognitiveBiasOntologies/blob/main/CognitiveBiasOntologies#MemoryEncoding">
        <rdfs:comment>The process of encoding memory.</rdfs:comment>
        <rdfs:label>Memory encoding</rdfs:label>
    </owl:Class>
    


    <!-- https://github.com/corrado877/CognitiveBiasOntologies/blob/main/CognitiveBiasOntologies#MemoryGap -->

    <owl:Class rdf:about="https://github.com/corrado877/CognitiveBiasOntologies/blob/main/CognitiveBiasOntologies#MemoryGap">
        <rdfs:comment>a class for Missing or incomplete information in memory</rdfs:comment>
    </owl:Class>
    


    <!-- https://github.com/corrado877/CognitiveBiasOntologies/blob/main/CognitiveBiasOntologies#NextChance-BasedOccurence -->

    <owl:Class rdf:about="https://github.com/corrado877/CognitiveBiasOntologies/blob/main/CognitiveBiasOntologies#NextChance-BasedOccurence">
        <rdfs:subClassOf rdf:resource="https://github.com/corrado877/CognitiveBiasOntologies/blob/main/CognitiveBiasOntologies#FutureEvent"/>
        <rdfs:subClassOf>
            <owl:Restriction>
                <owl:onProperty rdf:resource="http://www.ontologydesignpatterns.org/cp/owl/partof.owl#isPartOf"/>
                <owl:someValuesFrom rdf:resource="https://w3id.org/framester/data/framestercore/Activity"/>
            </owl:Restriction>
        </rdfs:subClassOf>
        <terms:description>This class represent an event that will happen in the next future and it is characterized by chance-based probability.</terms:description>
        <rdfs:label>Next Chance-Based Occurence</rdfs:label>
    </owl:Class>
    


    <!-- https://github.com/corrado877/CognitiveBiasOntologies/blob/main/CognitiveBiasOntologies#NextRandomOccurrence -->

    <owl:Class rdf:about="https://github.com/corrado877/CognitiveBiasOntologies/blob/main/CognitiveBiasOntologies#NextRandomOccurrence">
        <rdfs:subClassOf rdf:resource="https://github.com/corrado877/CognitiveBiasOntologies/blob/main/CognitiveBiasOntologies#FutureEvent"/>
        <rdfs:subClassOf>
            <owl:Restriction>
                <owl:onProperty rdf:resource="http://www.ontologydesignpatterns.org/cp/owl/partof.owl#isPartOf"/>
                <owl:someValuesFrom rdf:resource="https://w3id.org/framester/data/framestercore/Activity"/>
            </owl:Restriction>
        </rdfs:subClassOf>
        <terms:description>This class represent an event that will happen in the next future and it is characterized by randomness.</terms:description>
        <rdfs:label>NextRandomOccurence</rdfs:label>
    </owl:Class>
    


    <!-- https://github.com/corrado877/CognitiveBiasOntologies/blob/main/CognitiveBiasOntologies#Non-humanEntity -->

    <owl:Class rdf:about="https://github.com/corrado877/CognitiveBiasOntologies/blob/main/CognitiveBiasOntologies#Non-humanEntity">
        <rdfs:subClassOf rdf:resource="https://dbpedia.org/resource/Entity"/>
        <rdfs:comment>Any entity that isn&apos;t human</rdfs:comment>
        <rdfs:label>Non-human entity</rdfs:label>
    </owl:Class>
    


    <!-- https://github.com/corrado877/CognitiveBiasOntologies/blob/main/CognitiveBiasOntologies#Outcome -->

    <owl:Class rdf:about="https://github.com/corrado877/CognitiveBiasOntologies/blob/main/CognitiveBiasOntologies#Outcome">
        <owl:disjointWith rdf:resource="https://w3id.org/framester/data/framestercore/Activity"/>
        <owl:disjointWith rdf:resource="https://w3id.org/framester/data/framestercore/Event"/>
        <owl:disjointWith rdf:resource="https://w3id.org/framester/data/framestercore/People"/>
        <owl:disjointWith rdf:resource="https://w3id.org/framester/data/framestercore/Probability"/>
        <owl:disjointWith rdf:resource="https://w3id.org/framester/data/framestercore/Sequence"/>
        <terms:description>This class represent the outcome of an event such as a RandomOccurence</terms:description>
        <rdfs:comment>Refers to the result, effect, or consequence of a particular action, event, process, or situation</rdfs:comment>
        <rdfs:comment>Resulting consequences of experienced event</rdfs:comment>
        <rdfs:label>Outcome</rdfs:label>
        <rdfs:label>The final result of an activity.</rdfs:label>
    </owl:Class>
    


    <!-- https://github.com/corrado877/CognitiveBiasOntologies/blob/main/CognitiveBiasOntologies#OutcomeColorNumber -->

    <owl:Class rdf:about="https://github.com/corrado877/CognitiveBiasOntologies/blob/main/CognitiveBiasOntologies#OutcomeColorNumber">
        <rdfs:subClassOf rdf:resource="https://github.com/corrado877/CognitiveBiasOntologies/blob/main/CognitiveBiasOntologies#Outcome"/>
        <terms:description>A class representing a type of Outcome such as Colored Numbers</terms:description>
        <rdfs:label>ColorNumber</rdfs:label>
    </owl:Class>
    


    <!-- https://github.com/corrado877/CognitiveBiasOntologies/blob/main/CognitiveBiasOntologies#PastMemory -->

    <owl:Class rdf:about="https://github.com/corrado877/CognitiveBiasOntologies/blob/main/CognitiveBiasOntologies#PastMemory">
        <owl:equivalentClass>
            <owl:Class>
                <owl:intersectionOf rdf:parseType="Collection">
                    <rdf:Description rdf:about="https://w3id.org/framester/data/framestercore/Memory"/>
                    <owl:Restriction>
                        <owl:onProperty rdf:resource="http://www.ontologydesignpatterns.org/cp/owl/parameter.owl#hasParameter"/>
                        <owl:someValuesFrom rdf:resource="https://github.com/corrado877/CognitiveBiasOntologies/blob/main/CognitiveBiasOntologies#LowImportance"/>
                    </owl:Restriction>
                </owl:intersectionOf>
            </owl:Class>
        </owl:equivalentClass>
        <rdfs:subClassOf rdf:resource="https://w3id.org/framester/data/framestercore/Memory"/>
        <rdfs:comment>A memory that has been produced previously in the memory encoding process.</rdfs:comment>
        <rdfs:label>Past memory</rdfs:label>
    </owl:Class>
    


    <!-- https://github.com/corrado877/CognitiveBiasOntologies/blob/main/CognitiveBiasOntologies#PerceivedValidity -->

    <owl:Class rdf:about="https://github.com/corrado877/CognitiveBiasOntologies/blob/main/CognitiveBiasOntologies#PerceivedValidity">
        <rdfs:comment>It assess the perceived validity of an object due to a perception activity</rdfs:comment>
        <rdfs:label>Perceived validity</rdfs:label>
    </owl:Class>
    


    <!-- https://github.com/corrado877/CognitiveBiasOntologies/blob/main/CognitiveBiasOntologies#RecentMemory -->

    <owl:Class rdf:about="https://github.com/corrado877/CognitiveBiasOntologies/blob/main/CognitiveBiasOntologies#RecentMemory">
        <owl:equivalentClass>
            <owl:Class>
                <owl:intersectionOf rdf:parseType="Collection">
                    <rdf:Description rdf:about="https://w3id.org/framester/data/framestercore/Memory"/>
                    <owl:Restriction>
                        <owl:onProperty rdf:resource="http://www.ontologydesignpatterns.org/cp/owl/parameter.owl#hasParameter"/>
                        <owl:someValuesFrom rdf:resource="https://github.com/corrado877/CognitiveBiasOntologies/blob/main/CognitiveBiasOntologies#HighImportance"/>
                    </owl:Restriction>
                </owl:intersectionOf>
            </owl:Class>
        </owl:equivalentClass>
        <rdfs:subClassOf rdf:resource="https://w3id.org/framester/data/framestercore/Memory"/>
        <rdfs:comment>A memory that has been produced more recently in the memory encoding process.</rdfs:comment>
        <rdfs:label>Recent memory</rdfs:label>
    </owl:Class>
    


    <!-- https://github.com/corrado877/CognitiveBiasOntologies/blob/main/CognitiveBiasOntologies#RecognizablePattern -->

    <owl:Class rdf:about="https://github.com/corrado877/CognitiveBiasOntologies/blob/main/CognitiveBiasOntologies#RecognizablePattern">
        <rdfs:subClassOf rdf:resource="https://w3id.org/framester/data/framestercore/Pattern"/>
    </owl:Class>
    


    <!-- https://github.com/corrado877/CognitiveBiasOntologies/blob/main/CognitiveBiasOntologies#Thing -->

    <owl:Class rdf:about="https://github.com/corrado877/CognitiveBiasOntologies/blob/main/CognitiveBiasOntologies#Thing">
        <owl:disjointWith rdf:resource="https://github.com/corrado877/CognitiveBiasOntologies/blob/main/Neglect_of_probability_bias#Ignore"/>
        <owl:disjointWith rdf:resource="https://w3id.org/framester/data/framestercore/Assessing"/>
        <owl:disjointWith rdf:resource="https://w3id.org/framester/data/framestersyn/Person"/>
        <rdfs:comment>a class for defining any kind of information about which a person has some knowledge</rdfs:comment>
    </owl:Class>
    


    <!-- https://github.com/corrado877/CognitiveBiasOntologies/blob/main/CognitiveBiasOntologies#Un-knownFeature -->

    <owl:Class rdf:about="https://github.com/corrado877/CognitiveBiasOntologies/blob/main/CognitiveBiasOntologies#Un-knownFeature">
        <rdfs:subClassOf rdf:resource="https://github.com/corrado877/CognitiveBiasOntologies/blob/main/CognitiveBiasOntologies#Feature"/>
        <rdfs:comment>The feature, description or title used to refer to an entity but not aknowledged by the individual.</rdfs:comment>
        <rdfs:label>Un-known feature</rdfs:label>
    </owl:Class>
    


    <!-- https://github.com/corrado877/CognitiveBiasOntologies/blob/main/CognitiveBiasOntologies#VariableEntity1 -->

    <owl:Class rdf:about="https://github.com/corrado877/CognitiveBiasOntologies/blob/main/CognitiveBiasOntologies#VariableEntity1">
        <rdfs:subClassOf rdf:resource="https://github.com/corrado877/CognitiveBiasOntologies/blob/main/CognitiveBiasOntologies#Variables"/>
        <rdfs:subClassOf>
            <owl:Restriction>
                <owl:onProperty rdf:resource="http://www.ontologydesignpatterns.org/cp/owl/partof.owl#isPartOf"/>
                <owl:someValuesFrom rdf:resource="https://github.com/corrado877/CognitiveBiasOntologies/blob/main/CognitiveBiasOntologies#VariablesPattern"/>
            </owl:Restriction>
        </rdfs:subClassOf>
        <owl:disjointWith rdf:resource="https://github.com/corrado877/CognitiveBiasOntologies/blob/main/CognitiveBiasOntologies#VariableEntity2"/>
        <terms:description>A class for one one of the two variables that are perceived as correlated.</terms:description>
        <rdfs:label>Variable Entity 1</rdfs:label>
    </owl:Class>
    


    <!-- https://github.com/corrado877/CognitiveBiasOntologies/blob/main/CognitiveBiasOntologies#VariableEntity2 -->

    <owl:Class rdf:about="https://github.com/corrado877/CognitiveBiasOntologies/blob/main/CognitiveBiasOntologies#VariableEntity2">
        <rdfs:subClassOf rdf:resource="https://github.com/corrado877/CognitiveBiasOntologies/blob/main/CognitiveBiasOntologies#Variables"/>
        <rdfs:subClassOf>
            <owl:Restriction>
                <owl:onProperty rdf:resource="http://www.ontologydesignpatterns.org/cp/owl/partof.owl#isPartOf"/>
                <owl:someValuesFrom rdf:resource="https://github.com/corrado877/CognitiveBiasOntologies/blob/main/CognitiveBiasOntologies#VariablesPattern"/>
            </owl:Restriction>
        </rdfs:subClassOf>
        <terms:description>A class for one one of the two variables that are perceived as correlated.</terms:description>
        <rdfs:label>Variable Entity 2</rdfs:label>
    </owl:Class>
    


    <!-- https://github.com/corrado877/CognitiveBiasOntologies/blob/main/CognitiveBiasOntologies#Variables -->

    <owl:Class rdf:about="https://github.com/corrado877/CognitiveBiasOntologies/blob/main/CognitiveBiasOntologies#Variables">
        <owl:disjointWith rdf:resource="https://w3id.org/framester/data/framestercore/Activity"/>
        <owl:disjointWith rdf:resource="https://w3id.org/framester/data/framestercore/BecomingAware"/>
        <owl:disjointWith rdf:resource="https://w3id.org/framester/data/framestercore/CognitiveConnection"/>
        <owl:disjointWith rdf:resource="https://w3id.org/framester/data/framestercore/Pattern"/>
        <owl:disjointWith rdf:resource="https://w3id.org/framester/data/framestercore/People"/>
        <terms:description>A class representing all the possible variables or attributes that individuals mistakenly perceive to be correlated.</terms:description>
        <rdfs:label>Variables</rdfs:label>
    </owl:Class>
    


    <!-- https://github.com/corrado877/CognitiveBiasOntologies/blob/main/CognitiveBiasOntologies#VariablesPattern -->

    <owl:Class rdf:about="https://github.com/corrado877/CognitiveBiasOntologies/blob/main/CognitiveBiasOntologies#VariablesPattern">
        <owl:equivalentClass>
            <owl:Class>
                <owl:intersectionOf rdf:parseType="Collection">
                    <rdf:Description rdf:about="https://w3id.org/framester/data/framestercore/Pattern"/>
                    <owl:Restriction>
                        <owl:onProperty rdf:resource="http://www.ontologydesignpatterns.org/cp/owl/partof.owl#hasPart"/>
                        <owl:someValuesFrom rdf:resource="https://github.com/corrado877/CognitiveBiasOntologies/blob/main/CognitiveBiasOntologies#VariableEntity1"/>
                    </owl:Restriction>
                    <owl:Restriction>
                        <owl:onProperty rdf:resource="http://www.ontologydesignpatterns.org/cp/owl/partof.owl#hasPart"/>
                        <owl:someValuesFrom rdf:resource="https://github.com/corrado877/CognitiveBiasOntologies/blob/main/CognitiveBiasOntologies#VariableEntity2"/>
                    </owl:Restriction>
                </owl:intersectionOf>
            </owl:Class>
        </owl:equivalentClass>
        <rdfs:subClassOf rdf:resource="https://github.com/corrado877/CognitiveBiasOntologies/blob/main/CognitiveBiasOntologies#RecognizablePattern"/>
        <terms:description>An class and its individual representing the type of pattern recognized by an human agent as part of a trend, in this case a pattern where two elements often appear together.</terms:description>
        <rdfs:label>Variables Pattern</rdfs:label>
    </owl:Class>
    


    <!-- https://github.com/corrado877/CognitiveBiasOntologies/blob/main/CognitiveBiasOntologies#VisualStimulus -->

    <owl:Class rdf:about="https://github.com/corrado877/CognitiveBiasOntologies/blob/main/CognitiveBiasOntologies#VisualStimulus">
        <rdfs:subClassOf rdf:resource="https://github.com/corrado877/CognitiveBiasOntologies/blob/main/CognitiveBiasOntologies#AmbiguousStimulus"/>
        <terms:description>A class for visual stimuli, namely anything that involves the use of sight.</terms:description>
        <rdfs:label>Visual Stimulus</rdfs:label>
    </owl:Class>
    


    <!-- https://github.com/corrado877/CognitiveBiasOntologies/blob/main/Neglect_of_probability_bias#Ignore -->

    <owl:Class rdf:about="https://github.com/corrado877/CognitiveBiasOntologies/blob/main/Neglect_of_probability_bias#Ignore">
        <owl:disjointWith rdf:resource="https://w3id.org/framester/data/framestercore/Assessing"/>
        <owl:disjointWith rdf:resource="https://w3id.org/framester/data/framestersyn/Person"/>
    </owl:Class>
    


    <!-- https://w3id.org/framester/data/framestercore/Activity -->

    <owl:Class rdf:about="https://w3id.org/framester/data/framestercore/Activity">
        <owl:disjointWith rdf:resource="https://w3id.org/framester/data/framestercore/BecomingAware"/>
        <owl:disjointWith rdf:resource="https://w3id.org/framester/data/framestercore/CognitiveConnection"/>
        <owl:disjointWith rdf:resource="https://w3id.org/framester/data/framestercore/Event"/>
        <owl:disjointWith rdf:resource="https://w3id.org/framester/data/framestercore/ExperiencerObj"/>
        <owl:disjointWith rdf:resource="https://w3id.org/framester/data/framestercore/Pattern"/>
        <owl:disjointWith rdf:resource="https://w3id.org/framester/data/framestercore/People"/>
        <owl:disjointWith rdf:resource="https://w3id.org/framester/data/framestercore/PerceptionExperience"/>
        <owl:disjointWith rdf:resource="https://w3id.org/framester/data/framestercore/Probability"/>
        <owl:disjointWith rdf:resource="https://w3id.org/framester/data/framestercore/Sequence"/>
        <owl:disjointWith rdf:resource="https://w3id.org/framester/data/framestersyn/Person"/>
        <terms:description>This is an abstract frame for durative activities, in which the Agent enters an ongoing state of the Activity, remains in this state for some Duration of Time, and leaves this state either by finishing or by stopping. The Agent&apos;s Activity should be intentional. This frame is intended mostly for the inheritance of common FEs, and to provide the frame structure for the beginning, ongoing, finish, or stop stage of an Activity, each of which constitutes a subframe of this frame. This frame should be compared to the Process frame</terms:description>
        <terms:description>This is an abstract frame for durative activities, in which the Agent enters an ongoing state of the Activity, remains in this state for some Duration of Time, and leaves this state either by finishing or by stopping. The Agent&apos;s Activity should be intentional. This frame is intended mostly for the inheritance of common FEs, and to provide the frame structure for the beginning, ongoing, finish, or stop stage of an Activity, each of which constitutes a subframe of this frame. This frame should be compared to the Process frame.</terms:description>
        <terms:description>This is an abstract frame for durative activities, in which the Agent enters an ongoing state of the Activity, remains in this state for some Duration of Time, and leaves this state either by finishing or by stopping. The Agent&apos;s Activity should be intentional. This frame is intended mostly for the inheritance of common FEs, and to provide the frame structure for the beginning, ongoing, finish, or stop stage of an Activity, each of which constitutes a subframe of this frame. This frame should be compared to the Process frame.  In this case is a class representing an activity affected by a certain cognitive process (Becoming Aware of something).</terms:description>
        <terms:description>This is an abstract frame for durative activities, in which the Agent enters an ongoing state of the Activity, remains in this state for some Duration of Time, and leaves this state either by finishing or by stopping. The Agent&apos;s Activity should be intentional. This frame is intended mostly for the inheritance of common FEs, and to provide the frame structure for the beginning, ongoing, finish, or stop stage of an Activity, each of which constitutes a subframe of this frame. This frame should be compared to the Process frame. In this case the frame represents an activity with random or chance-based outcomes in which a person is involved in.</terms:description>
        <rdfs:comment>This is an abstract frame for durative activities, in which the Agent enters an ongoing state of the Activity, remains in this state for some Duration of Time, and leaves this state either by finishing or by stopping. The Agent&apos;s Activity should be intentional. This frame is intended mostly for the inheritance of common FEs, and to provide the frame structure for the beginning, ongoing, finish, or stop stage of an Activity, each of which constitutes a subframe of this frame. This frame should be compared to the Process frame.</rdfs:comment>
        <rdfs:label>Activity</rdfs:label>
    </owl:Class>
    


    <!-- https://w3id.org/framester/data/framestercore/Assessing -->

    <owl:Class rdf:about="https://w3id.org/framester/data/framestercore/Assessing">
        <owl:disjointWith rdf:resource="https://w3id.org/framester/data/framestersyn/Person"/>
        <rdfs:comment>An Assessor examines a Phenomenon to figure out its Value according to some Feature of the Phenomenon. This Value is a factor in determining the acceptability of the Phenomenon. In some cases, a Method (implicitly involving an Assessor) is used to determine the Phenomenon&apos;s Value. Each company is then evaluated for their earning potential. CNI From the evidence of the pilot studies the risk of damage to the test subjects was rated too high to continue. CNI He weighed his options carefully.</rdfs:comment>
    </owl:Class>
    


    <!-- https://w3id.org/framester/data/framestercore/Assistance -->

    <owl:Class rdf:about="https://w3id.org/framester/data/framestercore/Assistance">
        <rdfs:comment>A Helper benefits a Benefited_party by enabling the culmination of a Goal that the Benefited_party has. A Focal_entity that is involved in reaching the Goal may stand in for it. Will you help the Government find your brother? Maybe Stephen should assist him with the last manuscript. They helped me psychologically to overcome the physical loss I had suffered. You have helped him tremendously by showing him how to stand up for himself and by being his friend. By bringing assistance to his troops wherever they were in trouble he aided them greatly.</rdfs:comment>
    </owl:Class>
    


    <!-- https://w3id.org/framester/data/framestercore/BecomingAware -->

    <owl:Class rdf:about="https://w3id.org/framester/data/framestercore/BecomingAware">
        <owl:disjointWith rdf:resource="https://w3id.org/framester/data/framestercore/CognitiveConnection"/>
        <owl:disjointWith rdf:resource="https://w3id.org/framester/data/framestercore/Pattern"/>
        <owl:disjointWith rdf:resource="https://w3id.org/framester/data/framestercore/People"/>
        <terms:description>Words in this frame have to do with a Cognizer adding some Phenomenon to their model of the world. They are similar to Coming-to-believe words, except the latter generally involve reasoning from Evidence. The words in this frame take direct objects that denote entities in the world, and indicate awareness of those entities, without necessarily giving any information about the content of the Cognizer&apos;s belief or knowledge. These words also resemble perception words, since creatures often become aware of things by perceiving them. Later that night, they found the barely-alive victim inside the Red Hall estate flat. Almost immediately, the police discovered the wrought-iron crypt gate swinging open. In the bag on the tableI could vaguely discern two bottles of wine and several cartons of cakes and other goodies. People passing through recognize it from afar, by the clouds of coal dust darkening the air. General Grammatical Observations: Passive forms of the verbs in this frame can occur with extraposed clauses expressing Phenomenon: That year it was discovered that consumers preferred the older model. It is not always recognized how much work goes into a dinner party.</terms:description>
        <rdfs:label>Becoming Aware</rdfs:label>
    </owl:Class>
    


    <!-- https://w3id.org/framester/data/framestercore/CognitiveConnection -->

    <owl:Class rdf:about="https://w3id.org/framester/data/framestercore/CognitiveConnection">
        <owl:disjointWith rdf:resource="https://w3id.org/framester/data/framestercore/Pattern"/>
        <owl:disjointWith rdf:resource="https://w3id.org/framester/data/framestercore/People"/>
        <terms:description>A concept, Concept_1, is related causally or collocationally to another concept, Concept_2, by means of some Evidence. They may be related only under certain Circumstances or from a certain Point_of_view. The two concepts may be expressed collectively as associated Concepts. Any cognizer is deprofiled.</terms:description>
        <rdfs:label>Cognitive Connection</rdfs:label>
    </owl:Class>
    


    <!-- https://w3id.org/framester/data/framestercore/Deciding -->

    <owl:Class rdf:about="https://w3id.org/framester/data/framestercore/Deciding"/>
    


    <!-- https://w3id.org/framester/data/framestercore/Event -->

    <owl:Class rdf:about="https://w3id.org/framester/data/framestercore/Event">
        <owl:disjointWith rdf:resource="https://w3id.org/framester/data/framestercore/People"/>
        <owl:disjointWith rdf:resource="https://w3id.org/framester/data/framestercore/Probability"/>
        <owl:disjointWith rdf:resource="https://w3id.org/framester/data/framestercore/Sequence"/>
        <terms:description>An Event takes place at a Place and Time. Big earthquakes only happen along plate boundaries. INI The party will take place on Sunday in the all-you-can-eat buffet.</terms:description>
        <rdfs:comment>An Event takes place at a Place and Time. Big earthquakes only happen along plate boundaries. INI The party will take place on Sunday in the all-you-can-eat buffet. Eg:Situation prompting the emergence of Confabulation Bias</rdfs:comment>
        <rdfs:comment>An Event takes place at a Place and Time. Big earthquakes only happen along plate boundaries.INI The party will take place on Sunday in the all-you-can-eat buffet.</rdfs:comment>
        <rdfs:label>Event</rdfs:label>
    </owl:Class>
    


    <!-- https://w3id.org/framester/data/framestercore/Evidence -->

    <owl:Class rdf:about="https://w3id.org/framester/data/framestercore/Evidence">
        <rdfs:comment>The Support, a phenomenon or fact, lends support to a claim or proposed course of action, the Proposition, where the Domain_of_Relevance may also be expressed. Some of the words in this frame (e.g. argue) are communication words used in a non-communicative, epistemic sense. The latest poll results show that support of the president is at an all-time low.  Eg:Fabricated narrative created to fill memory gaps</rdfs:comment>
    </owl:Class>
    


    <!-- https://w3id.org/framester/data/framestercore/Expectation -->

    <owl:Class rdf:about="https://w3id.org/framester/data/framestercore/Expectation">
        <rdfs:comment>Words in this frame have to do with a Cognizer believing that some Phenomenon will take place in the future. Some words in the frame (e.g. foresee.v) indicate that the Phenomenon is asserted also to be true, while others do not.</rdfs:comment>
        <rdfs:label>Expectation</rdfs:label>
    </owl:Class>
    


    <!-- https://w3id.org/framester/data/framestercore/ExperiencerObj -->

    <owl:Class rdf:about="https://w3id.org/framester/data/framestercore/ExperiencerObj">
        <owl:disjointWith rdf:resource="https://w3id.org/framester/data/framestercore/Pattern"/>
        <owl:disjointWith rdf:resource="https://w3id.org/framester/data/framestercore/PerceptionExperience"/>
        <owl:disjointWith rdf:resource="https://w3id.org/framester/data/framestercore/Sequence"/>
        <owl:disjointWith rdf:resource="https://w3id.org/framester/data/framestersyn/Person"/>
        <rdfs:comment>Some phenomenon (the Stimulus) provokes a particular emotion in an Experiencer. Nightmare on Elm Street scared me silly.</rdfs:comment>
    </owl:Class>
    


    <!-- https://w3id.org/framester/data/framestercore/Identicality -->

    <owl:Class rdf:about="https://w3id.org/framester/data/framestercore/Identicality">
        <rdfs:comment>A Current_instance of a certain Type is under discussion. This instance is evaluated as being the same instance or a different instance from a Previous_instance encountered in a Previous_context.</rdfs:comment>
        <rdfs:label>Identicality</rdfs:label>
    </owl:Class>
    


    <!-- https://w3id.org/framester/data/framestercore/Importance -->

    <owl:Class rdf:about="https://w3id.org/framester/data/framestercore/Importance">
        <rdfs:comment>A Factor affects the outcome of an Undertaking, which can be a goal-oriented activity or the maintenance of a desirable state, the work in a Field, or something portrayed as affecting an Interested_party. A Reason may be given for the importance of the Factor. The Degree of importance may also be specified.</rdfs:comment>
        <rdfs:label>Importance</rdfs:label>
    </owl:Class>
    


    <!-- https://w3id.org/framester/data/framestercore/Memory -->

    <owl:Class rdf:about="https://w3id.org/framester/data/framestercore/Memory">
        <rdfs:comment>This frame is concerned with Cognizers remembering and forgetting mental Content.</rdfs:comment>
        <rdfs:label>Memory</rdfs:label>
    </owl:Class>
    


    <!-- https://w3id.org/framester/data/framestercore/Pattern -->

    <owl:Class rdf:about="https://w3id.org/framester/data/framestercore/Pattern">
        <owl:disjointWith rdf:resource="https://w3id.org/framester/data/framestercore/People"/>
        <owl:disjointWith rdf:resource="https://w3id.org/framester/data/framestercore/PerceptionExperience"/>
        <owl:disjointWith rdf:resource="https://w3id.org/framester/data/framestercore/Sequence"/>
        <owl:disjointWith rdf:resource="https://w3id.org/framester/data/framestersyn/Person"/>
        <terms:description>This frame describes the interrelation of a collection of Entities; they may be physical entities or shapes in a recognizable configuration, a pattern of events, or a relation among abstract entities. The pattern is not the individual Entities nor the set of Entities, but an abstraction of their interrelations, as a gestalt. The Cougers are playing in a Wing-T formation tonight. The auditors noticed a suspicious pattern of withdrawals from the maintenance account . The digits of irrational numbers do not repeat in any kind of pattern.</terms:description>
        <rdfs:comment>This frame describes the interrelation of a collection of Entities; they may be physical entities or shapes in a recognizable configuration, a pattern of events, or a relation among abstract entities. The pattern is not the individual Entities nor the set of Entities, but an abstraction of their interrelations, as a gestalt. The Cougers are playing in a Wing-T formation tonight. The auditors noticed a suspicious pattern of withdrawals from the maintenance account . The digits of irrational numbers do not repeat in any kind of pattern.</rdfs:comment>
        <rdfs:label>Pattern</rdfs:label>
    </owl:Class>
    


    <!-- https://w3id.org/framester/data/framestercore/People -->

    <owl:Class rdf:about="https://w3id.org/framester/data/framestercore/People">
        <owl:disjointWith rdf:resource="https://w3id.org/framester/data/framestercore/Probability"/>
        <owl:disjointWith rdf:resource="https://w3id.org/framester/data/framestercore/Sequence"/>
        <terms:description>This frame contains general words for Individuals, i.e. humans. The Person is conceived of as independent of other specific individuals with whom they have relationships and independent of their participation in any particular activity. They may have an Age, Descriptor, Origin, Persistent_characteristic, or Ethnicity. A man from Phoenix was shot yesterday. She gave birth to a screaming baby yesterday. I study 16-year-old female adolescents. I am dating an African-American man. She comforted the terrified child. I always thought of him as a stupid man.</terms:description>
        <rdfs:comment>This frame contains general words for Individuals, i.e. humans. The Person is conceived of as independent of other specific individuals with whom they have relationships and independent of their participation in any particular activity.</rdfs:comment>
        <rdfs:comment>This frame contains general words for Individuals, i.e. humans. The Person is conceived of as independent of other specific individuals with whom they have relationships and independent of their participation in any particular activity. They may have an Age, Descriptor, Origin, Persistent_characteristic, or Ethnicity. A man from Phoenix was shot yesterday. She gave birth to a screaming babyyesterday. I study 16-year-old female adolescents. I am dating an African-American man. She comforted the terrified child. I always thought of him as a stupid man.</rdfs:comment>
        <rdfs:label>People</rdfs:label>
    </owl:Class>
    


    <!-- https://w3id.org/framester/data/framestercore/PerceptionExperience -->

    <owl:Class rdf:about="https://w3id.org/framester/data/framestercore/PerceptionExperience">
        <owl:disjointWith rdf:resource="https://w3id.org/framester/data/framestercore/Sequence"/>
        <owl:disjointWith rdf:resource="https://w3id.org/framester/data/framestersyn/Person"/>
        <terms:description>This frame contains perception words whose Perceivers have perceptual experiences that they do not necessarily intend to. For this reason we call the Perceiver role Perceiver_passive. Comparing the Perception_experience frame to the Perception_active frame, we note that for some modalities there are different lexical items in each frame. For instance, whereas Perception_experience has see, Perception_active has look at. For other sense modalities, we find the same lexical items in both frames. To illustrate, consider the verb smell where I smell something rotten exemplifies its Perception_experience use and Smell this to see if it&apos;s fresh exemplifies its Perception_active sense. This frame also includes words which are not specific to any sense modality, including detect, perceive, perception, sense.</terms:description>
        <rdfs:comment>Perception experience</rdfs:comment>
        <rdfs:comment>This frame contains perception words whose Perceivers have perceptual experiences that they do not necessarily intend to. For this reason we call the Perceiver role Perceiver_passive. Comparing the Perception_experience frame to the Perception_active frame, we note that for some modalities there are different lexical items in each frame. For instance, whereas Perception_experience has see, Perception_active has look at. For other sense modalities, we find the same lexical items in both frames. To illustrate, consider the verb smell where I smell something rotten exemplifies its Perception_experience use and Smell this to see if it&apos;s fresh exemplifies its Perception_active sense. This frame also includes words which are not specific to any sense modality, including detect, perceive, perception, sense.</rdfs:comment>
        <rdfs:label>Perception Experience</rdfs:label>
        <rdfs:label>Perception experience</rdfs:label>
    </owl:Class>
    


    <!-- https://w3id.org/framester/data/framestercore/Predicting -->

    <owl:Class rdf:about="https://w3id.org/framester/data/framestercore/Predicting">
        <rdfs:comment>A Speaker states or makes known a future Eventuality on the basis of some Evidence.</rdfs:comment>
        <rdfs:label>Predicting</rdfs:label>
    </owl:Class>
    


    <!-- https://w3id.org/framester/data/framestercore/Probability -->

    <owl:Class rdf:about="https://w3id.org/framester/data/framestercore/Probability">
        <owl:disjointWith rdf:resource="https://w3id.org/framester/data/framestercore/Sequence"/>
        <terms:description>This frame characterizes the likelihood that a Hypothetical_event will happen as a position on a scale of impossible to inevitable. The likelihood can expressed as numerical Odds or a metaphorical representation of the Position on a scale. There&apos;s a 20 % chance that you&apos;ll succeed. The odds that he&apos;ll actually do it are one in a million.</terms:description>
        <rdfs:label>Probability</rdfs:label>
    </owl:Class>
    


    <!-- https://w3id.org/framester/data/framestercore/Sequence -->

    <owl:Class rdf:about="https://w3id.org/framester/data/framestercore/Sequence">
        <rdfs:subClassOf>
            <owl:Restriction>
                <owl:onProperty rdf:resource="http://www.w3.org/ns/prov#wasGeneratedBy"/>
                <owl:someValuesFrom rdf:resource="https://w3id.org/framester/data/framestercore/Activity"/>
            </owl:Restriction>
        </rdfs:subClassOf>
        <owl:disjointWith rdf:resource="https://w3id.org/framester/data/framestersyn/Person"/>
        <terms:description>The words in this frame describe entities that occur in some temporally-ordered sequence. The entities thus have some sort of relation between them that might be described by the Relative_time frame. However, at this time, this frame has no Frame Relation with that frame (though this is still under discussion). Additionally, it should be noted that the words in this frame have a metaphorical link to the words in Shape. Describe in detail the sequence of steps taken during an emergency.</terms:description>
        <terms:description>The words in this frame describe entities that occur in some temporally-ordered sequence. The entities thus have some sort of relation between them that might be described by the Relative_time frame. However, at this time, this frame has no Frame Relation with that frame (though this is still under discussion). Additionally, it should be noted that the words in this frame have a metaphorical link to the words in Shape. Describe in detail the sequence of steps taken during an emergency. In this case this frame represent a sequence of temporally-ordered past events that have the same outcome</terms:description>
        <rdfs:comment>The words in this frame describe entities that occur in some temporally-ordered sequence. The entities thus have some sort of relation between them that might be described by the Relative_time frame. However, at this time, this frame has no Frame Relation with that frame (though this is still under discussion). Additionally, it should be noted that the words in this frame have a metaphorical link to the words in Shape. Describe in detail the sequence of steps taken during an emergency.</rdfs:comment>
        <rdfs:label>Sequence</rdfs:label>
    </owl:Class>
    


    <!-- https://w3id.org/framester/data/framestercore/Statement -->

    <owl:Class rdf:about="https://w3id.org/framester/data/framestercore/Statement">
        <rdfs:comment>a class for defining a statement of a perspective</rdfs:comment>
    </owl:Class>
    


    <!-- https://w3id.org/framester/data/framestersyn/Belief.n.1 -->

    <owl:Class rdf:about="https://w3id.org/framester/data/framestersyn/Belief.n.1">
        <rdfs:comment>A belief is a mental state or attitude where an individual holds something to be true or probable. Beliefs can range from factual assertions about the world to subjective evaluations, opinions, or attitudes about various matters. They form a fundamental part of human cognition and influence perception, decision-making, and behavior. Beliefs can be based on evidence, personal experience, cultural upbringing, social influences, or even intuition. They often shape an individual&apos;s worldview and can be deeply ingrained or subject to change over time based on new information or experiences.</rdfs:comment>
    </owl:Class>
    


    <!-- https://w3id.org/framester/data/framestersyn/Bettor.n.1 -->

    <owl:Class rdf:about="https://w3id.org/framester/data/framestersyn/Bettor.n.1">
        <rdfs:subClassOf rdf:resource="https://w3id.org/framester/data/framestercore/People"/>
        <terms:description>A class for a player involved in an Activity such as Sport Bets.</terms:description>
        <rdfs:label>Player</rdfs:label>
    </owl:Class>
    


    <!-- https://w3id.org/framester/data/framestersyn/Hiker.n.1 -->

    <owl:Class rdf:about="https://w3id.org/framester/data/framestersyn/Hiker.n.1">
        <rdfs:subClassOf rdf:resource="https://w3id.org/framester/data/framestercore/People"/>
        <terms:description>A class for people that go hiking or go for a walk.</terms:description>
        <rdfs:label>Hiker</rdfs:label>
    </owl:Class>
    


    <!-- https://w3id.org/framester/data/framestersyn/Person -->

    <owl:Class rdf:about="https://w3id.org/framester/data/framestersyn/Person">
        <rdfs:subClassOf rdf:resource="https://w3id.org/framester/data/framestercore/People"/>
    </owl:Class>
    


    <!-- https://w3id.org/framester/data/framestersyn/Player.n.1 -->

    <owl:Class rdf:about="https://w3id.org/framester/data/framestersyn/Player.n.1">
        <rdfs:subClassOf rdf:resource="https://w3id.org/framester/data/framestercore/People"/>
        <terms:description>A class for a player involved in an Activity such as a Lottery Draw.</terms:description>
        <terms:description>A class for a player such as a Baseball_Player engaged in a cognitive process during an Activity.</terms:description>
        <rdfs:label>Player</rdfs:label>
    </owl:Class>
    


    <!-- 
    ///////////////////////////////////////////////////////////////////////////////////////
    //
    // Individuals
    //
    ///////////////////////////////////////////////////////////////////////////////////////
     -->

    


    <!-- http://www.semanticweb.org/salva/ontologies/2024/1/Anecdotal_fallacy#Diet_works -->

    <owl:NamedIndividual rdf:about="http://www.semanticweb.org/salva/ontologies/2024/1/Anecdotal_fallacy#Diet_works">
        <rdf:type rdf:resource="https://w3id.org/framester/data/framestercore/Pattern"/>
    </owl:NamedIndividual>
    


    <!-- http://www.semanticweb.org/salva/ontologies/2024/1/Anecdotal_fallacy#Friend_lost_weight -->

    <owl:NamedIndividual rdf:about="http://www.semanticweb.org/salva/ontologies/2024/1/Anecdotal_fallacy#Friend_lost_weight">
        <rdf:type rdf:resource="https://w3id.org/framester/data/framestercore/Sequence"/>
        <cbo:creates rdf:resource="http://www.semanticweb.org/salva/ontologies/2024/1/Anecdotal_fallacy#Working_diet"/>
    </owl:NamedIndividual>
    


    <!-- http://www.semanticweb.org/salva/ontologies/2024/1/Anecdotal_fallacy#Losing_weight -->

    <owl:NamedIndividual rdf:about="http://www.semanticweb.org/salva/ontologies/2024/1/Anecdotal_fallacy#Losing_weight">
        <rdf:type rdf:resource="https://w3id.org/framester/data/framestercore/Activity"/>
        <term:includes rdf:resource="http://www.semanticweb.org/salva/ontologies/2024/1/Anecdotal_fallacy#Diet_works"/>
    </owl:NamedIndividual>
    


    <!-- http://www.semanticweb.org/salva/ontologies/2024/1/Anecdotal_fallacy#Subject -->

    <owl:NamedIndividual rdf:about="http://www.semanticweb.org/salva/ontologies/2024/1/Anecdotal_fallacy#Subject">
        <rdf:type rdf:resource="https://w3id.org/framester/data/framestersyn/Person"/>
        <term:isEngagedIn rdf:resource="http://www.semanticweb.org/salva/ontologies/2024/1/Anecdotal_fallacy#Losing_weight"/>
        <core:belief rdf:resource="http://www.semanticweb.org/salva/ontologies/2024/1/Anecdotal_fallacy#Friend_lost_weight"/>
    </owl:NamedIndividual>
    


    <!-- http://www.semanticweb.org/salva/ontologies/2024/1/Anecdotal_fallacy#Working_diet -->

    <owl:NamedIndividual rdf:about="http://www.semanticweb.org/salva/ontologies/2024/1/Anecdotal_fallacy#Working_diet">
        <rdf:type rdf:resource="https://w3id.org/framester/data/framestercore/PerceptionExperience"/>
        <cbo:involves rdf:resource="http://www.semanticweb.org/salva/ontologies/2024/1/Anecdotal_fallacy#friend_losing_weight"/>
    </owl:NamedIndividual>
    


    <!-- http://www.semanticweb.org/salva/ontologies/2024/1/Anecdotal_fallacy#friend_losing_weight -->

    <owl:NamedIndividual rdf:about="http://www.semanticweb.org/salva/ontologies/2024/1/Anecdotal_fallacy#friend_losing_weight">
        <rdf:type rdf:resource="https://w3id.org/framester/data/framestercore/ExperiencerObj"/>
        <term:producedObservation rdf:resource="http://www.semanticweb.org/salva/ontologies/2024/1/Anecdotal_fallacy#Diet_works"/>
    </owl:NamedIndividual>
    


    <!-- https://github.com/corrado877/CognitiveBiasOntologies/RecencyBias#Final_decision -->

    <owl:NamedIndividual rdf:about="https://github.com/corrado877/CognitiveBiasOntologies/RecencyBias#Final_decision">
        <rdf:type rdf:resource="https://github.com/corrado877/CognitiveBiasOntologies/blob/main/CognitiveBiasOntologies#Decision"/>
        <rdfs:comment>Influenced by the Recency bias the interviewer gives the job to the applicant.</rdfs:comment>
    </owl:NamedIndividual>
    


    <!-- https://github.com/corrado877/CognitiveBiasOntologies/RecencyBias#Interview_perception_experience -->

    <owl:NamedIndividual rdf:about="https://github.com/corrado877/CognitiveBiasOntologies/RecencyBias#Interview_perception_experience">
        <rdf:type rdf:resource="https://w3id.org/framester/data/framestercore/PerceptionExperience"/>
        <cbo:involves rdf:resource="https://github.com/corrado877/CognitiveBiasOntologies/RecencyBias#Memory_encoding"/>
        <rdfs:comment>The perception experience the individual is engaged in during the job interview.</rdfs:comment>
    </owl:NamedIndividual>
    


    <!-- https://github.com/corrado877/CognitiveBiasOntologies/RecencyBias#Interviewer -->

    <owl:NamedIndividual rdf:about="https://github.com/corrado877/CognitiveBiasOntologies/RecencyBias#Interviewer">
        <rdf:type rdf:resource="https://w3id.org/framester/data/framestercore/People"/>
        <term:isEngagedIn rdf:resource="https://github.com/corrado877/CognitiveBiasOntologies/RecencyBias#Interview_perception_experience"/>
        <term:isEngagedIn rdf:resource="https://w3id.org/framester/data/framestercore/Deciding"/>
        <newsreportingevent:owns rdf:resource="https://github.com/corrado877/CognitiveBiasOntologies/blob/main/Recency_bias/Recency_bias.owl#Memory"/>
        <rdfs:comment>The individual conducting the job interview.</rdfs:comment>
    </owl:NamedIndividual>
    


    <!-- https://github.com/corrado877/CognitiveBiasOntologies/RecencyBias#Memory_encoding -->

    <owl:NamedIndividual rdf:about="https://github.com/corrado877/CognitiveBiasOntologies/RecencyBias#Memory_encoding">
        <rdf:type rdf:resource="https://github.com/corrado877/CognitiveBiasOntologies/blob/main/CognitiveBiasOntologies#MemoryEncoding"/>
        <ontology:produces rdf:resource="https://github.com/corrado877/CognitiveBiasOntologies/blob/main/Recency_bias/Recency_bias.owl#Memory"/>
        <cbo:hasOutcome rdf:resource="https://github.com/corrado877/CognitiveBiasOntologies/blob/main/Recency_bias/Recency_bias.owl#Importance"/>
        <rdfs:comment>The process of encoding memory.</rdfs:comment>
    </owl:NamedIndividual>
    


    <!-- https://github.com/corrado877/CognitiveBiasOntologies/RecencyBias#Past_memory -->

    <owl:NamedIndividual rdf:about="https://github.com/corrado877/CognitiveBiasOntologies/RecencyBias#Past_memory">
        <rdf:type rdf:resource="https://github.com/corrado877/CognitiveBiasOntologies/blob/main/CognitiveBiasOntologies#PastMemory"/>
        <sequence:precedes rdf:resource="https://github.com/corrado877/CognitiveBiasOntologies/RecencyBias#Recent_memory"/>
        <rdfs:comment>The memory about the applicant not performing really well at the start of the interview.</rdfs:comment>
    </owl:NamedIndividual>
    


    <!-- https://github.com/corrado877/CognitiveBiasOntologies/RecencyBias#Recent_memory -->

    <owl:NamedIndividual rdf:about="https://github.com/corrado877/CognitiveBiasOntologies/RecencyBias#Recent_memory">
        <rdf:type rdf:resource="https://github.com/corrado877/CognitiveBiasOntologies/blob/main/CognitiveBiasOntologies#RecentMemory"/>
        <aos:affects rdf:resource="https://w3id.org/framester/data/framestercore/Deciding"/>
        <rdfs:comment>The memory about the applicant performing really well in the really last part of the job interview.</rdfs:comment>
    </owl:NamedIndividual>
    


    <!-- https://github.com/corrado877/CognitiveBiasOntologies/blob/main/Antropomorphism/Anthropomorphism.owl#Child -->

    <owl:NamedIndividual rdf:about="https://github.com/corrado877/CognitiveBiasOntologies/blob/main/Antropomorphism/Anthropomorphism.owl#Child">
        <rdf:type rdf:resource="https://w3id.org/framester/data/framestercore/People"/>
        <term:isEngagedIn rdf:resource="https://github.com/corrado877/CognitiveBiasOntologies/blob/main/Antropomorphism/Anthropomorphism.owl#Child_perception_experience"/>
        <rdfs:comment>The child experiencing anthropomorphism bias.</rdfs:comment>
    </owl:NamedIndividual>
    


    <!-- https://github.com/corrado877/CognitiveBiasOntologies/blob/main/Antropomorphism/Anthropomorphism.owl#Child_perception_experience -->

    <owl:NamedIndividual rdf:about="https://github.com/corrado877/CognitiveBiasOntologies/blob/main/Antropomorphism/Anthropomorphism.owl#Child_perception_experience">
        <rdf:type rdf:resource="https://w3id.org/framester/data/framestercore/PerceptionExperience"/>
        <cbo:involves rdf:resource="https://github.com/corrado877/CognitiveBiasOntologies/blob/main/Antropomorphism/Anthropomorphism.owl#Puppet"/>
    </owl:NamedIndividual>
    


    <!-- https://github.com/corrado877/CognitiveBiasOntologies/blob/main/Antropomorphism/Anthropomorphism.owl#Joy -->

    <owl:NamedIndividual rdf:about="https://github.com/corrado877/CognitiveBiasOntologies/blob/main/Antropomorphism/Anthropomorphism.owl#Joy">
        <rdf:type rdf:resource="https://github.com/corrado877/CognitiveBiasOntologies/blob/main/CognitiveBiasOntologies#HumanFeature"/>
        <term:isReflectionOn rdf:resource="https://github.com/corrado877/CognitiveBiasOntologies/blob/main/Antropomorphism/Anthropomorphism.owl#Child_perception_experience"/>
        <rdfs:comment>The emotion the child assumes Mr. Whiskers is feeling during playtime.</rdfs:comment>
    </owl:NamedIndividual>
    


    <!-- https://github.com/corrado877/CognitiveBiasOntologies/blob/main/Antropomorphism/Anthropomorphism.owl#Puppet -->

    <owl:NamedIndividual rdf:about="https://github.com/corrado877/CognitiveBiasOntologies/blob/main/Antropomorphism/Anthropomorphism.owl#Puppet">
        <rdf:type rdf:resource="http://www.ontologydesignpatterns.org/cp/owl/move.owl#PhysicalObject"/>
        <term:producedObservation rdf:resource="https://github.com/corrado877/CognitiveBiasOntologies/blob/main/Antropomorphism/Anthropomorphism.owl#Joy"/>
        <term:producedObservation rdf:resource="https://github.com/corrado877/CognitiveBiasOntologies/blob/main/Antropomorphism/Anthropomorphism.owl#Sadness"/>
        <rdfs:comment>Mr Whiskers, the child&apos;s puppet.</rdfs:comment>
    </owl:NamedIndividual>
    


    <!-- https://github.com/corrado877/CognitiveBiasOntologies/blob/main/Antropomorphism/Anthropomorphism.owl#Sadness -->

    <owl:NamedIndividual rdf:about="https://github.com/corrado877/CognitiveBiasOntologies/blob/main/Antropomorphism/Anthropomorphism.owl#Sadness">
        <rdf:type rdf:resource="https://github.com/corrado877/CognitiveBiasOntologies/blob/main/CognitiveBiasOntologies#HumanFeature"/>
        <term:isReflectionOn rdf:resource="https://github.com/corrado877/CognitiveBiasOntologies/blob/main/Antropomorphism/Anthropomorphism.owl#Child_perception_experience"/>
        <rdfs:comment>The emotion the child assumes Mr. Whiskers is feeling when left alone.</rdfs:comment>
    </owl:NamedIndividual>
    


    <!-- https://github.com/corrado877/CognitiveBiasOntologies/blob/main/Clustering_illusion#Consecutive_digits -->

    <owl:NamedIndividual rdf:about="https://github.com/corrado877/CognitiveBiasOntologies/blob/main/Clustering_illusion#Consecutive_digits">
        <rdf:type rdf:resource="https://w3id.org/framester/data/framestercore/ExperiencerObj"/>
        <term:producedObservation rdf:resource="https://github.com/corrado877/CognitiveBiasOntologies/blob/main/Clustering_illusion#Pattern_lottery_numbers"/>
    </owl:NamedIndividual>
    


    <!-- https://github.com/corrado877/CognitiveBiasOntologies/blob/main/Clustering_illusion#Illusion_pattern -->

    <owl:NamedIndividual rdf:about="https://github.com/corrado877/CognitiveBiasOntologies/blob/main/Clustering_illusion#Illusion_pattern">
        <rdf:type rdf:resource="https://dbpedia.org/page/Illusion"/>
        <cbo:involves rdf:resource="https://github.com/corrado877/CognitiveBiasOntologies/blob/main/Clustering_illusion#Consecutive_digits"/>
    </owl:NamedIndividual>
    


    <!-- https://github.com/corrado877/CognitiveBiasOntologies/blob/main/Clustering_illusion#Lottery -->

    <owl:NamedIndividual rdf:about="https://github.com/corrado877/CognitiveBiasOntologies/blob/main/Clustering_illusion#Lottery">
        <rdf:type rdf:resource="https://w3id.org/framester/data/framestercore/Activity"/>
        <cbo:creates rdf:resource="https://github.com/corrado877/CognitiveBiasOntologies/blob/main/Clustering_illusion#Illusion_pattern"/>
    </owl:NamedIndividual>
    


    <!-- https://github.com/corrado877/CognitiveBiasOntologies/blob/main/Clustering_illusion#Pattern_lottery_numbers -->

    <owl:NamedIndividual rdf:about="https://github.com/corrado877/CognitiveBiasOntologies/blob/main/Clustering_illusion#Pattern_lottery_numbers">
        <rdf:type rdf:resource="https://w3id.org/framester/data/framestercore/Pattern"/>
        <term:isReflectionOn rdf:resource="https://github.com/corrado877/CognitiveBiasOntologies/blob/main/Clustering_illusion#Lottery"/>
    </owl:NamedIndividual>
    


    <!-- https://github.com/corrado877/CognitiveBiasOntologies/blob/main/Clustering_illusion#Sarah -->

    <owl:NamedIndividual rdf:about="https://github.com/corrado877/CognitiveBiasOntologies/blob/main/Clustering_illusion#Sarah">
        <rdf:type rdf:resource="https://w3id.org/framester/data/framestersyn/Person"/>
    </owl:NamedIndividual>
    


    <!-- https://github.com/corrado877/CognitiveBiasOntologies/blob/main/GamblersFallacyOntology/GamblersFallacyOntology.owl#Black_Number -->

    <owl:NamedIndividual rdf:about="https://github.com/corrado877/CognitiveBiasOntologies/blob/main/GamblersFallacyOntology/GamblersFallacyOntology.owl#Black_Number">
        <rdf:type rdf:resource="https://github.com/corrado877/CognitiveBiasOntologies/blob/main/CognitiveBiasOntologies#OutcomeColorNumber"/>
        <rdfs:comment>The outcome of the next number draw or past number draws. Black numbers and red numbers have the same probability of being extracted.</rdfs:comment>
        <rdfs:label>Black Number</rdfs:label>
    </owl:NamedIndividual>
    


    <!-- https://github.com/corrado877/CognitiveBiasOntologies/blob/main/GamblersFallacyOntology/GamblersFallacyOntology.owl#Lottery_Draw -->

    <owl:NamedIndividual rdf:about="https://github.com/corrado877/CognitiveBiasOntologies/blob/main/GamblersFallacyOntology/GamblersFallacyOntology.owl#Lottery_Draw">
        <rdf:type rdf:resource="https://w3id.org/framester/data/framestercore/Activity"/>
        <rdfs:comment>an activity where numbers are of two different colours (black and red) and where only one number is extracted for each draw.</rdfs:comment>
        <rdfs:label>Lottery Draw</rdfs:label>
    </owl:NamedIndividual>
    


    <!-- https://github.com/corrado877/CognitiveBiasOntologies/blob/main/GamblersFallacyOntology/GamblersFallacyOntology.owl#Lottery_Player -->

    <owl:NamedIndividual rdf:about="https://github.com/corrado877/CognitiveBiasOntologies/blob/main/GamblersFallacyOntology/GamblersFallacyOntology.owl#Lottery_Player">
        <rdf:type rdf:resource="https://w3id.org/framester/data/framestersyn/Player.n.1"/>
        <core:belief rdf:resource="https://github.com/corrado877/CognitiveBiasOntologies/blob/main/GamblersFallacyOntology/GamblersFallacyOntology.owl#Past_Number_Draw_Series"/>
        <participation:isParticipantIn rdf:resource="https://github.com/corrado877/CognitiveBiasOntologies/blob/main/GamblersFallacyOntology/GamblersFallacyOntology.owl#Lottery_Draw"/>
        <cbo:hasBiasedOpinion rdf:resource="https://github.com/corrado877/CognitiveBiasOntologies/blob/main/GamblersFallacyOntology/GamblersFallacyOntology.owl#Next_Number_Draw"/>
        <rdfs:comment>An human being that participates as a player to a lottery draw.</rdfs:comment>
        <rdfs:label>Lottery Player</rdfs:label>
    </owl:NamedIndividual>
    


    <!-- https://github.com/corrado877/CognitiveBiasOntologies/blob/main/GamblersFallacyOntology/GamblersFallacyOntology.owl#Next_Number_Draw -->

    <owl:NamedIndividual rdf:about="https://github.com/corrado877/CognitiveBiasOntologies/blob/main/GamblersFallacyOntology/GamblersFallacyOntology.owl#Next_Number_Draw">
        <rdf:type rdf:resource="https://github.com/corrado877/CognitiveBiasOntologies/blob/main/CognitiveBiasOntologies#NextRandomOccurrence"/>
        <parameter:hasParameter rdf:resource="https://github.com/corrado877/CognitiveBiasOntologies/blob/main/GamblersFallacyOntology/GamblersFallacyOntology.owl#ProbabilityLevel"/>
        <partof:isPartOf rdf:resource="https://github.com/corrado877/CognitiveBiasOntologies/blob/main/GamblersFallacyOntology/GamblersFallacyOntology.owl#Lottery_Draw"/>
        <ontology:produces rdf:resource="https://github.com/corrado877/CognitiveBiasOntologies/blob/main/GamblersFallacyOntology/GamblersFallacyOntology.owl#Black_Number"/>
        <ontology:produces rdf:resource="https://github.com/corrado877/CognitiveBiasOntologies/blob/main/GamblersFallacyOntology/GamblersFallacyOntology.owl#Red_Number"/>
        <rdfs:comment>A number draw in a lottery is an event totally random where each number has the same probability of being extracted. In this case the outcome of the next number draw can be the same of the past number draws series  or not. If  in the past Number draws series the Outcome was Black and player believes that the probability of drawing a Black number in the next draw is lower so the next outcome will be Red, he/she is affected by the Gambler&apos;s Fallacy Bias. On the contrary, if he/she believes that the probability of drawing again a Black number is higher, he/she is affected by the Hot Outcome bias.</rdfs:comment>
        <rdfs:label>Number Draw</rdfs:label>
    </owl:NamedIndividual>
    


    <!-- https://github.com/corrado877/CognitiveBiasOntologies/blob/main/GamblersFallacyOntology/GamblersFallacyOntology.owl#Past_Number_Draw_Series -->

    <owl:NamedIndividual rdf:about="https://github.com/corrado877/CognitiveBiasOntologies/blob/main/GamblersFallacyOntology/GamblersFallacyOntology.owl#Past_Number_Draw_Series">
        <rdf:type rdf:resource="https://w3id.org/framester/data/framestercore/Sequence"/>
        <prov:wasGeneratedBy rdf:resource="https://github.com/corrado877/CognitiveBiasOntologies/blob/main/GamblersFallacyOntology/GamblersFallacyOntology.owl#Lottery_Draw"/>
        <cbo:hasOutcome rdf:resource="https://github.com/corrado877/CognitiveBiasOntologies/blob/main/GamblersFallacyOntology/GamblersFallacyOntology.owl#Black_Number"/>
        <rdfs:comment>An ordered sequence of past number draws that has the same outcome (black) will influence the judgment of the participant about the probability of the outcome in the next number draw.</rdfs:comment>
        <rdfs:label>Past Number Draw Series</rdfs:label>
    </owl:NamedIndividual>
    


    <!-- https://github.com/corrado877/CognitiveBiasOntologies/blob/main/GamblersFallacyOntology/GamblersFallacyOntology.owl#ProbabilityLevel -->

    <owl:NamedIndividual rdf:about="https://github.com/corrado877/CognitiveBiasOntologies/blob/main/GamblersFallacyOntology/GamblersFallacyOntology.owl#ProbabilityLevel">
        <rdf:type rdf:resource="https://w3id.org/framester/data/framestercore/Probability"/>
        <affectedBy:influencedBy rdf:resource="https://github.com/corrado877/CognitiveBiasOntologies/blob/main/GamblersFallacyOntology/GamblersFallacyOntology.owl#Past_Number_Draw_Series"/>
        <parameter:hasParameterDataValue>High</parameter:hasParameterDataValue>
        <parameter:hasParameterDataValue>Low</parameter:hasParameterDataValue>
        <rdfs:comment>The level of probability that the outcome of the next number draw will be red or black  can be higher or lower for the participant, depending on the outcomes of the previous number draws.</rdfs:comment>
        <rdfs:label>Probability Level</rdfs:label>
    </owl:NamedIndividual>
    


    <!-- https://github.com/corrado877/CognitiveBiasOntologies/blob/main/GamblersFallacyOntology/GamblersFallacyOntology.owl#Red_Number -->

    <owl:NamedIndividual rdf:about="https://github.com/corrado877/CognitiveBiasOntologies/blob/main/GamblersFallacyOntology/GamblersFallacyOntology.owl#Red_Number">
        <rdf:type rdf:resource="https://github.com/corrado877/CognitiveBiasOntologies/blob/main/CognitiveBiasOntologies#OutcomeColorNumber"/>
        <rdfs:comment>The outcome of the next number draw or past number draws. Black numbers and red numbers have the same probability of being extracted</rdfs:comment>
        <rdfs:label>Red Number</rdfs:label>
    </owl:NamedIndividual>
    


    <!-- https://github.com/corrado877/CognitiveBiasOntologies/blob/main/HotHandFallacyOntology/HotHandFallacyOntology.owl#Football_Team_Match_Bet -->

    <owl:NamedIndividual rdf:about="https://github.com/corrado877/CognitiveBiasOntologies/blob/main/HotHandFallacyOntology/HotHandFallacyOntology.owl#Football_Team_Match_Bet">
        <rdf:type rdf:resource="https://github.com/corrado877/CognitiveBiasOntologies/blob/main/CognitiveBiasOntologies#NextChance-BasedOccurence"/>
        <parameter:hasParameter rdf:resource="https://github.com/corrado877/CognitiveBiasOntologies/blob/main/HotHandFallacyOntology/HotHandFallacyOntology.owl#ProbabilityLevel"/>
        <cbo:producesOutcomeEffect rdf:resource="https://github.com/corrado877/CognitiveBiasOntologies/blob/main/HotHandFallacyOntology/HotHandFallacyOntology.owl#Winning_Bet"/>
        <rdfs:comment>An individual for the next chance-based occurence class such as a Footbal Team Match Bet where the probability level is not completely random and can be influenced by different external and/or internal elements of the game itself.</rdfs:comment>
        <rdfs:label>Football Team Match Bet</rdfs:label>
    </owl:NamedIndividual>
    


    <!-- https://github.com/corrado877/CognitiveBiasOntologies/blob/main/HotHandFallacyOntology/HotHandFallacyOntology.owl#Football_Team_Match_Bet_Series -->

    <owl:NamedIndividual rdf:about="https://github.com/corrado877/CognitiveBiasOntologies/blob/main/HotHandFallacyOntology/HotHandFallacyOntology.owl#Football_Team_Match_Bet_Series">
        <rdf:type rdf:resource="https://w3id.org/framester/data/framestercore/Sequence"/>
        <prov:wasGeneratedBy rdf:resource="https://github.com/corrado877/CognitiveBiasOntologies/blob/main/HotHandFallacyOntology/HotHandFallacyOntology.owl#Sport_Bets"/>
        <cbo:hasOutcomeEffect rdf:resource="https://github.com/corrado877/CognitiveBiasOntologies/blob/main/HotHandFallacyOntology/HotHandFallacyOntology.owl#Winning_Bet"/>
        <rdfs:comment>a sequence of past bets that have the same outcome effect, namely in this case a Winning Bet.</rdfs:comment>
        <rdfs:label>Football Team Match Bet Series</rdfs:label>
    </owl:NamedIndividual>
    


    <!-- https://github.com/corrado877/CognitiveBiasOntologies/blob/main/HotHandFallacyOntology/HotHandFallacyOntology.owl#ProbabilityLevel -->

    <owl:NamedIndividual rdf:about="https://github.com/corrado877/CognitiveBiasOntologies/blob/main/HotHandFallacyOntology/HotHandFallacyOntology.owl#ProbabilityLevel">
        <rdf:type rdf:resource="https://w3id.org/framester/data/framestercore/Probability"/>
        <affectedBy:influencedBy rdf:resource="https://github.com/corrado877/CognitiveBiasOntologies/blob/main/HotHandFallacyOntology/HotHandFallacyOntology.owl#Football_Team_Match_Bet_Series"/>
        <parameter:hasParameterDataValue>High</parameter:hasParameterDataValue>
        <parameter:hasParameterDataValue>Low</parameter:hasParameterDataValue>
        <rdfs:comment>The probability level that an event n the next futur, such a chance-based occurence, can have  a specific outcome effect. For example In the Hot Hand fallacy bias if the outcome of previous events series was a Victory then for the player the probability level that the next  event will be a Victory is higher. On the contrary in the opposite bias, the stock of luck, the player belevies that is less probable of winning again in the next event because the luck will be less.</rdfs:comment>
        <rdfs:label>ProbabiltyLevel</rdfs:label>
    </owl:NamedIndividual>
    


    <!-- https://github.com/corrado877/CognitiveBiasOntologies/blob/main/HotHandFallacyOntology/HotHandFallacyOntology.owl#Sport_Bets -->

    <owl:NamedIndividual rdf:about="https://github.com/corrado877/CognitiveBiasOntologies/blob/main/HotHandFallacyOntology/HotHandFallacyOntology.owl#Sport_Bets">
        <rdf:type rdf:resource="https://w3id.org/framester/data/framestercore/Activity"/>
        <participation:hasParticipant rdf:resource="https://github.com/corrado877/CognitiveBiasOntologies/blob/main/HotHandFallacyOntology/HotHandFallacyOntology.owl#Sport_Bettor"/>
        <partof:hasPart rdf:resource="https://github.com/corrado877/CognitiveBiasOntologies/blob/main/HotHandFallacyOntology/HotHandFallacyOntology.owl#Football_Team_Match_Bet"/>
        <rdfs:comment>An individual representing an Acitvity such as Sport Bets in which is involved a person such as a Bettor.</rdfs:comment>
        <rdfs:label>Sport Bets</rdfs:label>
    </owl:NamedIndividual>
    


    <!-- https://github.com/corrado877/CognitiveBiasOntologies/blob/main/HotHandFallacyOntology/HotHandFallacyOntology.owl#Sport_Bettor -->

    <owl:NamedIndividual rdf:about="https://github.com/corrado877/CognitiveBiasOntologies/blob/main/HotHandFallacyOntology/HotHandFallacyOntology.owl#Sport_Bettor">
        <rdf:type rdf:resource="https://w3id.org/framester/data/framestersyn/Bettor.n.1"/>
        <core:belief rdf:resource="https://github.com/corrado877/CognitiveBiasOntologies/blob/main/HotHandFallacyOntology/HotHandFallacyOntology.owl#Football_Team_Match_Bet_Series"/>
        <cbo:hasBiasedOpinion rdf:resource="https://github.com/corrado877/CognitiveBiasOntologies/blob/main/HotHandFallacyOntology/HotHandFallacyOntology.owl#Football_Team_Match_Bet"/>
        <rdfs:comment>A sport Bettor individual who is participating in an Activity such as Sport Bets</rdfs:comment>
        <rdfs:label>Sport Bettor</rdfs:label>
    </owl:NamedIndividual>
    


    <!-- https://github.com/corrado877/CognitiveBiasOntologies/blob/main/HotHandFallacyOntology/HotHandFallacyOntology.owl#Winning_Bet -->

    <owl:NamedIndividual rdf:about="https://github.com/corrado877/CognitiveBiasOntologies/blob/main/HotHandFallacyOntology/HotHandFallacyOntology.owl#Winning_Bet">
        <rdf:type rdf:resource="https://dbpedia.org/page/Success"/>
        <rdfs:comment>An individual representing the outcome effect of events such as a Football Team Match Bet. In this case a winning bet will be the effect of a winning match.</rdfs:comment>
        <rdfs:label>Winning Bet</rdfs:label>
    </owl:NamedIndividual>
    


    <!-- https://github.com/corrado877/CognitiveBiasOntologies/blob/main/Illusion_of_validity/Illusion_of_validity.owl#Biased_investement -->

    <owl:NamedIndividual rdf:about="https://github.com/corrado877/CognitiveBiasOntologies/blob/main/Illusion_of_validity/Illusion_of_validity.owl#Biased_investement">
        <rdf:type rdf:resource="http://www.ontology.se/odp/content/owl/Action.owl#Action"/>
        <Action:hasConsequence rdf:resource="https://github.com/corrado877/CognitiveBiasOntologies/blob/main/Illusion_of_validity/Illusion_of_validity.owl#Negative_outcome"/>
        <rdfs:comment>John continues  to invest based on his overconfident strategy, relying on the Illusion of Validity bias. Despite occasional market fluctuations, he attributes any success to his perceived expertise rather than considering the role of unpredictable factors or external influences.</rdfs:comment>
    </owl:NamedIndividual>
    


    <!-- https://github.com/corrado877/CognitiveBiasOntologies/blob/main/Illusion_of_validity/Illusion_of_validity.owl#Expert_investor -->

    <owl:NamedIndividual rdf:about="https://github.com/corrado877/CognitiveBiasOntologies/blob/main/Illusion_of_validity/Illusion_of_validity.owl#Expert_investor">
        <rdf:type rdf:resource="https://w3id.org/framester/data/framestercore/People"/>
        <term:isEngagedIn rdf:resource="https://github.com/corrado877/CognitiveBiasOntologies/blob/main/Illusion_of_validity/Illusion_of_validity.owl#Biased_investement"/>
        <term:isEngagedIn rdf:resource="https://github.com/corrado877/CognitiveBiasOntologies/blob/main/Illusion_of_validity/Illusion_of_validity.owl#Investor_predicting"/>
        <rdfs:comment>John, an hypotetical biased investor</rdfs:comment>
    </owl:NamedIndividual>
    


    <!-- https://github.com/corrado877/CognitiveBiasOntologies/blob/main/Illusion_of_validity/Illusion_of_validity.owl#Identicality_aspect -->

    <owl:NamedIndividual rdf:about="https://github.com/corrado877/CognitiveBiasOntologies/blob/main/Illusion_of_validity/Illusion_of_validity.owl#Identicality_aspect">
        <rdf:type rdf:resource="https://w3id.org/framester/data/framestercore/Identicality"/>
        <parameter:hasParameterDataValue rdf:datatype="http://www.w3.org/2001/XMLSchema#boolean">false</parameter:hasParameterDataValue>
    </owl:NamedIndividual>
    


    <!-- https://github.com/corrado877/CognitiveBiasOntologies/blob/main/Illusion_of_validity/Illusion_of_validity.owl#Investor_PerceivedValidity -->

    <owl:NamedIndividual rdf:about="https://github.com/corrado877/CognitiveBiasOntologies/blob/main/Illusion_of_validity/Illusion_of_validity.owl#Investor_PerceivedValidity">
        <rdf:type rdf:resource="https://github.com/corrado877/CognitiveBiasOntologies/blob/main/CognitiveBiasOntologies#PerceivedValidity"/>
        <participation1:isParticipantIn rdf:resource="https://github.com/corrado877/CognitiveBiasOntologies/blob/main/Illusion_of_validity/Illusion_of_validity.owl#Investor_predicting"/>
        <rdfs:comment>The investor&apos;s perception of validity in his previous knowledge and consequentially his predictions.</rdfs:comment>
    </owl:NamedIndividual>
    


    <!-- https://github.com/corrado877/CognitiveBiasOntologies/blob/main/Illusion_of_validity/Illusion_of_validity.owl#Investor_predicting -->

    <owl:NamedIndividual rdf:about="https://github.com/corrado877/CognitiveBiasOntologies/blob/main/Illusion_of_validity/Illusion_of_validity.owl#Investor_predicting">
        <rdf:type rdf:resource="https://w3id.org/framester/data/framestercore/Predicting"/>
        <ActivityPattern:produces rdf:resource="https://github.com/corrado877/CognitiveBiasOntologies/blob/main/Illusion_of_validity/Illusion_of_validity.owl#Positive_outcome"/>
        <rdfs:comment>The predicting process taken on by the investor to calculate the future possible outcome of his investement.</rdfs:comment>
    </owl:NamedIndividual>
    


    <!-- https://github.com/corrado877/CognitiveBiasOntologies/blob/main/Illusion_of_validity/Illusion_of_validity.owl#Investorship_knowledge -->

    <owl:NamedIndividual rdf:about="https://github.com/corrado877/CognitiveBiasOntologies/blob/main/Illusion_of_validity/Illusion_of_validity.owl#Investorship_knowledge">
        <rdf:type rdf:resource="https://dbpedia.org/resource/Knowledge"/>
        <aos:affects rdf:resource="https://github.com/corrado877/CognitiveBiasOntologies/blob/main/Illusion_of_validity/Illusion_of_validity.owl#Investor_PerceivedValidity"/>
        <rdfs:comment>The previous knowledge on the field which the investor owns and relies on.</rdfs:comment>
    </owl:NamedIndividual>
    


    <!-- https://github.com/corrado877/CognitiveBiasOntologies/blob/main/Illusion_of_validity/Illusion_of_validity.owl#Negative_outcome -->

    <owl:NamedIndividual rdf:about="https://github.com/corrado877/CognitiveBiasOntologies/blob/main/Illusion_of_validity/Illusion_of_validity.owl#Negative_outcome">
        <rdf:type rdf:resource="https://github.com/corrado877/CognitiveBiasOntologies/blob/main/CognitiveBiasOntologies#Outcome"/>
        <cbo:hasAttribute rdf:resource="https://github.com/corrado877/CognitiveBiasOntologies/blob/main/Illusion_of_validity/Illusion_of_validity.owl#Identicality_aspect"/>
        <rdfs:comment>The final result given by the investement choices.</rdfs:comment>
    </owl:NamedIndividual>
    


    <!-- https://github.com/corrado877/CognitiveBiasOntologies/blob/main/Illusion_of_validity/Illusion_of_validity.owl#Positive_outcome -->

    <owl:NamedIndividual rdf:about="https://github.com/corrado877/CognitiveBiasOntologies/blob/main/Illusion_of_validity/Illusion_of_validity.owl#Positive_outcome">
        <rdf:type rdf:resource="https://w3id.org/framester/data/framestercore/Expectation"/>
        <cbo:hasAttribute rdf:resource="https://github.com/corrado877/CognitiveBiasOntologies/blob/main/Illusion_of_validity/Illusion_of_validity.owl#Identicality_aspect"/>
        <rdfs:comment>The positive outcome John expects to get as result of his predicting process</rdfs:comment>
    </owl:NamedIndividual>
    


    <!-- https://github.com/corrado877/CognitiveBiasOntologies/blob/main/IllusoryOfCorrelationOntology/IllusoryOfCorrelationOntology.owl#Baseball_Match -->

    <owl:NamedIndividual rdf:about="https://github.com/corrado877/CognitiveBiasOntologies/blob/main/IllusoryOfCorrelationOntology/IllusoryOfCorrelationOntology.owl#Baseball_Match">
        <rdf:type rdf:resource="https://w3id.org/framester/data/framestercore/Activity"/>
        <term:includes rdf:resource="https://github.com/corrado877/CognitiveBiasOntologies/blob/main/IllusoryOfCorrelationOntology/IllusoryOfCorrelationOntology.owl#VariablesCorrelation"/>
        <rdfs:comment>An individual representing the activity in which the person&apos;s cognitive process of becoming aware takes place.</rdfs:comment>
        <rdfs:label>Baseball Match</rdfs:label>
    </owl:NamedIndividual>
    


    <!-- https://github.com/corrado877/CognitiveBiasOntologies/blob/main/IllusoryOfCorrelationOntology/IllusoryOfCorrelationOntology.owl#Baseball_Player -->

    <owl:NamedIndividual rdf:about="https://github.com/corrado877/CognitiveBiasOntologies/blob/main/IllusoryOfCorrelationOntology/IllusoryOfCorrelationOntology.owl#Baseball_Player">
        <rdf:type rdf:resource="https://w3id.org/framester/data/framestersyn/Player.n.1"/>
        <term:isEngagedIn rdf:resource="https://github.com/corrado877/CognitiveBiasOntologies/blob/main/IllusoryOfCorrelationOntology/IllusoryOfCorrelationOntology.owl#TrendAwareness"/>
        <rdfs:comment>an individual representing the type of person involved in the Illusory Correlation Bias, in this case a baseball player.</rdfs:comment>
        <rdfs:label>Baseball Player</rdfs:label>
    </owl:NamedIndividual>
    


    <!-- https://github.com/corrado877/CognitiveBiasOntologies/blob/main/IllusoryOfCorrelationOntology/IllusoryOfCorrelationOntology.owl#IllusionEffect -->

    <owl:NamedIndividual rdf:about="https://github.com/corrado877/CognitiveBiasOntologies/blob/main/IllusoryOfCorrelationOntology/IllusoryOfCorrelationOntology.owl#IllusionEffect">
        <rdf:type rdf:resource="https://dbpedia.org/page/Illusion"/>
        <rdfs:comment>An individual representing the conseguent illusory effect made by the correlation perceived between the variables.</rdfs:comment>
        <rdfs:label>Illusion Effect</rdfs:label>
    </owl:NamedIndividual>
    


    <!-- https://github.com/corrado877/CognitiveBiasOntologies/blob/main/IllusoryOfCorrelationOntology/IllusoryOfCorrelationOntology.owl#TrendAwareness -->

    <owl:NamedIndividual rdf:about="https://github.com/corrado877/CognitiveBiasOntologies/blob/main/IllusoryOfCorrelationOntology/IllusoryOfCorrelationOntology.owl#TrendAwareness">
        <rdf:type rdf:resource="https://w3id.org/framester/data/framestercore/BecomingAware"/>
        <term:inActivity rdf:resource="https://github.com/corrado877/CognitiveBiasOntologies/blob/main/IllusoryOfCorrelationOntology/IllusoryOfCorrelationOntology.owl#Baseball_Match"/>
        <cbo:isPerceivedAs rdf:resource="https://github.com/corrado877/CognitiveBiasOntologies/blob/main/IllusoryOfCorrelationOntology/IllusoryOfCorrelationOntology.owl#VariablesPattern"/>
        <rdfs:comment>An individual representing the person&apos;s cognitive process of becoming aware of something.</rdfs:comment>
        <rdfs:label>Trend Awareness</rdfs:label>
    </owl:NamedIndividual>
    


    <!-- https://github.com/corrado877/CognitiveBiasOntologies/blob/main/IllusoryOfCorrelationOntology/IllusoryOfCorrelationOntology.owl#VariablesCorrelation -->

    <owl:NamedIndividual rdf:about="https://github.com/corrado877/CognitiveBiasOntologies/blob/main/IllusoryOfCorrelationOntology/IllusoryOfCorrelationOntology.owl#VariablesCorrelation">
        <rdf:type rdf:resource="https://w3id.org/framester/data/framestercore/CognitiveConnection"/>
        <term:isReflectionOn rdf:resource="https://github.com/corrado877/CognitiveBiasOntologies/blob/main/IllusoryOfCorrelationOntology/IllusoryOfCorrelationOntology.owl#TrendAwareness"/>
        <cbo:hasEffect rdf:resource="https://github.com/corrado877/CognitiveBiasOntologies/blob/main/IllusoryOfCorrelationOntology/IllusoryOfCorrelationOntology.owl#IllusionEffect"/>
        <rdfs:comment>An individual representing the possible correlation between the variables of the pattern detected as part of a trend.</rdfs:comment>
        <rdfs:label>Variables Correlation</rdfs:label>
    </owl:NamedIndividual>
    


    <!-- https://github.com/corrado877/CognitiveBiasOntologies/blob/main/IllusoryOfCorrelationOntology/IllusoryOfCorrelationOntology.owl#VariablesPattern -->

    <owl:NamedIndividual rdf:about="https://github.com/corrado877/CognitiveBiasOntologies/blob/main/IllusoryOfCorrelationOntology/IllusoryOfCorrelationOntology.owl#VariablesPattern">
        <rdf:type rdf:resource="https://github.com/corrado877/CognitiveBiasOntologies/blob/main/CognitiveBiasOntologies#VariablesPattern"/>
        <partof:hasPart rdf:resource="https://github.com/corrado877/CognitiveBiasOntologies/blob/main/IllusoryOfCorrelationOntology/IllusoryOfCorrelationOntology.owl#Victories"/>
        <partof:hasPart rdf:resource="https://github.com/corrado877/CognitiveBiasOntologies/blob/main/IllusoryOfCorrelationOntology/IllusoryOfCorrelationOntology.owl#pair_of_socks"/>
    </owl:NamedIndividual>
    


    <!-- https://github.com/corrado877/CognitiveBiasOntologies/blob/main/IllusoryOfCorrelationOntology/IllusoryOfCorrelationOntology.owl#Victories -->

    <owl:NamedIndividual rdf:about="https://github.com/corrado877/CognitiveBiasOntologies/blob/main/IllusoryOfCorrelationOntology/IllusoryOfCorrelationOntology.owl#Victories">
        <rdf:type rdf:resource="https://github.com/corrado877/CognitiveBiasOntologies/blob/main/CognitiveBiasOntologies#VariableEntity2"/>
        <term:producedObservation rdf:resource="https://github.com/corrado877/CognitiveBiasOntologies/blob/main/IllusoryOfCorrelationOntology/IllusoryOfCorrelationOntology.owl#VariablesCorrelation"/>
        <rdfs:comment>One of the variables that occur together as part of a pattern.</rdfs:comment>
        <rdfs:label>Victories</rdfs:label>
    </owl:NamedIndividual>
    


    <!-- https://github.com/corrado877/CognitiveBiasOntologies/blob/main/IllusoryOfCorrelationOntology/IllusoryOfCorrelationOntology.owl#pair_of_socks -->

    <owl:NamedIndividual rdf:about="https://github.com/corrado877/CognitiveBiasOntologies/blob/main/IllusoryOfCorrelationOntology/IllusoryOfCorrelationOntology.owl#pair_of_socks">
        <rdf:type rdf:resource="https://github.com/corrado877/CognitiveBiasOntologies/blob/main/CognitiveBiasOntologies#VariableEntity1"/>
        <term:producedObservation rdf:resource="https://github.com/corrado877/CognitiveBiasOntologies/blob/main/IllusoryOfCorrelationOntology/IllusoryOfCorrelationOntology.owl#VariablesCorrelation"/>
        <rdfs:comment>One of the variables that occur together as part of a pattern.</rdfs:comment>
        <rdfs:label>Pair of socks</rdfs:label>
    </owl:NamedIndividual>
    


    <!-- https://github.com/corrado877/CognitiveBiasOntologies/blob/main/Insensitivity_to_sample_size#Game_bought -->

    <owl:NamedIndividual rdf:about="https://github.com/corrado877/CognitiveBiasOntologies/blob/main/Insensitivity_to_sample_size#Game_bought">
        <rdf:type rdf:resource="https://github.com/corrado877/CognitiveBiasOntologies/blob/main/CognitiveBiasOntologies#Decision"/>
        <affectedBy:influencedBy rdf:resource="https://github.com/corrado877/CognitiveBiasOntologies/blob/main/Insensitivity_to_sample_size#Game_review"/>
    </owl:NamedIndividual>
    


    <!-- https://github.com/corrado877/CognitiveBiasOntologies/blob/main/Insensitivity_to_sample_size#Game_choice -->

    <owl:NamedIndividual rdf:about="https://github.com/corrado877/CognitiveBiasOntologies/blob/main/Insensitivity_to_sample_size#Game_choice">
        <rdf:type rdf:resource="https://w3id.org/framester/data/framestercore/Assessing"/>
        <term:inActivity rdf:resource="https://github.com/corrado877/CognitiveBiasOntologies/blob/main/Insensitivity_to_sample_size#Game_bought"/>
    </owl:NamedIndividual>
    


    <!-- https://github.com/corrado877/CognitiveBiasOntologies/blob/main/Insensitivity_to_sample_size#Game_review -->

    <owl:NamedIndividual rdf:about="https://github.com/corrado877/CognitiveBiasOntologies/blob/main/Insensitivity_to_sample_size#Game_review">
        <rdf:type rdf:resource="https://github.com/corrado877/CognitiveBiasOntologies/blob/main/CognitiveBiasOntologies#Thing"/>
        <affectedBy:influencedBy rdf:resource="https://github.com/corrado877/CognitiveBiasOntologies/blob/main/Insensitivity_to_sample_size#Game_bought"/>
    </owl:NamedIndividual>
    


    <!-- https://github.com/corrado877/CognitiveBiasOntologies/blob/main/Insensitivity_to_sample_size#Me -->

    <owl:NamedIndividual rdf:about="https://github.com/corrado877/CognitiveBiasOntologies/blob/main/Insensitivity_to_sample_size#Me">
        <rdf:type rdf:resource="https://w3id.org/framester/data/framestersyn/Person"/>
        <term:isEngagedIn rdf:resource="https://github.com/corrado877/CognitiveBiasOntologies/blob/main/Insensitivity_to_sample_size#Game_choice"/>
        <cbo:have_knowledge rdf:resource="https://github.com/corrado877/CognitiveBiasOntologies/blob/main/Insensitivity_to_sample_size#Game_review"/>
    </owl:NamedIndividual>
    


    <!-- https://github.com/corrado877/CognitiveBiasOntologies/blob/main/Masked_man_fallacy/Masked_Man_Fallacy.owl#Heart_surgeon -->

    <owl:NamedIndividual rdf:about="https://github.com/corrado877/CognitiveBiasOntologies/blob/main/Masked_man_fallacy/Masked_Man_Fallacy.owl#Heart_surgeon">
        <rdf:type rdf:resource="https://github.com/corrado877/CognitiveBiasOntologies/blob/main/CognitiveBiasOntologies#KnownFeature"/>
        <rdfs:comment>The feature that characterizes John Smith (the entity) and is known to the biased individual.</rdfs:comment>
    </owl:NamedIndividual>
    


    <!-- https://github.com/corrado877/CognitiveBiasOntologies/blob/main/Masked_man_fallacy/Masked_Man_Fallacy.owl#Individual -->

    <owl:NamedIndividual rdf:about="https://github.com/corrado877/CognitiveBiasOntologies/blob/main/Masked_man_fallacy/Masked_Man_Fallacy.owl#Individual">
        <rdf:type rdf:resource="https://w3id.org/framester/data/framestercore/People"/>
        <term:isEngagedIn rdf:resource="https://github.com/corrado877/CognitiveBiasOntologies/blob/main/Masked_man_fallacy/Masked_Man_Fallacy.owl#Individual_perception_experience"/>
        <newsreportingevent:owns rdf:resource="https://github.com/corrado877/CognitiveBiasOntologies/blob/main/Masked_man_fallacy/Masked_Man_Fallacy.owl#Knowledge"/>
        <rdfs:comment>A masked man fallacy biased individual</rdfs:comment>
    </owl:NamedIndividual>
    


    <!-- https://github.com/corrado877/CognitiveBiasOntologies/blob/main/Masked_man_fallacy/Masked_Man_Fallacy.owl#Individual_perceived_validity -->

    <owl:NamedIndividual rdf:about="https://github.com/corrado877/CognitiveBiasOntologies/blob/main/Masked_man_fallacy/Masked_Man_Fallacy.owl#Individual_perceived_validity">
        <rdf:type rdf:resource="https://github.com/corrado877/CognitiveBiasOntologies/blob/main/CognitiveBiasOntologies#PerceivedValidity"/>
        <cbo:rejects rdf:resource="https://github.com/corrado877/CognitiveBiasOntologies/blob/main/Masked_man_fallacy/Masked_Man_Fallacy.owl#Jazz_saxophonist"/>
        <cbo:supports rdf:resource="https://github.com/corrado877/CognitiveBiasOntologies/blob/main/Masked_man_fallacy/Masked_Man_Fallacy.owl#Heart_surgeon"/>
        <rdfs:comment>The perceived validity towards the known feature at the expense of the unknown one</rdfs:comment>
    </owl:NamedIndividual>
    


    <!-- https://github.com/corrado877/CognitiveBiasOntologies/blob/main/Masked_man_fallacy/Masked_Man_Fallacy.owl#Individual_perception_experience -->

    <owl:NamedIndividual rdf:about="https://github.com/corrado877/CognitiveBiasOntologies/blob/main/Masked_man_fallacy/Masked_Man_Fallacy.owl#Individual_perception_experience">
        <rdf:type rdf:resource="https://w3id.org/framester/data/framestercore/PerceptionExperience"/>
        <ontology:produces rdf:resource="https://github.com/corrado877/CognitiveBiasOntologies/blob/main/Masked_man_fallacy/Masked_Man_Fallacy.owl#Individual_perceived_validity"/>
        <cbo:involves rdf:resource="https://github.com/corrado877/CognitiveBiasOntologies/blob/main/Masked_man_fallacy/Masked_Man_Fallacy.owl#John_Smith"/>
        <rdfs:comment>The perception experience of the individual when he discovers that the name of the musician is the same of a local surgeon.</rdfs:comment>
    </owl:NamedIndividual>
    


    <!-- https://github.com/corrado877/CognitiveBiasOntologies/blob/main/Masked_man_fallacy/Masked_Man_Fallacy.owl#Jazz_saxophonist -->

    <owl:NamedIndividual rdf:about="https://github.com/corrado877/CognitiveBiasOntologies/blob/main/Masked_man_fallacy/Masked_Man_Fallacy.owl#Jazz_saxophonist">
        <rdf:type rdf:resource="https://github.com/corrado877/CognitiveBiasOntologies/blob/main/CognitiveBiasOntologies#Un-knownFeature"/>
        <rdfs:comment>The feature that characterizes John Smith (the entity) and is un-known to the biased individual.</rdfs:comment>
    </owl:NamedIndividual>
    


    <!-- https://github.com/corrado877/CognitiveBiasOntologies/blob/main/Masked_man_fallacy/Masked_Man_Fallacy.owl#John_Smith -->

    <owl:NamedIndividual rdf:about="https://github.com/corrado877/CognitiveBiasOntologies/blob/main/Masked_man_fallacy/Masked_Man_Fallacy.owl#John_Smith">
        <rdf:type rdf:resource="https://dbpedia.org/resource/Entity"/>
        <cbo:hasFeature rdf:resource="https://github.com/corrado877/CognitiveBiasOntologies/blob/main/Masked_man_fallacy/Masked_Man_Fallacy.owl#Heart_surgeon"/>
        <cbo:hasFeature rdf:resource="https://github.com/corrado877/CognitiveBiasOntologies/blob/main/Masked_man_fallacy/Masked_Man_Fallacy.owl#Jazz_saxophonist"/>
        <rdfs:comment>John Smith, both a talented local surgeon and a great jazz saxophonist</rdfs:comment>
    </owl:NamedIndividual>
    


    <!-- https://github.com/corrado877/CognitiveBiasOntologies/blob/main/Masked_man_fallacy/Masked_Man_Fallacy.owl#Knowledge -->

    <owl:NamedIndividual rdf:about="https://github.com/corrado877/CognitiveBiasOntologies/blob/main/Masked_man_fallacy/Masked_Man_Fallacy.owl#Knowledge">
        <rdf:type rdf:resource="https://dbpedia.org/resource/Knowledge"/>
        <aos:affects rdf:resource="https://github.com/corrado877/CognitiveBiasOntologies/blob/main/Masked_man_fallacy/Masked_Man_Fallacy.owl#Individual_perception_experience"/>
        <rdfs:comment>The biased individual knowledge about an entity that leads him to associate to it only a particular intention.</rdfs:comment>
    </owl:NamedIndividual>
    


    <!-- https://github.com/corrado877/CognitiveBiasOntologies/blob/main/Neglect_of_probability_bias#Amelia -->

    <owl:NamedIndividual rdf:about="https://github.com/corrado877/CognitiveBiasOntologies/blob/main/Neglect_of_probability_bias#Amelia">
        <rdf:type rdf:resource="https://w3id.org/framester/data/framestersyn/Person"/>
        <term:isEngagedIn rdf:resource="https://github.com/corrado877/CognitiveBiasOntologies/blob/main/Neglect_of_probability_bias#Task_management"/>
        <cbo:have_knowledge rdf:resource="https://github.com/corrado877/CognitiveBiasOntologies/blob/main/Neglect_of_probability_bias#Deadline"/>
    </owl:NamedIndividual>
    


    <!-- https://github.com/corrado877/CognitiveBiasOntologies/blob/main/Neglect_of_probability_bias#Deadline -->

    <owl:NamedIndividual rdf:about="https://github.com/corrado877/CognitiveBiasOntologies/blob/main/Neglect_of_probability_bias#Deadline">
        <rdf:type rdf:resource="https://github.com/corrado877/CognitiveBiasOntologies/blob/main/CognitiveBiasOntologies#Thing"/>
        <cbo:decide rdf:resource="https://github.com/corrado877/CognitiveBiasOntologies/blob/main/Neglect_of_probability_bias#Procrastinate"/>
    </owl:NamedIndividual>
    


    <!-- https://github.com/corrado877/CognitiveBiasOntologies/blob/main/Neglect_of_probability_bias#Job_presentation -->

    <owl:NamedIndividual rdf:about="https://github.com/corrado877/CognitiveBiasOntologies/blob/main/Neglect_of_probability_bias#Job_presentation">
        <rdf:type rdf:resource="https://github.com/corrado877/CognitiveBiasOntologies/blob/main/CognitiveBiasOntologies#Decision"/>
        <affectedBy:influencedBy rdf:resource="https://github.com/corrado877/CognitiveBiasOntologies/blob/main/Neglect_of_probability_bias#Procrastinate"/>
    </owl:NamedIndividual>
    


    <!-- https://github.com/corrado877/CognitiveBiasOntologies/blob/main/Neglect_of_probability_bias#Procrastinate -->

    <owl:NamedIndividual rdf:about="https://github.com/corrado877/CognitiveBiasOntologies/blob/main/Neglect_of_probability_bias#Procrastinate">
        <rdf:type rdf:resource="https://github.com/corrado877/CognitiveBiasOntologies/blob/main/Neglect_of_probability_bias#Ignore"/>
    </owl:NamedIndividual>
    


    <!-- https://github.com/corrado877/CognitiveBiasOntologies/blob/main/Neglect_of_probability_bias#Task_management -->

    <owl:NamedIndividual rdf:about="https://github.com/corrado877/CognitiveBiasOntologies/blob/main/Neglect_of_probability_bias#Task_management">
        <rdf:type rdf:resource="https://w3id.org/framester/data/framestercore/Assessing"/>
        <term:inActivity rdf:resource="https://github.com/corrado877/CognitiveBiasOntologies/blob/main/Neglect_of_probability_bias#Job_presentation"/>
    </owl:NamedIndividual>
    


    <!-- https://github.com/corrado877/CognitiveBiasOntologies/blob/main/PareidoliaOntology/PareidoliaBiasOntology.owl#FacialShape -->

    <owl:NamedIndividual rdf:about="https://github.com/corrado877/CognitiveBiasOntologies/blob/main/PareidoliaOntology/PareidoliaBiasOntology.owl#FacialShape">
        <rdf:type rdf:resource="https://github.com/corrado877/CognitiveBiasOntologies/blob/main/CognitiveBiasOntologies#RecognizablePattern"/>
        <cbo:hasEffect rdf:resource="https://github.com/corrado877/CognitiveBiasOntologies/blob/main/PareidoliaOntology/PareidoliaBiasOntology.owl#FacialShapeIllusion"/>
        <cbo:hasInfluence rdf:resource="https://github.com/corrado877/CognitiveBiasOntologies/blob/main/PareidoliaOntology/PareidoliaBiasOntology.owl#SensorialPerception"/>
        <terms:description>this individual represent the pattern, such as familiar shapes of faces or objects, recognized by the mind and caused by the visual stimulus.</terms:description>
        <rdfs:label>Facial Shape</rdfs:label>
    </owl:NamedIndividual>
    


    <!-- https://github.com/corrado877/CognitiveBiasOntologies/blob/main/PareidoliaOntology/PareidoliaBiasOntology.owl#FacialShapeIllusion -->

    <owl:NamedIndividual rdf:about="https://github.com/corrado877/CognitiveBiasOntologies/blob/main/PareidoliaOntology/PareidoliaBiasOntology.owl#FacialShapeIllusion">
        <rdf:type rdf:resource="https://dbpedia.org/page/Illusion"/>
        <rdfs:comment>The actual illusion effect of seeing a facial shape in a weather-beaten tree trunk.</rdfs:comment>
        <rdfs:label>FacialShapeIllusion</rdfs:label>
    </owl:NamedIndividual>
    


    <!-- https://github.com/corrado877/CognitiveBiasOntologies/blob/main/PareidoliaOntology/PareidoliaBiasOntology.owl#RandomStimulus -->

    <owl:NamedIndividual rdf:about="https://github.com/corrado877/CognitiveBiasOntologies/blob/main/PareidoliaOntology/PareidoliaBiasOntology.owl#RandomStimulus">
        <rdf:type rdf:resource="https://github.com/corrado877/CognitiveBiasOntologies/blob/main/CognitiveBiasOntologies#AmbiguousStimulus"/>
        <rdfs:comment>An individual representing any kind of Random Stimulus that can involve a sensorial perception.</rdfs:comment>
        <rdfs:label>Random Stimulus</rdfs:label>
    </owl:NamedIndividual>
    


    <!-- https://github.com/corrado877/CognitiveBiasOntologies/blob/main/PareidoliaOntology/PareidoliaBiasOntology.owl#SensorialPerception -->

    <owl:NamedIndividual rdf:about="https://github.com/corrado877/CognitiveBiasOntologies/blob/main/PareidoliaOntology/PareidoliaBiasOntology.owl#SensorialPerception">
        <rdf:type rdf:resource="https://w3id.org/framester/data/framestercore/PerceptionExperience"/>
        <term:inActivity rdf:resource="https://github.com/corrado877/CognitiveBiasOntologies/blob/main/PareidoliaOntology/PareidoliaBiasOntology.owl#Walk"/>
        <rdfs:comment>The perception experience in which is involed a person: it can be sensorial but not only.</rdfs:comment>
        <rdfs:label>Sensorial Perception</rdfs:label>
    </owl:NamedIndividual>
    


    <!-- https://github.com/corrado877/CognitiveBiasOntologies/blob/main/PareidoliaOntology/PareidoliaBiasOntology.owl#Walk -->

    <owl:NamedIndividual rdf:about="https://github.com/corrado877/CognitiveBiasOntologies/blob/main/PareidoliaOntology/PareidoliaBiasOntology.owl#Walk">
        <rdf:type rdf:resource="https://w3id.org/framester/data/framestercore/Activity"/>
        <term:includes rdf:resource="https://github.com/corrado877/CognitiveBiasOntologies/blob/main/PareidoliaOntology/PareidoliaBiasOntology.owl#FacialShape"/>
        <cbo:involves rdf:resource="https://github.com/corrado877/CognitiveBiasOntologies/blob/main/PareidoliaOntology/PareidoliaBiasOntology.owl#RandomStimulus"/>
        <rdfs:comment>the activity  (such a walk in a park) ih which a perception experience is involved.</rdfs:comment>
        <rdfs:label>Walk</rdfs:label>
    </owl:NamedIndividual>
    


    <!-- https://github.com/corrado877/CognitiveBiasOntologies/blob/main/PareidoliaOntology/PareidoliaBiasOntology.owl#park_hiker -->

    <owl:NamedIndividual rdf:about="https://github.com/corrado877/CognitiveBiasOntologies/blob/main/PareidoliaOntology/PareidoliaBiasOntology.owl#park_hiker">
        <rdf:type rdf:resource="https://w3id.org/framester/data/framestersyn/Hiker.n.1"/>
        <term:isEngagedIn rdf:resource="https://github.com/corrado877/CognitiveBiasOntologies/blob/main/PareidoliaOntology/PareidoliaBiasOntology.owl#SensorialPerception"/>
        <cbo:isBiasedBy rdf:resource="https://github.com/corrado877/CognitiveBiasOntologies/blob/main/PareidoliaOntology/PareidoliaBiasOntology.owl#FacialShape"/>
        <rdfs:comment>an individual representing a person such as an hiker who goes for a walk in a park.</rdfs:comment>
        <rdfs:label>Park hiker</rdfs:label>
    </owl:NamedIndividual>
    


    <!-- https://github.com/corrado877/CognitiveBiasOntologies/blob/main/PareidoliaOntology/PareidoliaBiasOntology.owl#weather-beaten_tree_trunk -->

    <owl:NamedIndividual rdf:about="https://github.com/corrado877/CognitiveBiasOntologies/blob/main/PareidoliaOntology/PareidoliaBiasOntology.owl#weather-beaten_tree_trunk">
        <rdf:type rdf:resource="https://github.com/corrado877/CognitiveBiasOntologies/blob/main/CognitiveBiasOntologies#VisualStimulus"/>
        <term:producedObservation rdf:resource="https://github.com/corrado877/CognitiveBiasOntologies/blob/main/PareidoliaOntology/PareidoliaBiasOntology.owl#FacialShape"/>
        <rdfs:comment>A subclass individual  involving a visual stimuli  that can stimulate a process of association with familiar patterns such as facial shapes.</rdfs:comment>
        <rdfs:label>weather beaten tree trunk</rdfs:label>
    </owl:NamedIndividual>
    


    <!-- https://github.com/corrado877/CognitiveBiasOntologies/blob/main/Recency_bias/Recency_bias.owl#High_importance -->

    <owl:NamedIndividual rdf:about="https://github.com/corrado877/CognitiveBiasOntologies/blob/main/Recency_bias/Recency_bias.owl#High_importance">
        <rdf:type rdf:resource="https://github.com/corrado877/CognitiveBiasOntologies/blob/main/CognitiveBiasOntologies#HighImportance"/>
        <classification:classifies rdf:resource="https://github.com/corrado877/CognitiveBiasOntologies/RecencyBias#Recent_memory"/>
        <parameter:hasParameterDataValue>High</parameter:hasParameterDataValue>
    </owl:NamedIndividual>
    


    <!-- https://github.com/corrado877/CognitiveBiasOntologies/blob/main/Recency_bias/Recency_bias.owl#Importance -->

    <owl:NamedIndividual rdf:about="https://github.com/corrado877/CognitiveBiasOntologies/blob/main/Recency_bias/Recency_bias.owl#Importance">
        <rdf:type rdf:resource="https://w3id.org/framester/data/framestercore/Importance"/>
        <classification:classifies rdf:resource="https://github.com/corrado877/CognitiveBiasOntologies/RecencyBias#Past_memory"/>
        <classification:classifies rdf:resource="https://github.com/corrado877/CognitiveBiasOntologies/RecencyBias#Recent_memory"/>
        <rdfs:comment>The  value the interviewer gives to some memoryes at the expense of others</rdfs:comment>
    </owl:NamedIndividual>
    


    <!-- https://github.com/corrado877/CognitiveBiasOntologies/blob/main/Recency_bias/Recency_bias.owl#Low_importance -->

    <owl:NamedIndividual rdf:about="https://github.com/corrado877/CognitiveBiasOntologies/blob/main/Recency_bias/Recency_bias.owl#Low_importance">
        <rdf:type rdf:resource="https://github.com/corrado877/CognitiveBiasOntologies/blob/main/CognitiveBiasOntologies#LowImportance"/>
        <classification:classifies rdf:resource="https://github.com/corrado877/CognitiveBiasOntologies/RecencyBias#Past_memory"/>
        <parameter:hasParameterDataValue>Low</parameter:hasParameterDataValue>
    </owl:NamedIndividual>
    


    <!-- https://github.com/corrado877/CognitiveBiasOntologies/blob/main/Recency_bias/Recency_bias.owl#Memory -->

    <owl:NamedIndividual rdf:about="https://github.com/corrado877/CognitiveBiasOntologies/blob/main/Recency_bias/Recency_bias.owl#Memory">
        <rdf:type rdf:resource="https://w3id.org/framester/data/framestercore/Memory"/>
    </owl:NamedIndividual>
    


    <!-- https://github.com/corrado877/CognitiveBiasOntologies/tree/main/Bias%20Blind%20Spot#Biased_Opinion -->

    <owl:NamedIndividual rdf:about="https://github.com/corrado877/CognitiveBiasOntologies/tree/main/Bias%20Blind%20Spot#Biased_Opinion">
        <rdf:type rdf:resource="https://github.com/corrado877/CognitiveBiasOntologies/blob/main/CognitiveBiasOntologies#Bias"/>
    </owl:NamedIndividual>
    


    <!-- https://github.com/corrado877/CognitiveBiasOntologies/tree/main/Bias%20Blind%20Spot#Chris -->

    <owl:NamedIndividual rdf:about="https://github.com/corrado877/CognitiveBiasOntologies/tree/main/Bias%20Blind%20Spot#Chris">
        <rdf:type rdf:resource="https://w3id.org/framester/data/framestercore/People"/>
        <cbo:hasBiasedOpinion rdf:resource="https://github.com/corrado877/CognitiveBiasOntologies/tree/main/Bias%20Blind%20Spot#Biased_Opinion"/>
    </owl:NamedIndividual>
    


    <!-- https://github.com/corrado877/CognitiveBiasOntologies/tree/main/Bias%20Blind%20Spot#Decision -->

    <owl:NamedIndividual rdf:about="https://github.com/corrado877/CognitiveBiasOntologies/tree/main/Bias%20Blind%20Spot#Decision">
        <rdf:type rdf:resource="http://www.semanticweb.org/mein/ontologies/2024/2/untitled-ontology-17#MentalProperty"/>
        <cbo:hasOutcome rdf:resource="https://github.com/corrado877/CognitiveBiasOntologies/tree/main/Bias%20Blind%20Spot#Realization_of_bias"/>
        <affectedBy:affectedBy rdf:resource="https://github.com/corrado877/CognitiveBiasOntologies/tree/main/Bias%20Blind%20Spot#Superiority_of_one&apos;s_idea"/>
    </owl:NamedIndividual>
    


    <!-- https://github.com/corrado877/CognitiveBiasOntologies/tree/main/Bias%20Blind%20Spot#Emily -->

    <owl:NamedIndividual rdf:about="https://github.com/corrado877/CognitiveBiasOntologies/tree/main/Bias%20Blind%20Spot#Emily">
        <rdf:type rdf:resource="https://github.com/corrado877/CognitiveBiasOntologies/blob/main/CognitiveBiasOntologies#Agent"/>
        <term:isEngagedIn rdf:resource="https://github.com/corrado877/CognitiveBiasOntologies/tree/main/Bias%20Blind%20Spot#Decision"/>
        <core:belief rdf:resource="https://github.com/corrado877/CognitiveBiasOntologies/tree/main/Bias%20Blind%20Spot#Superiority_of_one&apos;s_idea"/>
        <cbo:focusesOn rdf:resource="https://github.com/corrado877/CognitiveBiasOntologies/tree/main/Bias%20Blind%20Spot#Superiority_of_one&apos;s_idea"/>
        <cbo:isUnawareOf rdf:resource="https://github.com/corrado877/CognitiveBiasOntologies/tree/main/Bias%20Blind%20Spot#Superiority_of_one&apos;s_idea"/>
    </owl:NamedIndividual>
    


    <!-- https://github.com/corrado877/CognitiveBiasOntologies/tree/main/Bias%20Blind%20Spot#Realization_of_bias -->

    <owl:NamedIndividual rdf:about="https://github.com/corrado877/CognitiveBiasOntologies/tree/main/Bias%20Blind%20Spot#Realization_of_bias">
        <rdf:type rdf:resource="https://github.com/corrado877/CognitiveBiasOntologies/blob/main/CognitiveBiasOntologies#Outcome"/>
        <affectedBy:affectedBy rdf:resource="https://github.com/corrado877/CognitiveBiasOntologies/tree/main/Bias%20Blind%20Spot#Superiority_of_one&apos;s_idea"/>
    </owl:NamedIndividual>
    


    <!-- https://github.com/corrado877/CognitiveBiasOntologies/tree/main/Bias%20Blind%20Spot#Superiority_of_one&apos;s_idea -->

    <owl:NamedIndividual rdf:about="https://github.com/corrado877/CognitiveBiasOntologies/tree/main/Bias%20Blind%20Spot#Superiority_of_one&apos;s_idea">
        <rdf:type rdf:resource="https://w3id.org/framester/data/framestersyn/Belief.n.1"/>
    </owl:NamedIndividual>
    


    <!-- https://github.com/corrado877/CognitiveBiasOntologies/tree/main/Confabulation%20Bias#Fabricated_story -->

    <owl:NamedIndividual rdf:about="https://github.com/corrado877/CognitiveBiasOntologies/tree/main/Confabulation%20Bias#Fabricated_story">
        <rdf:type rdf:resource="https://w3id.org/framester/data/framestercore/Evidence"/>
        <cbo:fillsMemoryGap rdf:resource="https://github.com/corrado877/CognitiveBiasOntologies/tree/main/Confabulation%20Bias#Memory_gap"/>
    </owl:NamedIndividual>
    


    <!-- https://github.com/corrado877/CognitiveBiasOntologies/tree/main/Confabulation%20Bias#Memory_gap -->

    <owl:NamedIndividual rdf:about="https://github.com/corrado877/CognitiveBiasOntologies/tree/main/Confabulation%20Bias#Memory_gap">
        <rdf:type rdf:resource="https://github.com/corrado877/CognitiveBiasOntologies/blob/main/CognitiveBiasOntologies#MemoryGap"/>
    </owl:NamedIndividual>
    


    <!-- https://github.com/corrado877/CognitiveBiasOntologies/tree/main/Confabulation%20Bias#Night_Out -->

    <owl:NamedIndividual rdf:about="https://github.com/corrado877/CognitiveBiasOntologies/tree/main/Confabulation%20Bias#Night_Out">
        <rdf:type rdf:resource="https://w3id.org/framester/data/framestercore/Event"/>
        <term:includes rdf:resource="https://github.com/corrado877/CognitiveBiasOntologies/tree/main/Confabulation%20Bias#Memory_gap"/>
        <cbo:hasOutcome rdf:resource="https://github.com/corrado877/CognitiveBiasOntologies/tree/main/Confabulation%20Bias#Telling_parents_fabricated_evidence"/>
    </owl:NamedIndividual>
    


    <!-- https://github.com/corrado877/CognitiveBiasOntologies/tree/main/Confabulation%20Bias#Sarah -->

    <owl:NamedIndividual rdf:about="https://github.com/corrado877/CognitiveBiasOntologies/tree/main/Confabulation%20Bias#Sarah">
        <rdf:type rdf:resource="https://w3id.org/framester/data/framestercore/People"/>
        <term:isEngagedIn rdf:resource="https://github.com/corrado877/CognitiveBiasOntologies/tree/main/Confabulation%20Bias#Night_Out"/>
        <ontology:produces rdf:resource="https://github.com/corrado877/CognitiveBiasOntologies/tree/main/Confabulation%20Bias#Fabricated_story"/>
        <cbo:hasMemoryGap rdf:resource="https://github.com/corrado877/CognitiveBiasOntologies/tree/main/Confabulation%20Bias#Memory_gap"/>
    </owl:NamedIndividual>
    


    <!-- https://github.com/corrado877/CognitiveBiasOntologies/tree/main/Confabulation%20Bias#Telling_parents_fabricated_evidence -->

    <owl:NamedIndividual rdf:about="https://github.com/corrado877/CognitiveBiasOntologies/tree/main/Confabulation%20Bias#Telling_parents_fabricated_evidence">
        <rdf:type rdf:resource="https://github.com/corrado877/CognitiveBiasOntologies/blob/main/CognitiveBiasOntologies#Outcome"/>
        <term:includes rdf:resource="https://github.com/corrado877/CognitiveBiasOntologies/tree/main/Confabulation%20Bias#Fabricated_story"/>
        <affectedBy:affectedBy rdf:resource="https://github.com/corrado877/CognitiveBiasOntologies/tree/main/Confabulation%20Bias#Telling_parents_fabricated_evidence"/>
    </owl:NamedIndividual>
    


    <!-- https://github.com/corrado877/CognitiveBiasOntologies/tree/main/Naive%20Cynicism#Chris -->

    <owl:NamedIndividual rdf:about="https://github.com/corrado877/CognitiveBiasOntologies/tree/main/Naive%20Cynicism#Chris">
        <rdf:type rdf:resource="https://w3id.org/framester/data/framestercore/People"/>
        <term:isEngagedIn rdf:resource="https://github.com/corrado877/CognitiveBiasOntologies/tree/main/Naive%20Cynicism#Current_challenge"/>
        <cbo:hasBiasedOpinion rdf:resource="https://github.com/corrado877/CognitiveBiasOntologies/tree/main/Naive%20Cynicism#Naive_Cynicism"/>
        <Naive_Cynicism:receives rdf:resource="https://github.com/corrado877/CognitiveBiasOntologies/tree/main/Naive%20Cynicism#Offered_help"/>
    </owl:NamedIndividual>
    


    <!-- https://github.com/corrado877/CognitiveBiasOntologies/tree/main/Naive%20Cynicism#Current_challenge -->

    <owl:NamedIndividual rdf:about="https://github.com/corrado877/CognitiveBiasOntologies/tree/main/Naive%20Cynicism#Current_challenge">
        <rdf:type rdf:resource="https://w3id.org/framester/data/framestercore/Event"/>
        <cbo:hasOutcome rdf:resource="https://github.com/corrado877/CognitiveBiasOntologies/tree/main/Naive%20Cynicism#Decline_of_offer"/>
        <cbo:involves rdf:resource="https://github.com/corrado877/CognitiveBiasOntologies/tree/main/Naive%20Cynicism#Offered_help"/>
    </owl:NamedIndividual>
    


    <!-- https://github.com/corrado877/CognitiveBiasOntologies/tree/main/Naive%20Cynicism#Decline_of_offer -->

    <owl:NamedIndividual rdf:about="https://github.com/corrado877/CognitiveBiasOntologies/tree/main/Naive%20Cynicism#Decline_of_offer">
        <rdf:type rdf:resource="https://github.com/corrado877/CognitiveBiasOntologies/blob/main/CognitiveBiasOntologies#Outcome"/>
    </owl:NamedIndividual>
    


    <!-- https://github.com/corrado877/CognitiveBiasOntologies/tree/main/Naive%20Cynicism#Naive_Cynicism -->

    <owl:NamedIndividual rdf:about="https://github.com/corrado877/CognitiveBiasOntologies/tree/main/Naive%20Cynicism#Naive_Cynicism">
        <rdf:type rdf:resource="https://github.com/corrado877/CognitiveBiasOntologies/blob/main/CognitiveBiasOntologies#Bias"/>
        <Naive_Cynicism:misjudges rdf:resource="https://github.com/corrado877/CognitiveBiasOntologies/tree/main/Naive%20Cynicism#Offered_help"/>
    </owl:NamedIndividual>
    


    <!-- https://github.com/corrado877/CognitiveBiasOntologies/tree/main/Naive%20Cynicism#Offered_help -->

    <owl:NamedIndividual rdf:about="https://github.com/corrado877/CognitiveBiasOntologies/tree/main/Naive%20Cynicism#Offered_help">
        <rdf:type rdf:resource="https://w3id.org/framester/data/framestercore/Assistance"/>
    </owl:NamedIndividual>
    


    <!-- https://github.com/corrado877/CognitiveBiasOntologies/tree/main/Naive%20Realism#Akio -->

    <owl:NamedIndividual rdf:about="https://github.com/corrado877/CognitiveBiasOntologies/tree/main/Naive%20Realism#Akio">
        <rdf:type rdf:resource="https://w3id.org/framester/data/framestercore/People"/>
        <cbo:hasPerspective rdf:resource="https://github.com/corrado877/CognitiveBiasOntologies/tree/main/Naive%20Realism#Target_Perspective"/>
    </owl:NamedIndividual>
    


    <!-- https://github.com/corrado877/CognitiveBiasOntologies/tree/main/Naive%20Realism#Maria -->

    <owl:NamedIndividual rdf:about="https://github.com/corrado877/CognitiveBiasOntologies/tree/main/Naive%20Realism#Maria">
        <rdf:type rdf:resource="https://github.com/corrado877/CognitiveBiasOntologies/blob/main/CognitiveBiasOntologies#Agent"/>
        <rdf:type rdf:resource="https://w3id.org/framester/data/framestercore/People"/>
        <core:belief rdf:resource="https://github.com/corrado877/CognitiveBiasOntologies/tree/main/Naive%20Realism#Underlying_belief_(cultural_universality)"/>
        <cbo:hasBias rdf:resource="https://github.com/corrado877/CognitiveBiasOntologies/tree/main/Naive%20Realism#Naive_Realism"/>
        <cbo:ignores rdf:resource="https://github.com/corrado877/CognitiveBiasOntologies/tree/main/Naive%20Realism#Target_Perspective"/>
    </owl:NamedIndividual>
    


    <!-- https://github.com/corrado877/CognitiveBiasOntologies/tree/main/Naive%20Realism#Naive_Realism -->

    <owl:NamedIndividual rdf:about="https://github.com/corrado877/CognitiveBiasOntologies/tree/main/Naive%20Realism#Naive_Realism">
        <rdf:type rdf:resource="https://github.com/corrado877/CognitiveBiasOntologies/blob/main/CognitiveBiasOntologies#Bias"/>
        <term:includes rdf:resource="https://github.com/corrado877/CognitiveBiasOntologies/tree/main/Naive%20Realism#Perception_of_own&apos;s_belief"/>
    </owl:NamedIndividual>
    


    <!-- https://github.com/corrado877/CognitiveBiasOntologies/tree/main/Naive%20Realism#Target_Perspective -->

    <owl:NamedIndividual rdf:about="https://github.com/corrado877/CognitiveBiasOntologies/tree/main/Naive%20Realism#Target_Perspective">
        <rdf:type rdf:resource="https://w3id.org/framester/data/framestercore/Statement"/>
    </owl:NamedIndividual>
    


    <!-- https://github.com/corrado877/CognitiveBiasOntologies/tree/main/Naive%20Realism#Perception_of_own&apos;s_belief -->

    <owl:NamedIndividual rdf:about="https://github.com/corrado877/CognitiveBiasOntologies/tree/main/Naive%20Realism#Perception_of_own&apos;s_belief">
        <rdf:type rdf:resource="https://w3id.org/framester/data/framestercore/PerceptionExperience"/>
    </owl:NamedIndividual>
    


    <!-- https://github.com/corrado877/CognitiveBiasOntologies/tree/main/Naive%20Realism#Underlying_belief_(cultural_universality) -->

    <owl:NamedIndividual rdf:about="https://github.com/corrado877/CognitiveBiasOntologies/tree/main/Naive%20Realism#Underlying_belief_(cultural_universality)">
        <rdf:type rdf:resource="https://w3id.org/framester/data/framestersyn/Belief.n.1"/>
        <affectedBy:affectedBy rdf:resource="https://github.com/corrado877/CognitiveBiasOntologies/tree/main/Naive%20Realism#Perception_of_own&apos;s_belief"/>
    </owl:NamedIndividual>
    


    <!-- https://w3id.org/framester/data/framestercore/Deciding -->

    <owl:NamedIndividual rdf:about="https://w3id.org/framester/data/framestercore/Deciding">
        <rdf:type rdf:resource="https://w3id.org/framester/data/framestercore/Deciding"/>
        <ontology:produces rdf:resource="https://github.com/corrado877/CognitiveBiasOntologies/RecencyBias#Final_decision"/>
    </owl:NamedIndividual>
    


    <!-- 
    ///////////////////////////////////////////////////////////////////////////////////////
    //
    // Annotations
    //
    ///////////////////////////////////////////////////////////////////////////////////////
     -->

    <rdf:Description rdf:about="https://w3id.org/framester/data/framestercore/Deciding">
        <rdfs:comment>The decision-making process carried out by the individual about the final outcome of the job interview.</rdfs:comment>
    </rdf:Description>
    


    <!-- 
    ///////////////////////////////////////////////////////////////////////////////////////
    //
    // General axioms
    //
    ///////////////////////////////////////////////////////////////////////////////////////
     -->

    <rdf:Description>
        <rdf:type rdf:resource="http://www.w3.org/2002/07/owl#AllDisjointClasses"/>
        <owl:members rdf:parseType="Collection">
            <rdf:Description rdf:about="https://dbpedia.org/page/Illusion"/>
            <rdf:Description rdf:about="https://github.com/corrado877/CognitiveBiasOntologies/blob/main/CognitiveBiasOntologies#AmbiguousStimulus"/>
            <rdf:Description rdf:about="https://w3id.org/framester/data/framestercore/Activity"/>
            <rdf:Description rdf:about="https://w3id.org/framester/data/framestercore/Pattern"/>
            <rdf:Description rdf:about="https://w3id.org/framester/data/framestercore/People"/>
            <rdf:Description rdf:about="https://w3id.org/framester/data/framestercore/PerceptionExperience"/>
        </owl:members>
    </rdf:Description>
</rdf:RDF>



<!-- Generated by the OWL API (version 4.5.26.2023-07-17T20:34:13Z) https://github.com/owlcs/owlapi -->

