<?xml version="1.0"?>
<rdf:RDF xmlns="https://github.com/corrado877/CognitiveBiasOntologies/blob/main/HotHandFallacyOntology/HotHandFallacyOntology.owl"
     xml:base="https://github.com/corrado877/CognitiveBiasOntologies/blob/main/HotHandFallacyOntology/HotHandFallacyOntology.owl"
     xmlns:fs="https://w3id.org/framester/data/framestercore/"
     xmlns:aff="https://w3id.org/affectedBy#"
     xmlns:cco="http://purl.org/ontology/cco/core#"
     xmlns:dbr="https://dbpedia.org/resource/"
     xmlns:owl="http://www.w3.org/2002/07/owl#"
     xmlns:rdf="http://www.w3.org/1999/02/22-rdf-syntax-ns#"
     xmlns:xml="http://www.w3.org/XML/1998/namespace"
     xmlns:xsd="http://www.w3.org/2001/XMLSchema#"
     xmlns:foaf="http://xmlns.com/foaf/0.1/"
     xmlns:prov="http://www.w3.org/ns/prov#"
     xmlns:rdfs="http://www.w3.org/2000/01/rdf-schema#"
     xmlns:terms="http://purl.org/dc/terms/"
     xmlns:partof="http://www.ontologydesignpatterns.org/cp/owl/partof.owl#"
     xmlns:parameter="http://www.ontologydesignpatterns.org/cp/owl/parameter.owl#"
     xmlns:participation="http://www.ontologydesignpatterns.org/cp/owl/participation.owl#"
     xmlns:activitypattern="http://descartes-core.org/ontologies/activities/1.0/ActivityPattern.owl#"
     xmlns:cpannotationschema="http://www.ontologydesignpatterns.org/schemas/cpannotationschema.owl#"
     xmlns:HotHandFallacyOntology="https://github.com/corrado877/CognitiveBiasOntologies/blob/main/HotHandFallacyOntology/HotHandFallacyOntology.owl#">
    <owl:Ontology rdf:about="https://github.com/corrado877/CognitiveBiasOntologies/blob/main/HotHandFallacyOntology/HotHandFallacyOntology.owl">
        <terms:created>February 2024</terms:created>
        <terms:creator>Corrado Consiglio</terms:creator>
        <terms:description>The Hot Hand Fallacy module of the Cognitive Bias Ontology</terms:description>
        <terms:title>Hot Hand Fallacy Bias Ontology</terms:title>
        <cpannotationschema:hasComponent rdf:resource="http://ontologydesignpatterns.org/wiki/Submissions:AffectedBy"/>
        <cpannotationschema:hasComponent rdf:resource="http://ontologydesignpatterns.org/wiki/Submissions:An_Ontology_Design_Pattern_for_Activity_Reasoning"/>
        <cpannotationschema:hasComponent rdf:resource="http://ontologydesignpatterns.org/wiki/Submissions:Parameter"/>
        <cpannotationschema:hasComponent rdf:resource="http://ontologydesignpatterns.org/wiki/Submissions:PartOf"/>
        <cpannotationschema:hasComponent rdf:resource="http://ontologydesignpatterns.org/wiki/Submissions:Participation"/>
        <cpannotationschema:hasComponent rdf:resource="http://ontologydesignpatterns.org/wiki/Submissions:Provenance"/>
        <cpannotationschema:hasComponent rdf:resource="http://purl.org/ontology/cco/20100926/cognitivecharacteristics.html"/>
        <cpannotationschema:hasComponent rdf:resource="http://xmlns.com/foaf/spec/"/>
        <cpannotationschema:hasComponent rdf:resource="https://www.dbpedia.org/about/"/>
        <cpannotationschema:scenarios>Sports Betting: A sports bettor assumes that a team that has won several games in a row is more likely to win the next one, overlooking factors like team performance and matchups.</cpannotationschema:scenarios>
        <rdfs:comment xml:lang="en">The Hot Hand Fallacy Bias, also known as the Hot Hand Fallacy, is a cognitive bias that leads people to believe that a series of successful outcomes in a random or chance-based process is more likely to continue in the short term. In other words, individuals tend to think that if they or someone else has experienced a streak of wins or successes, they are more likely to keep winning or succeeding in the near future. This bias can be observed in various contexts, such as sports, gambling, or even everyday decision-making.</rdfs:comment>
    </owl:Ontology>
    


    <!-- 
    ///////////////////////////////////////////////////////////////////////////////////////
    //
    // Annotation properties
    //
    ///////////////////////////////////////////////////////////////////////////////////////
     -->

    


    <!-- http://purl.org/dc/terms/created -->

    <owl:AnnotationProperty rdf:about="http://purl.org/dc/terms/created"/>
    


    <!-- http://purl.org/dc/terms/creator -->

    <owl:AnnotationProperty rdf:about="http://purl.org/dc/terms/creator"/>
    


    <!-- http://purl.org/dc/terms/description -->

    <owl:AnnotationProperty rdf:about="http://purl.org/dc/terms/description"/>
    


    <!-- http://purl.org/dc/terms/title -->

    <owl:AnnotationProperty rdf:about="http://purl.org/dc/terms/title"/>
    


    <!-- http://www.ontologydesignpatterns.org/schemas/cpannotationschema.owl#hasComponent -->

    <owl:AnnotationProperty rdf:about="http://www.ontologydesignpatterns.org/schemas/cpannotationschema.owl#hasComponent"/>
    


    <!-- http://www.ontologydesignpatterns.org/schemas/cpannotationschema.owl#scenarios -->

    <owl:AnnotationProperty rdf:about="http://www.ontologydesignpatterns.org/schemas/cpannotationschema.owl#scenarios"/>
    


    <!-- 
    ///////////////////////////////////////////////////////////////////////////////////////
    //
    // Object Properties
    //
    ///////////////////////////////////////////////////////////////////////////////////////
     -->

    


    <!-- http://purl.org/ontology/cco/core#belief -->

    <owl:ObjectProperty rdf:about="http://purl.org/ontology/cco/core#belief">
        <rdfs:domain rdf:resource="https://w3id.org/framester/data/framestercore/People"/>
        <rdfs:range rdf:resource="https://w3id.org/framester/data/framestercore/Sequence"/>
    </owl:ObjectProperty>
    


    <!-- http://www.ontologydesignpatterns.org/cp/owl/parameter.owl#hasParameter -->

    <owl:ObjectProperty rdf:about="http://www.ontologydesignpatterns.org/cp/owl/parameter.owl#hasParameter">
        <owl:inverseOf rdf:resource="http://www.ontologydesignpatterns.org/cp/owl/parameter.owl#isParameterFor"/>
        <rdfs:domain rdf:resource="https://w3id.org/framester/data/framestercore/Event"/>
        <rdfs:range rdf:resource="https://w3id.org/framester/data/framestercore/Probability"/>
    </owl:ObjectProperty>
    


    <!-- http://www.ontologydesignpatterns.org/cp/owl/parameter.owl#isParameterFor -->

    <owl:ObjectProperty rdf:about="http://www.ontologydesignpatterns.org/cp/owl/parameter.owl#isParameterFor">
        <rdfs:domain rdf:resource="https://w3id.org/framester/data/framestercore/Probability"/>
    </owl:ObjectProperty>
    


    <!-- http://www.ontologydesignpatterns.org/cp/owl/participation.owl#hasParticipant -->

    <owl:ObjectProperty rdf:about="http://www.ontologydesignpatterns.org/cp/owl/participation.owl#hasParticipant">
        <owl:inverseOf rdf:resource="http://www.ontologydesignpatterns.org/cp/owl/participation.owl#isParticipantIn"/>
        <rdfs:domain rdf:resource="https://w3id.org/framester/data/framestercore/Activity"/>
        <rdfs:range rdf:resource="https://w3id.org/framester/data/framestercore/People"/>
    </owl:ObjectProperty>
    


    <!-- http://www.ontologydesignpatterns.org/cp/owl/participation.owl#isParticipantIn -->

    <owl:ObjectProperty rdf:about="http://www.ontologydesignpatterns.org/cp/owl/participation.owl#isParticipantIn"/>
    


    <!-- http://www.ontologydesignpatterns.org/cp/owl/partof.owl#hasPart -->

    <owl:ObjectProperty rdf:about="http://www.ontologydesignpatterns.org/cp/owl/partof.owl#hasPart">
        <owl:inverseOf rdf:resource="http://www.ontologydesignpatterns.org/cp/owl/partof.owl#isPartOf"/>
        <rdfs:domain rdf:resource="https://w3id.org/framester/data/framestercore/Activity"/>
        <rdfs:range rdf:resource="https://w3id.org/framester/data/framestercore/Event"/>
    </owl:ObjectProperty>
    


    <!-- http://www.ontologydesignpatterns.org/cp/owl/partof.owl#isPartOf -->

    <owl:ObjectProperty rdf:about="http://www.ontologydesignpatterns.org/cp/owl/partof.owl#isPartOf"/>
    


    <!-- http://www.w3.org/ns/prov#wasGeneratedBy -->

    <owl:ObjectProperty rdf:about="http://www.w3.org/ns/prov#wasGeneratedBy">
        <rdfs:domain rdf:resource="https://w3id.org/framester/data/framestercore/Sequence"/>
        <rdfs:range rdf:resource="https://w3id.org/framester/data/framestercore/Activity"/>
    </owl:ObjectProperty>
    


    <!-- https://github.com/corrado877/CognitiveBiasOntologies/blob/main/HotHandFallacyOntology/HotHandFallacyOntology.owl#hasBiasedOpinion -->

    <owl:ObjectProperty rdf:about="https://github.com/corrado877/CognitiveBiasOntologies/blob/main/HotHandFallacyOntology/HotHandFallacyOntology.owl#hasBiasedOpinion">
        <rdfs:domain rdf:resource="https://w3id.org/framester/data/framestercore/People"/>
        <rdfs:range rdf:resource="https://w3id.org/framester/data/framestercore/Event"/>
        <rdfs:comment>a property connecting a Person who has a biased opinion about the possible outcome of an Event such as a Random or Chance-based Occurrence</rdfs:comment>
    </owl:ObjectProperty>
    


    <!-- https://github.com/corrado877/CognitiveBiasOntologies/blob/main/HotHandFallacyOntology/HotHandFallacyOntology.owl#hasInfluence -->

    <owl:ObjectProperty rdf:about="https://github.com/corrado877/CognitiveBiasOntologies/blob/main/HotHandFallacyOntology/HotHandFallacyOntology.owl#hasInfluence">
        <owl:inverseOf rdf:resource="https://w3id.org/affectedBy#influencedBy"/>
        <rdfs:domain rdf:resource="https://w3id.org/framester/data/framestercore/Sequence"/>
        <rdfs:range rdf:resource="https://w3id.org/framester/data/framestercore/Probability"/>
    </owl:ObjectProperty>
    


    <!-- https://github.com/corrado877/CognitiveBiasOntologies/blob/main/HotHandFallacyOntology/HotHandFallacyOntology.owl#hasOutcomeEffect -->

    <owl:ObjectProperty rdf:about="https://github.com/corrado877/CognitiveBiasOntologies/blob/main/HotHandFallacyOntology/HotHandFallacyOntology.owl#hasOutcomeEffect">
        <owl:inverseOf rdf:resource="https://github.com/corrado877/CognitiveBiasOntologies/blob/main/HotHandFallacyOntology/HotHandFallacyOntology.owl#isOutcomeEffectOf"/>
        <rdfs:domain rdf:resource="https://w3id.org/framester/data/framestercore/Sequence"/>
        <rdfs:range rdf:resource="https://dbpedia.org/page/Success"/>
        <rdfs:comment>A property linking a series of events which Outcome brings to the same effect</rdfs:comment>
    </owl:ObjectProperty>
    


    <!-- https://github.com/corrado877/CognitiveBiasOntologies/blob/main/HotHandFallacyOntology/HotHandFallacyOntology.owl#isOutcomeEffectOf -->

    <owl:ObjectProperty rdf:about="https://github.com/corrado877/CognitiveBiasOntologies/blob/main/HotHandFallacyOntology/HotHandFallacyOntology.owl#isOutcomeEffectOf">
        <rdfs:comment>inverse property of HasOutcomeEffect</rdfs:comment>
    </owl:ObjectProperty>
    


    <!-- https://github.com/corrado877/CognitiveBiasOntologies/blob/main/HotHandFallacyOntology/HotHandFallacyOntology.owl#isProducedEffectBy -->

    <owl:ObjectProperty rdf:about="https://github.com/corrado877/CognitiveBiasOntologies/blob/main/HotHandFallacyOntology/HotHandFallacyOntology.owl#isProducedEffectBy">
        <owl:inverseOf rdf:resource="https://github.com/corrado877/CognitiveBiasOntologies/blob/main/HotHandFallacyOntology/HotHandFallacyOntology.owl#producesOutcomeEffect"/>
        <rdfs:comment>inverse property of producesOutcomeEffect</rdfs:comment>
    </owl:ObjectProperty>
    


    <!-- https://github.com/corrado877/CognitiveBiasOntologies/blob/main/HotHandFallacyOntology/HotHandFallacyOntology.owl#producesOutcomeEffect -->

    <owl:ObjectProperty rdf:about="https://github.com/corrado877/CognitiveBiasOntologies/blob/main/HotHandFallacyOntology/HotHandFallacyOntology.owl#producesOutcomeEffect">
        <rdfs:domain rdf:resource="https://w3id.org/framester/data/framestercore/Event"/>
        <rdfs:range rdf:resource="https://dbpedia.org/page/Success"/>
        <rdfs:comment>a property linking an event which Outcome will produce an effect</rdfs:comment>
    </owl:ObjectProperty>
    


    <!-- https://w3id.org/affectedBy#influencedBy -->

    <owl:ObjectProperty rdf:about="https://w3id.org/affectedBy#influencedBy">
        <rdfs:domain rdf:resource="https://w3id.org/framester/data/framestercore/Probability"/>
    </owl:ObjectProperty>
    


    <!-- 
    ///////////////////////////////////////////////////////////////////////////////////////
    //
    // Data properties
    //
    ///////////////////////////////////////////////////////////////////////////////////////
     -->

    


    <!-- http://www.ontologydesignpatterns.org/cp/owl/parameter.owl#hasParameterDataValue -->

    <owl:DatatypeProperty rdf:about="http://www.ontologydesignpatterns.org/cp/owl/parameter.owl#hasParameterDataValue">
        <rdfs:domain rdf:resource="https://w3id.org/framester/data/framestercore/Probability"/>
        <rdfs:range rdf:resource="http://www.w3.org/2001/XMLSchema#string"/>
    </owl:DatatypeProperty>
    


    <!-- 
    ///////////////////////////////////////////////////////////////////////////////////////
    //
    // Classes
    //
    ///////////////////////////////////////////////////////////////////////////////////////
     -->

    


    <!-- https://dbpedia.org/page/Success -->

    <owl:Class rdf:about="https://dbpedia.org/page/Success">
        <owl:disjointWith rdf:resource="https://w3id.org/framester/data/framestercore/Activity"/>
        <owl:disjointWith rdf:resource="https://w3id.org/framester/data/framestercore/Event"/>
        <owl:disjointWith rdf:resource="https://w3id.org/framester/data/framestercore/People"/>
        <owl:disjointWith rdf:resource="https://w3id.org/framester/data/framestercore/Probability"/>
        <owl:disjointWith rdf:resource="https://w3id.org/framester/data/framestercore/Sequence"/>
        <rdfs:comment>Success is the state or condition of meeting a defined range of expectations. It may be viewed as the opposite of failure. The criteria for success depend on context and may be relative to a particular observer or belief system. One person might consider a success what another person considers a failure, particularly in cases of direct competition or a zero-sum game. Similarly, the degree of success or failure in a situation may be differently viewed by distinct observers or participants, such that a situation that one considers to be a success, another might consider to be a failure, a qualified success or a neutral situation. For example, a film that is a commercial failure or even a box-office bomb can go on to receive a cult following, with the initial lack of commercial success even.</rdfs:comment>
        <rdfs:label>Success</rdfs:label>
    </owl:Class>
    


    <!-- https://github.com/corrado877/CognitiveBiasOntologies/blob/main/HotHandFallacyOntology/HotHandFallacyOntology.owl#FutureEvent -->

    <owl:Class rdf:about="https://github.com/corrado877/CognitiveBiasOntologies/blob/main/HotHandFallacyOntology/HotHandFallacyOntology.owl#FutureEvent">
        <rdfs:subClassOf rdf:resource="https://w3id.org/framester/data/framestercore/Event"/>
        <rdfs:comment>This class represent an event that will happen in the next future.</rdfs:comment>
        <rdfs:label>FutureEvent</rdfs:label>
    </owl:Class>
    


    <!-- https://github.com/corrado877/CognitiveBiasOntologies/blob/main/HotHandFallacyOntology/HotHandFallacyOntology.owl#NextChance-BasedOccurence -->

    <owl:Class rdf:about="https://github.com/corrado877/CognitiveBiasOntologies/blob/main/HotHandFallacyOntology/HotHandFallacyOntology.owl#NextChance-BasedOccurence">
        <rdfs:subClassOf rdf:resource="https://github.com/corrado877/CognitiveBiasOntologies/blob/main/HotHandFallacyOntology/HotHandFallacyOntology.owl#FutureEvent"/>
        <rdfs:comment>This class represent an event that will happen in the next future and it is characterized by chance-based probability.</rdfs:comment>
        <rdfs:label>Next Chance-Based Occurence</rdfs:label>
    </owl:Class>
    


    <!-- https://w3id.org/framester/data/framestercore/Activity -->

    <owl:Class rdf:about="https://w3id.org/framester/data/framestercore/Activity">
        <owl:disjointWith rdf:resource="https://w3id.org/framester/data/framestercore/Event"/>
        <owl:disjointWith rdf:resource="https://w3id.org/framester/data/framestercore/People"/>
        <owl:disjointWith rdf:resource="https://w3id.org/framester/data/framestercore/Probability"/>
        <owl:disjointWith rdf:resource="https://w3id.org/framester/data/framestercore/Sequence"/>
        <rdfs:comment>This is an abstract frame for durative activities, in which the Agent enters an ongoing state of the Activity, remains in this state for some Duration of Time, and leaves this state either by finishing or by stopping. The Agent&apos;s Activity should be intentional. This frame is intended mostly for the inheritance of common FEs, and to provide the frame structure for the beginning, ongoing, finish, or stop stage of an Activity, each of which constitutes a subframe of this frame. This frame should be compared to the Process frame</rdfs:comment>
        <rdfs:label>Activity</rdfs:label>
    </owl:Class>
    


    <!-- https://w3id.org/framester/data/framestercore/Event -->

    <owl:Class rdf:about="https://w3id.org/framester/data/framestercore/Event">
        <owl:disjointWith rdf:resource="https://w3id.org/framester/data/framestercore/People"/>
        <owl:disjointWith rdf:resource="https://w3id.org/framester/data/framestercore/Probability"/>
        <owl:disjointWith rdf:resource="https://w3id.org/framester/data/framestercore/Sequence"/>
        <rdfs:comment>An Event takes place at a Place and Time. Big earthquakes only happen along plate boundaries. INI The party will take place on Sunday in the all-you-can-eat buffet.</rdfs:comment>
        <rdfs:label>Event</rdfs:label>
    </owl:Class>
    


    <!-- https://w3id.org/framester/data/framestercore/People -->

    <owl:Class rdf:about="https://w3id.org/framester/data/framestercore/People">
        <owl:disjointWith rdf:resource="https://w3id.org/framester/data/framestercore/Probability"/>
        <owl:disjointWith rdf:resource="https://w3id.org/framester/data/framestercore/Sequence"/>
        <rdfs:comment>This frame contains general words for Individuals, i.e. humans. The Person is conceived of as independent of other specific individuals with whom they have relationships and independent of their participation in any particular activity. They may have an Age, Descriptor, Origin, Persistent_characteristic, or Ethnicity. A man from Phoenix was shot yesterday. She gave birth to a screaming baby yesterday. I study 16-year-old female adolescents. I am dating an African-American man. She comforted the terrified child. I always thought of him as a stupid man.</rdfs:comment>
        <rdfs:label>People</rdfs:label>
    </owl:Class>
    


    <!-- https://w3id.org/framester/data/framestercore/Probability -->

    <owl:Class rdf:about="https://w3id.org/framester/data/framestercore/Probability">
        <owl:disjointWith rdf:resource="https://w3id.org/framester/data/framestercore/Sequence"/>
        <rdfs:comment>This frame characterizes the likelihood that a Hypothetical_event will happen as a position on a scale of impossible to inevitable. The likelihood can expressed as numerical Odds or a metaphorical representation of the Position on a scale. There&apos;s a 20 % chance that you&apos;ll succeed. The odds that he&apos;ll actually do it are one in a million.</rdfs:comment>
        <rdfs:label>Probability</rdfs:label>
    </owl:Class>
    


    <!-- https://w3id.org/framester/data/framestercore/Sequence -->

    <owl:Class rdf:about="https://w3id.org/framester/data/framestercore/Sequence">
        <rdfs:comment>The words in this frame describe entities that occur in some temporally-ordered sequence. The entities thus have some sort of relation between them that might be described by the Relative_time frame. However, at this time, this frame has no Frame Relation with that frame (though this is still under discussion). Additionally, it should be noted that the words in this frame have a metaphorical link to the words in Shape. Describe in detail the sequence of steps taken during an emergency.</rdfs:comment>
        <rdfs:label>Sequence</rdfs:label>
    </owl:Class>
    


    <!-- https://w3id.org/framester/data/framestersyn/Bettor.n.1 -->

    <owl:Class rdf:about="https://w3id.org/framester/data/framestersyn/Bettor.n.1">
        <rdfs:subClassOf rdf:resource="https://w3id.org/framester/data/framestercore/People"/>
        <rdfs:comment>A class for a player involved in an Activity such as Sport Bets.</rdfs:comment>
        <rdfs:label>Player</rdfs:label>
    </owl:Class>
    


    <!-- 
    ///////////////////////////////////////////////////////////////////////////////////////
    //
    // Individuals
    //
    ///////////////////////////////////////////////////////////////////////////////////////
     -->

    


    <!-- https://github.com/corrado877/CognitiveBiasOntologies/blob/main/HotHandFallacyOntology/HotHandFallacyOntology.owl#Football_Team_Match_Bet -->

    <owl:NamedIndividual rdf:about="https://github.com/corrado877/CognitiveBiasOntologies/blob/main/HotHandFallacyOntology/HotHandFallacyOntology.owl#Football_Team_Match_Bet">
        <rdf:type rdf:resource="https://github.com/corrado877/CognitiveBiasOntologies/blob/main/HotHandFallacyOntology/HotHandFallacyOntology.owl#NextChance-BasedOccurence"/>
        <parameter:hasParameter rdf:resource="https://github.com/corrado877/CognitiveBiasOntologies/blob/main/HotHandFallacyOntology/HotHandFallacyOntology.owl#ProbabilityLevel"/>
        <HotHandFallacyOntology:producesOutcomeEffect rdf:resource="https://github.com/corrado877/CognitiveBiasOntologies/blob/main/HotHandFallacyOntology/HotHandFallacyOntology.owl#Winning_Bet"/>
        <rdfs:comment>An indivifual for the next chance-based occurence class such as a Footbal Team Match Bet where the probability level is not completely random and can be influenced by different external elements.</rdfs:comment>
        <rdfs:label>Football Team Match Bet</rdfs:label>
    </owl:NamedIndividual>
    


    <!-- https://github.com/corrado877/CognitiveBiasOntologies/blob/main/HotHandFallacyOntology/HotHandFallacyOntology.owl#Football_Team_Match_Bet_Series -->

    <owl:NamedIndividual rdf:about="https://github.com/corrado877/CognitiveBiasOntologies/blob/main/HotHandFallacyOntology/HotHandFallacyOntology.owl#Football_Team_Match_Bet_Series">
        <rdf:type rdf:resource="https://w3id.org/framester/data/framestercore/Sequence"/>
        <prov:wasGeneratedBy rdf:resource="https://github.com/corrado877/CognitiveBiasOntologies/blob/main/HotHandFallacyOntology/HotHandFallacyOntology.owl#Sport_Bets"/>
        <HotHandFallacyOntology:hasOutcomeEffect rdf:resource="https://github.com/corrado877/CognitiveBiasOntologies/blob/main/HotHandFallacyOntology/HotHandFallacyOntology.owl#Winning_Bet"/>
        <rdfs:comment>a sequence of past bets that have the same outcome effect</rdfs:comment>
        <rdfs:label>Football Team Match Bet Series</rdfs:label>
    </owl:NamedIndividual>
    


    <!-- https://github.com/corrado877/CognitiveBiasOntologies/blob/main/HotHandFallacyOntology/HotHandFallacyOntology.owl#ProbabilityLevel -->

    <owl:NamedIndividual rdf:about="https://github.com/corrado877/CognitiveBiasOntologies/blob/main/HotHandFallacyOntology/HotHandFallacyOntology.owl#ProbabilityLevel">
        <rdf:type rdf:resource="https://w3id.org/framester/data/framestercore/Probability"/>
        <aff:influencedBy rdf:resource="https://github.com/corrado877/CognitiveBiasOntologies/blob/main/HotHandFallacyOntology/HotHandFallacyOntology.owl#Football_Team_Match_Bet_Series"/>
        <parameter:hasParameterDataValue>High</parameter:hasParameterDataValue>
        <rdfs:comment>The probability level that an event such a chance-based occurence can have in the next future a specific outcome effect.</rdfs:comment>
        <rdfs:label>ProbabiltyLevel</rdfs:label>
    </owl:NamedIndividual>
    


    <!-- https://github.com/corrado877/CognitiveBiasOntologies/blob/main/HotHandFallacyOntology/HotHandFallacyOntology.owl#Sport_Bets -->

    <owl:NamedIndividual rdf:about="https://github.com/corrado877/CognitiveBiasOntologies/blob/main/HotHandFallacyOntology/HotHandFallacyOntology.owl#Sport_Bets">
        <rdf:type rdf:resource="https://w3id.org/framester/data/framestercore/Activity"/>
        <participation:hasParticipant rdf:resource="https://github.com/corrado877/CognitiveBiasOntologies/blob/main/HotHandFallacyOntology/HotHandFallacyOntology.owl#Sport_Bettor"/>
        <partof:hasPart rdf:resource="https://github.com/corrado877/CognitiveBiasOntologies/blob/main/HotHandFallacyOntology/HotHandFallacyOntology.owl#Football_Team_Match_Bet"/>
        <rdfs:comment>An individual representing an Acitvity such as Sport Bets in which is involved a player.</rdfs:comment>
        <rdfs:label>Sport Bets</rdfs:label>
    </owl:NamedIndividual>
    


    <!-- https://github.com/corrado877/CognitiveBiasOntologies/blob/main/HotHandFallacyOntology/HotHandFallacyOntology.owl#Sport_Bettor -->

    <owl:NamedIndividual rdf:about="https://github.com/corrado877/CognitiveBiasOntologies/blob/main/HotHandFallacyOntology/HotHandFallacyOntology.owl#Sport_Bettor">
        <rdf:type rdf:resource="https://w3id.org/framester/data/framestersyn/Bettor.n.1"/>
        <cco:belief rdf:resource="https://github.com/corrado877/CognitiveBiasOntologies/blob/main/HotHandFallacyOntology/HotHandFallacyOntology.owl#Football_Team_Match_Bet_Series"/>
        <HotHandFallacyOntology:hasBiasedOpinion rdf:resource="https://github.com/corrado877/CognitiveBiasOntologies/blob/main/HotHandFallacyOntology/HotHandFallacyOntology.owl#Football_Team_Match_Bet"/>
        <rdfs:comment>A sport Bettor individual who is participating in an Activity such as Sport Bets</rdfs:comment>
        <rdfs:label>Sport Bettor</rdfs:label>
    </owl:NamedIndividual>
    


    <!-- https://github.com/corrado877/CognitiveBiasOntologies/blob/main/HotHandFallacyOntology/HotHandFallacyOntology.owl#Winning_Bet -->

    <owl:NamedIndividual rdf:about="https://github.com/corrado877/CognitiveBiasOntologies/blob/main/HotHandFallacyOntology/HotHandFallacyOntology.owl#Winning_Bet">
        <rdf:type rdf:resource="https://dbpedia.org/page/Success"/>
        <rdfs:comment>An individual representing the outcome effect of events such as a Football Team Match Bet</rdfs:comment>
        <rdfs:label>Winning Bet</rdfs:label>
    </owl:NamedIndividual>
</rdf:RDF>



<!-- Generated by the OWL API (version 4.5.26.2023-07-17T20:34:13Z) https://github.com/owlcs/owlapi -->

