<?xml version="1.0"?>
<rdf:RDF xmlns="https://github.com/corrado877/CognitiveBiasOntologies/blob/main/GamblersFallacyOntology/GamblersFallacyOntology.owl#"
     xml:base="https://github.com/corrado877/CognitiveBiasOntologies/blob/main/GamblersFallacyOntology/GamblersFallacyOntology.owl"
     xmlns:fs="https://w3id.org/framester/data/framestercore"
     xmlns:cco="http://purl.org/ontology/cco/cognitivecharacteristics.owl"
     xmlns:owl="http://www.w3.org/2002/07/owl#"
     xmlns:rdf="http://www.w3.org/1999/02/22-rdf-syntax-ns#"
     xmlns:xml="http://www.w3.org/XML/1998/namespace"
     xmlns:xsd="http://www.w3.org/2001/XMLSchema#"
     xmlns:foaf="http://xmlns.com/foaf/spec/index.rdf"
     xmlns:rdfs="http://www.w3.org/2000/01/rdf-schema#"
     xmlns:terms="http://purl.org/dc/terms/"
     xmlns:partof="http://www.ontologydesignpatterns.org/cp/owl/partof.owl#"
     xmlns:parameter="http://ontologydesignpatterns.org/cp/owl/parameter.owl"
     xmlns:affectedBy="https://w3id.org/affectedBy"
     xmlns:provenance="https://raw.githubusercontent.com/cogan-shimizu-wsu/ProvenanceOWL/master/EntityWithProvenanceOntologyPattern.owl"
     xmlns:participation="http://ontologydesignpatterns.org/cp/owl/participation.owl"
     xmlns:activitypattern="http://descartes-core.org/ontologies/activities/1.0/ActivityPattern.owl"
     xmlns:cpannotationschema="http://www.ontologydesignpatterns.org/schemas/cpannotationschema.owl#"
     xmlns:GamblersFallacyOntology="https://github.com/corrado877/CognitiveBiasOntologies/blob/main/GamblersFallacyOntology/GamblersFallacyOntology.owl">
    <owl:Ontology rdf:about="https://github.com/corrado877/CognitiveBiasOntologies/blob/main/GamblersFallacyOntology/GamblersFallacyOntology.owl">
        <terms:created rdf:datatype="http://www.w3.org/2001/XMLSchema#dateTime">2024-02-20T00:00:00</terms:created>
        <terms:creator>Corrado Consiglio</terms:creator>
        <terms:description>The Gamblers&apos;Fallacy module of the Cognitive Bias Ontology</terms:description>
        <terms:title>The Gamblers&apos;Fallacy Ontology Bias</terms:title>
        <cpannotationschema:hasComponent rdf:resource="http://ontologydesignpatterns.org/wiki/Submissions:AffectedBy"/>
        <cpannotationschema:hasComponent rdf:resource="http://ontologydesignpatterns.org/wiki/Submissions:An_Ontology_Design_Pattern_for_Activity_Reasoning"/>
        <cpannotationschema:hasComponent rdf:resource="http://ontologydesignpatterns.org/wiki/Submissions:Parameter"/>
        <cpannotationschema:hasComponent rdf:resource="http://ontologydesignpatterns.org/wiki/Submissions:PartOf"/>
        <cpannotationschema:hasComponent rdf:resource="http://ontologydesignpatterns.org/wiki/Submissions:Participation"/>
        <cpannotationschema:hasComponent rdf:resource="http://ontologydesignpatterns.org/wiki/Submissions:Provenance"/>
        <cpannotationschema:hasComponent rdf:resource="http://ontologydesignpatterns.org/wiki/Submissions:RecurrentEventSeries"/>
        <cpannotationschema:hasComponent rdf:resource="http://purl.org/ontology/cco/20100926/cognitivecharacteristics.html"/>
        <cpannotationschema:hasComponent rdf:resource="http://xmlns.com/foaf/spec/20140114.html"/>
        <cpannotationschema:scenarios>In a lottery, a person thinks that a certain number is more likely to be drawn next because it hasn&apos;t been drawn in a long time.</cpannotationschema:scenarios>
        <rdfs:comment xml:lang="en">The Gambler&apos;s Fallacy bias, also known as the Fallacy of the Maturity of Chances, is a cognitive bias that occurs when an individual believes that past events in a random or chance-based process can influence the likelihood of future events in the same process. It is a mistaken belief that, because a certain outcome has occurred frequently or infrequently in the past, the probability of that outcome occurring again in the future is somehow altered or &quot;due&quot; to happen.</rdfs:comment>
    </owl:Ontology>
    


    <!-- 
    ///////////////////////////////////////////////////////////////////////////////////////
    //
    // Annotation properties
    //
    ///////////////////////////////////////////////////////////////////////////////////////
     -->

    


    <!-- http://purl.org/dc/terms/created -->

    <owl:AnnotationProperty rdf:about="http://purl.org/dc/terms/created"/>
    


    <!-- http://purl.org/dc/terms/creator -->

    <owl:AnnotationProperty rdf:about="http://purl.org/dc/terms/creator"/>
    


    <!-- http://purl.org/dc/terms/description -->

    <owl:AnnotationProperty rdf:about="http://purl.org/dc/terms/description"/>
    


    <!-- http://purl.org/dc/terms/title -->

    <owl:AnnotationProperty rdf:about="http://purl.org/dc/terms/title"/>
    


    <!-- http://www.ontologydesignpatterns.org/schemas/cpannotationschema.owl#hasComponent -->

    <owl:AnnotationProperty rdf:about="http://www.ontologydesignpatterns.org/schemas/cpannotationschema.owl#hasComponent"/>
    


    <!-- http://www.ontologydesignpatterns.org/schemas/cpannotationschema.owl#scenarios -->

    <owl:AnnotationProperty rdf:about="http://www.ontologydesignpatterns.org/schemas/cpannotationschema.owl#scenarios"/>
    


    <!-- 
    ///////////////////////////////////////////////////////////////////////////////////////
    //
    // Object Properties
    //
    ///////////////////////////////////////////////////////////////////////////////////////
     -->

    


    <!-- https://github.com/corrado877/CognitiveBiasOntologies/blob/main/GamblersFallacyOntology/GamblersFallacyOntology.owl#generatedBy -->

    <owl:ObjectProperty rdf:about="https://github.com/corrado877/CognitiveBiasOntologies/blob/main/GamblersFallacyOntology/GamblersFallacyOntology.owl#generatedBy">
        <rdfs:domain rdf:resource="https://github.com/corrado877/CognitiveBiasOntologies/blob/main/GamblersFallacyOntology/GamblersFallacyOntology.owl#Sequence"/>
        <rdfs:range rdf:resource="https://w3id.org/framester/data/framestercore/Activity"/>
    </owl:ObjectProperty>
    


    <!-- https://github.com/corrado877/CognitiveBiasOntologies/blob/main/GamblersFallacyOntology/GamblersFallacyOntology.owl#hasBelief -->

    <owl:ObjectProperty rdf:about="https://github.com/corrado877/CognitiveBiasOntologies/blob/main/GamblersFallacyOntology/GamblersFallacyOntology.owl#hasBelief">
        <rdfs:domain rdf:resource="https://github.com/corrado877/CognitiveBiasOntologies/blob/main/GamblersFallacyOntology/GamblersFallacyOntology.owl#Person"/>
        <rdfs:range rdf:resource="https://github.com/corrado877/CognitiveBiasOntologies/blob/main/GamblersFallacyOntology/GamblersFallacyOntology.owl#Sequence"/>
        <rdfs:comment>An uncertain relation for competence representation. That means beliefs, persuasions or opinions, which can also be misconceptions. A Person who believes that a sequence of past events with the same outcome can change the probability of the outcome of the same event in the future</rdfs:comment>
    </owl:ObjectProperty>
    


    <!-- https://github.com/corrado877/CognitiveBiasOntologies/blob/main/GamblersFallacyOntology/GamblersFallacyOntology.owl#hasBiasedOpinion -->

    <owl:ObjectProperty rdf:about="https://github.com/corrado877/CognitiveBiasOntologies/blob/main/GamblersFallacyOntology/GamblersFallacyOntology.owl#hasBiasedOpinion">
        <rdfs:domain rdf:resource="https://github.com/corrado877/CognitiveBiasOntologies/blob/main/GamblersFallacyOntology/GamblersFallacyOntology.owl#Person"/>
        <rdfs:range rdf:resource="https://github.com/corrado877/CognitiveBiasOntologies/blob/main/GamblersFallacyOntology/GamblersFallacyOntology.owl#NextRandomOccurrence"/>
        <rdfs:comment>a property connecting a Person who has a biased opinion about the possible outcome of an Event such as a Random or Chance-based Occurrence</rdfs:comment>
    </owl:ObjectProperty>
    


    <!-- https://github.com/corrado877/CognitiveBiasOntologies/blob/main/GamblersFallacyOntology/GamblersFallacyOntology.owl#hasInfluence -->

    <owl:ObjectProperty rdf:about="https://github.com/corrado877/CognitiveBiasOntologies/blob/main/GamblersFallacyOntology/GamblersFallacyOntology.owl#hasInfluence">
        <owl:inverseOf rdf:resource="https://github.com/corrado877/CognitiveBiasOntologies/blob/main/GamblersFallacyOntology/GamblersFallacyOntology.owl#influencedBy"/>
    </owl:ObjectProperty>
    


    <!-- https://github.com/corrado877/CognitiveBiasOntologies/blob/main/GamblersFallacyOntology/GamblersFallacyOntology.owl#hasOutcome -->

    <owl:ObjectProperty rdf:about="https://github.com/corrado877/CognitiveBiasOntologies/blob/main/GamblersFallacyOntology/GamblersFallacyOntology.owl#hasOutcome">
        <owl:inverseOf rdf:resource="https://github.com/corrado877/CognitiveBiasOntologies/blob/main/GamblersFallacyOntology/GamblersFallacyOntology.owl#isOutcomeOf"/>
        <rdfs:domain rdf:resource="https://github.com/corrado877/CognitiveBiasOntologies/blob/main/GamblersFallacyOntology/GamblersFallacyOntology.owl#Sequence"/>
        <rdfs:range rdf:resource="https://github.com/corrado877/CognitiveBiasOntologies/blob/main/GamblersFallacyOntology/GamblersFallacyOntology.owl#ColorNumber"/>
        <rdfs:comment>A property linking series of events to the same Outcome</rdfs:comment>
    </owl:ObjectProperty>
    


    <!-- https://github.com/corrado877/CognitiveBiasOntologies/blob/main/GamblersFallacyOntology/GamblersFallacyOntology.owl#hasParameter -->

    <owl:ObjectProperty rdf:about="https://github.com/corrado877/CognitiveBiasOntologies/blob/main/GamblersFallacyOntology/GamblersFallacyOntology.owl#hasParameter">
        <owl:inverseOf rdf:resource="https://github.com/corrado877/CognitiveBiasOntologies/blob/main/GamblersFallacyOntology/GamblersFallacyOntology.owl#isParameterFor"/>
        <rdfs:domain rdf:resource="https://github.com/corrado877/CognitiveBiasOntologies/blob/main/GamblersFallacyOntology/GamblersFallacyOntology.owl#NextRandomOccurrence"/>
        <rdfs:range rdf:resource="https://github.com/corrado877/CognitiveBiasOntologies/blob/main/GamblersFallacyOntology/GamblersFallacyOntology.owl#Probability"/>
    </owl:ObjectProperty>
    


    <!-- https://github.com/corrado877/CognitiveBiasOntologies/blob/main/GamblersFallacyOntology/GamblersFallacyOntology.owl#hasPart -->

    <owl:ObjectProperty rdf:about="https://github.com/corrado877/CognitiveBiasOntologies/blob/main/GamblersFallacyOntology/GamblersFallacyOntology.owl#hasPart">
        <owl:inverseOf rdf:resource="https://github.com/corrado877/CognitiveBiasOntologies/blob/main/GamblersFallacyOntology/GamblersFallacyOntology.owl#isPartOf"/>
    </owl:ObjectProperty>
    


    <!-- https://github.com/corrado877/CognitiveBiasOntologies/blob/main/GamblersFallacyOntology/GamblersFallacyOntology.owl#hasParticipant -->

    <owl:ObjectProperty rdf:about="https://github.com/corrado877/CognitiveBiasOntologies/blob/main/GamblersFallacyOntology/GamblersFallacyOntology.owl#hasParticipant">
        <owl:inverseOf rdf:resource="https://github.com/corrado877/CognitiveBiasOntologies/blob/main/GamblersFallacyOntology/GamblersFallacyOntology.owl#isParticipantIn"/>
        <rdfs:domain rdf:resource="https://w3id.org/framester/data/framestercore/Activity"/>
        <rdfs:range rdf:resource="https://github.com/corrado877/CognitiveBiasOntologies/blob/main/GamblersFallacyOntology/GamblersFallacyOntology.owl#Person"/>
    </owl:ObjectProperty>
    


    <!-- https://github.com/corrado877/CognitiveBiasOntologies/blob/main/GamblersFallacyOntology/GamblersFallacyOntology.owl#influencedBy -->

    <owl:ObjectProperty rdf:about="https://github.com/corrado877/CognitiveBiasOntologies/blob/main/GamblersFallacyOntology/GamblersFallacyOntology.owl#influencedBy">
        <rdfs:domain rdf:resource="https://github.com/corrado877/CognitiveBiasOntologies/blob/main/GamblersFallacyOntology/GamblersFallacyOntology.owl#Probability"/>
        <rdfs:range rdf:resource="https://github.com/corrado877/CognitiveBiasOntologies/blob/main/GamblersFallacyOntology/GamblersFallacyOntology.owl#Sequence"/>
    </owl:ObjectProperty>
    


    <!-- https://github.com/corrado877/CognitiveBiasOntologies/blob/main/GamblersFallacyOntology/GamblersFallacyOntology.owl#isOutcomeOf -->

    <owl:ObjectProperty rdf:about="https://github.com/corrado877/CognitiveBiasOntologies/blob/main/GamblersFallacyOntology/GamblersFallacyOntology.owl#isOutcomeOf">
        <rdfs:comment>Inverse property of HasOutcome property</rdfs:comment>
    </owl:ObjectProperty>
    


    <!-- https://github.com/corrado877/CognitiveBiasOntologies/blob/main/GamblersFallacyOntology/GamblersFallacyOntology.owl#isParameterFor -->

    <owl:ObjectProperty rdf:about="https://github.com/corrado877/CognitiveBiasOntologies/blob/main/GamblersFallacyOntology/GamblersFallacyOntology.owl#isParameterFor"/>
    


    <!-- https://github.com/corrado877/CognitiveBiasOntologies/blob/main/GamblersFallacyOntology/GamblersFallacyOntology.owl#isPartOf -->

    <owl:ObjectProperty rdf:about="https://github.com/corrado877/CognitiveBiasOntologies/blob/main/GamblersFallacyOntology/GamblersFallacyOntology.owl#isPartOf">
        <rdfs:domain rdf:resource="https://github.com/corrado877/CognitiveBiasOntologies/blob/main/GamblersFallacyOntology/GamblersFallacyOntology.owl#NextRandomOccurrence"/>
        <rdfs:range rdf:resource="https://w3id.org/framester/data/framestercore/Activity"/>
    </owl:ObjectProperty>
    


    <!-- https://github.com/corrado877/CognitiveBiasOntologies/blob/main/GamblersFallacyOntology/GamblersFallacyOntology.owl#isParticipantIn -->

    <owl:ObjectProperty rdf:about="https://github.com/corrado877/CognitiveBiasOntologies/blob/main/GamblersFallacyOntology/GamblersFallacyOntology.owl#isParticipantIn"/>
    


    <!-- https://github.com/corrado877/CognitiveBiasOntologies/blob/main/GamblersFallacyOntology/GamblersFallacyOntology.owl#isProducedBy -->

    <owl:ObjectProperty rdf:about="https://github.com/corrado877/CognitiveBiasOntologies/blob/main/GamblersFallacyOntology/GamblersFallacyOntology.owl#isProducedBy">
        <owl:inverseOf rdf:resource="https://github.com/corrado877/CognitiveBiasOntologies/blob/main/GamblersFallacyOntology/GamblersFallacyOntology.owl#produces"/>
    </owl:ObjectProperty>
    


    <!-- https://github.com/corrado877/CognitiveBiasOntologies/blob/main/GamblersFallacyOntology/GamblersFallacyOntology.owl#produces -->

    <owl:ObjectProperty rdf:about="https://github.com/corrado877/CognitiveBiasOntologies/blob/main/GamblersFallacyOntology/GamblersFallacyOntology.owl#produces">
        <rdfs:domain rdf:resource="https://github.com/corrado877/CognitiveBiasOntologies/blob/main/GamblersFallacyOntology/GamblersFallacyOntology.owl#NextRandomOccurrence"/>
        <rdfs:range rdf:resource="https://github.com/corrado877/CognitiveBiasOntologies/blob/main/GamblersFallacyOntology/GamblersFallacyOntology.owl#Outcome"/>
    </owl:ObjectProperty>
    


    <!-- 
    ///////////////////////////////////////////////////////////////////////////////////////
    //
    // Data properties
    //
    ///////////////////////////////////////////////////////////////////////////////////////
     -->

    


    <!-- https://github.com/corrado877/CognitiveBiasOntologies/blob/main/GamblersFallacyOntology/GamblersFallacyOntology.owl#hasParameterDataValue -->

    <owl:DatatypeProperty rdf:about="https://github.com/corrado877/CognitiveBiasOntologies/blob/main/GamblersFallacyOntology/GamblersFallacyOntology.owl#hasParameterDataValue">
        <rdfs:domain rdf:resource="https://github.com/corrado877/CognitiveBiasOntologies/blob/main/GamblersFallacyOntology/GamblersFallacyOntology.owl#Probability"/>
        <rdfs:range rdf:resource="http://www.w3.org/2001/XMLSchema#string"/>
    </owl:DatatypeProperty>
    


    <!-- 
    ///////////////////////////////////////////////////////////////////////////////////////
    //
    // Classes
    //
    ///////////////////////////////////////////////////////////////////////////////////////
     -->

    


    <!-- https://github.com/corrado877/CognitiveBiasOntologies/blob/main/GamblersFallacyOntology/GamblersFallacyOntology.owl#ColorNumber -->

    <owl:Class rdf:about="https://github.com/corrado877/CognitiveBiasOntologies/blob/main/GamblersFallacyOntology/GamblersFallacyOntology.owl#ColorNumber">
        <rdfs:subClassOf rdf:resource="https://github.com/corrado877/CognitiveBiasOntologies/blob/main/GamblersFallacyOntology/GamblersFallacyOntology.owl#Outcome"/>
    </owl:Class>
    


    <!-- https://github.com/corrado877/CognitiveBiasOntologies/blob/main/GamblersFallacyOntology/GamblersFallacyOntology.owl#FutureEvent -->

    <owl:Class rdf:about="https://github.com/corrado877/CognitiveBiasOntologies/blob/main/GamblersFallacyOntology/GamblersFallacyOntology.owl#FutureEvent">
        <rdfs:subClassOf rdf:resource="https://w3id.org/framester/data/framestercore/Event"/>
        <rdfs:comment>This class represent an event that will happen in the next future.</rdfs:comment>
        <rdfs:label>FutureEvent</rdfs:label>
    </owl:Class>
    


    <!-- https://github.com/corrado877/CognitiveBiasOntologies/blob/main/GamblersFallacyOntology/GamblersFallacyOntology.owl#NextRandomOccurrence -->

    <owl:Class rdf:about="https://github.com/corrado877/CognitiveBiasOntologies/blob/main/GamblersFallacyOntology/GamblersFallacyOntology.owl#NextRandomOccurrence">
        <rdfs:subClassOf rdf:resource="https://github.com/corrado877/CognitiveBiasOntologies/blob/main/GamblersFallacyOntology/GamblersFallacyOntology.owl#FutureEvent"/>
        <rdfs:subClassOf>
            <owl:Restriction>
                <owl:onProperty rdf:resource="https://github.com/corrado877/CognitiveBiasOntologies/blob/main/GamblersFallacyOntology/GamblersFallacyOntology.owl#isPartOf"/>
                <owl:someValuesFrom rdf:resource="https://w3id.org/framester/data/framestercore/Activity"/>
            </owl:Restriction>
        </rdfs:subClassOf>
        <rdfs:comment>This class represent an event that will happen in the next future and it is characterized by randomness.</rdfs:comment>
        <rdfs:label>NextRandomOccurence</rdfs:label>
    </owl:Class>
    


    <!-- https://github.com/corrado877/CognitiveBiasOntologies/blob/main/GamblersFallacyOntology/GamblersFallacyOntology.owl#Outcome -->

    <owl:Class rdf:about="https://github.com/corrado877/CognitiveBiasOntologies/blob/main/GamblersFallacyOntology/GamblersFallacyOntology.owl#Outcome">
        <rdfs:comment>This class represent the outcome of an event such as a RandomOccurence</rdfs:comment>
    </owl:Class>
    


    <!-- https://github.com/corrado877/CognitiveBiasOntologies/blob/main/GamblersFallacyOntology/GamblersFallacyOntology.owl#Person -->

    <owl:Class rdf:about="https://github.com/corrado877/CognitiveBiasOntologies/blob/main/GamblersFallacyOntology/GamblersFallacyOntology.owl#Person">
        <rdfs:comment>Any individual involved in an activity.</rdfs:comment>
    </owl:Class>
    


    <!-- https://github.com/corrado877/CognitiveBiasOntologies/blob/main/GamblersFallacyOntology/GamblersFallacyOntology.owl#Probability -->

    <owl:Class rdf:about="https://github.com/corrado877/CognitiveBiasOntologies/blob/main/GamblersFallacyOntology/GamblersFallacyOntology.owl#Probability">
        <rdfs:comment>This frame characterizes the likelihood that a Hypothetical_event will happen as a position on a scale of impossible to inevitable.</rdfs:comment>
    </owl:Class>
    


    <!-- https://github.com/corrado877/CognitiveBiasOntologies/blob/main/GamblersFallacyOntology/GamblersFallacyOntology.owl#Sequence -->

    <owl:Class rdf:about="https://github.com/corrado877/CognitiveBiasOntologies/blob/main/GamblersFallacyOntology/GamblersFallacyOntology.owl#Sequence">
        <rdfs:subClassOf>
            <owl:Restriction>
                <owl:onProperty rdf:resource="https://github.com/corrado877/CognitiveBiasOntologies/blob/main/GamblersFallacyOntology/GamblersFallacyOntology.owl#generatedBy"/>
                <owl:someValuesFrom rdf:resource="https://w3id.org/framester/data/framestercore/Activity"/>
            </owl:Restriction>
        </rdfs:subClassOf>
        <rdfs:comment>This frame represent a sequence of temporally-ordered past events that have the same outcome</rdfs:comment>
    </owl:Class>
    


    <!-- https://w3id.org/framester/data/framestercore/Activity -->

    <owl:Class rdf:about="https://w3id.org/framester/data/framestercore/Activity">
        <rdfs:comment>This is an abstract frame for durative activities, in which the Agent enters an ongoing state of the Activity, remains in this state for some Duration of Time, and leaves this state either by finishing or by stopping. The Agent&apos;s Activity should be intentional. This frame is intended mostly for the inheritance of common FEs, and to provide the frame structure for the beginning, ongoing, finish, or stop stage of an Activity, each of which constitutes a subframe of this frame. This frame should be compared to the Process frame. In this case the frame represents an activity with random or chance-based outcomes in which a person is involved in.</rdfs:comment>
        <rdfs:label>Activity</rdfs:label>
    </owl:Class>
    


    <!-- https://w3id.org/framester/data/framestercore/Event -->

    <owl:Class rdf:about="https://w3id.org/framester/data/framestercore/Event">
        <rdfs:comment>An Event takes place at a Place and Time. Big earthquakes only happen along plate boundaries. INI The party will take place on Sunday in the all-you-can-eat buffet.</rdfs:comment>
        <rdfs:label>Event</rdfs:label>
    </owl:Class>
    


    <!-- 
    ///////////////////////////////////////////////////////////////////////////////////////
    //
    // Individuals
    //
    ///////////////////////////////////////////////////////////////////////////////////////
     -->

    


    <!-- https://github.com/corrado877/CognitiveBiasOntologies/blob/main/GamblersFallacyOntology/GamblersFallacyOntology.owl#Black_Number -->

    <owl:NamedIndividual rdf:about="https://github.com/corrado877/CognitiveBiasOntologies/blob/main/GamblersFallacyOntology/GamblersFallacyOntology.owl#Black_Number">
        <rdf:type rdf:resource="https://github.com/corrado877/CognitiveBiasOntologies/blob/main/GamblersFallacyOntology/GamblersFallacyOntology.owl#ColorNumber"/>
        <rdfs:comment>The outcome of the next number draw or past number draws. Black numbers and red numbers have the same probability of being extracted.</rdfs:comment>
    </owl:NamedIndividual>
    


    <!-- https://github.com/corrado877/CognitiveBiasOntologies/blob/main/GamblersFallacyOntology/GamblersFallacyOntology.owl#Lottery_Draw -->

    <owl:NamedIndividual rdf:about="https://github.com/corrado877/CognitiveBiasOntologies/blob/main/GamblersFallacyOntology/GamblersFallacyOntology.owl#Lottery_Draw">
        <rdf:type rdf:resource="https://w3id.org/framester/data/framestercore/Activity"/>
        <rdfs:comment>an activity where numbers are of two different colours (black and red) and where only one number is extracted for each draw.</rdfs:comment>
    </owl:NamedIndividual>
    


    <!-- https://github.com/corrado877/CognitiveBiasOntologies/blob/main/GamblersFallacyOntology/GamblersFallacyOntology.owl#Lottery_Participant -->

    <owl:NamedIndividual rdf:about="https://github.com/corrado877/CognitiveBiasOntologies/blob/main/GamblersFallacyOntology/GamblersFallacyOntology.owl#Lottery_Participant">
        <rdf:type rdf:resource="https://github.com/corrado877/CognitiveBiasOntologies/blob/main/GamblersFallacyOntology/GamblersFallacyOntology.owl#Person"/>
        <hasBelief rdf:resource="https://github.com/corrado877/CognitiveBiasOntologies/blob/main/GamblersFallacyOntology/GamblersFallacyOntology.owl#Past_Number_Draw_Series"/>
        <hasBiasedOpinion rdf:resource="https://github.com/corrado877/CognitiveBiasOntologies/blob/main/GamblersFallacyOntology/GamblersFallacyOntology.owl#NumberDraw"/>
        <isParticipantIn rdf:resource="https://github.com/corrado877/CognitiveBiasOntologies/blob/main/GamblersFallacyOntology/GamblersFallacyOntology.owl#Lottery_Draw"/>
        <rdfs:comment>An human being that participates to a lottery draw.</rdfs:comment>
    </owl:NamedIndividual>
    


    <!-- https://github.com/corrado877/CognitiveBiasOntologies/blob/main/GamblersFallacyOntology/GamblersFallacyOntology.owl#NumberDraw -->

    <owl:NamedIndividual rdf:about="https://github.com/corrado877/CognitiveBiasOntologies/blob/main/GamblersFallacyOntology/GamblersFallacyOntology.owl#NumberDraw">
        <rdf:type rdf:resource="https://github.com/corrado877/CognitiveBiasOntologies/blob/main/GamblersFallacyOntology/GamblersFallacyOntology.owl#NextRandomOccurrence"/>
        <hasParameter rdf:resource="https://github.com/corrado877/CognitiveBiasOntologies/blob/main/GamblersFallacyOntology/GamblersFallacyOntology.owl#ProbabilityLevel"/>
        <isPartOf rdf:resource="https://github.com/corrado877/CognitiveBiasOntologies/blob/main/GamblersFallacyOntology/GamblersFallacyOntology.owl#Lottery_Draw"/>
        <produces rdf:resource="https://github.com/corrado877/CognitiveBiasOntologies/blob/main/GamblersFallacyOntology/GamblersFallacyOntology.owl#Black_Number"/>
        <rdfs:comment>a number draw in a lottery is an event totally random where each number has the same probability of being extracted.</rdfs:comment>
    </owl:NamedIndividual>
    


    <!-- https://github.com/corrado877/CognitiveBiasOntologies/blob/main/GamblersFallacyOntology/GamblersFallacyOntology.owl#Past_Number_Draw_Series -->

    <owl:NamedIndividual rdf:about="https://github.com/corrado877/CognitiveBiasOntologies/blob/main/GamblersFallacyOntology/GamblersFallacyOntology.owl#Past_Number_Draw_Series">
        <rdf:type rdf:resource="https://github.com/corrado877/CognitiveBiasOntologies/blob/main/GamblersFallacyOntology/GamblersFallacyOntology.owl#Sequence"/>
        <generatedBy rdf:resource="https://github.com/corrado877/CognitiveBiasOntologies/blob/main/GamblersFallacyOntology/GamblersFallacyOntology.owl#Lottery_Draw"/>
        <hasOutcome rdf:resource="https://github.com/corrado877/CognitiveBiasOntologies/blob/main/GamblersFallacyOntology/GamblersFallacyOntology.owl#Black_Number"/>
        <rdfs:comment>An ordered sequence of past number draws that has the same outcome (black) will influence the judgment of the participant about the probability of the outcome in the next number draw.</rdfs:comment>
    </owl:NamedIndividual>
    


    <!-- https://github.com/corrado877/CognitiveBiasOntologies/blob/main/GamblersFallacyOntology/GamblersFallacyOntology.owl#ProbabilityLevel -->

    <owl:NamedIndividual rdf:about="https://github.com/corrado877/CognitiveBiasOntologies/blob/main/GamblersFallacyOntology/GamblersFallacyOntology.owl#ProbabilityLevel">
        <rdf:type rdf:resource="https://github.com/corrado877/CognitiveBiasOntologies/blob/main/GamblersFallacyOntology/GamblersFallacyOntology.owl#Probability"/>
        <influencedBy rdf:resource="https://github.com/corrado877/CognitiveBiasOntologies/blob/main/GamblersFallacyOntology/GamblersFallacyOntology.owl#Past_Number_Draw_Series"/>
        <hasParameterDataValue>Low</hasParameterDataValue>
        <rdfs:comment>The level of probability that the outcome of the next number draw will be red or black  can be higher or lower for the participant, depending on the outcomes of the previous number draws.</rdfs:comment>
    </owl:NamedIndividual>
    


    <!-- https://github.com/corrado877/CognitiveBiasOntologies/blob/main/GamblersFallacyOntology/GamblersFallacyOntology.owl#Red_Number -->

    <owl:NamedIndividual rdf:about="https://github.com/corrado877/CognitiveBiasOntologies/blob/main/GamblersFallacyOntology/GamblersFallacyOntology.owl#Red_Number">
        <rdf:type rdf:resource="https://github.com/corrado877/CognitiveBiasOntologies/blob/main/GamblersFallacyOntology/GamblersFallacyOntology.owl#ColorNumber"/>
        <rdfs:comment>The outcome of the next number draw or past number draws. Black numbers and red numbers have the same probability of being extracted</rdfs:comment>
    </owl:NamedIndividual>
    


    <!-- 
    ///////////////////////////////////////////////////////////////////////////////////////
    //
    // General axioms
    //
    ///////////////////////////////////////////////////////////////////////////////////////
     -->

    <rdf:Description>
        <rdf:type rdf:resource="http://www.w3.org/2002/07/owl#AllDisjointClasses"/>
        <owl:members rdf:parseType="Collection">
            <rdf:Description rdf:about="https://github.com/corrado877/CognitiveBiasOntologies/blob/main/GamblersFallacyOntology/GamblersFallacyOntology.owl#Outcome"/>
            <rdf:Description rdf:about="https://github.com/corrado877/CognitiveBiasOntologies/blob/main/GamblersFallacyOntology/GamblersFallacyOntology.owl#Person"/>
            <rdf:Description rdf:about="https://github.com/corrado877/CognitiveBiasOntologies/blob/main/GamblersFallacyOntology/GamblersFallacyOntology.owl#Probability"/>
            <rdf:Description rdf:about="https://github.com/corrado877/CognitiveBiasOntologies/blob/main/GamblersFallacyOntology/GamblersFallacyOntology.owl#Sequence"/>
            <rdf:Description rdf:about="https://w3id.org/framester/data/framestercore/Activity"/>
            <rdf:Description rdf:about="https://w3id.org/framester/data/framestercore/Event"/>
        </owl:members>
    </rdf:Description>
</rdf:RDF>



<!-- Generated by the OWL API (version 4.5.26.2023-07-17T20:34:13Z) https://github.com/owlcs/owlapi -->

